\section{The Geometric Inequality}\label{GeometricInequalitySection}
In this section we will finalize the proof of Theorem \ref{MainDecompTheorem} by proving the geometric inequality \eqref{GeometricInequality}. We will use an induction argument based on a recursive integral formula for the Jacobian. This was first done in \cite{DW}, and we refer to Section $5$ in the same paper for a full derivation of the formula.
\begin{prop}\label{DW-Prop}
Given a curve $\gamma:I\to\R^d$, let $L_d=L_\g$ denote the torsion of the curve, and $L_i$ denote the determinant of the $i\times i$ minor matrix,
\[
L_i(t)=\det\begin{pmatrix}
\g_1'(t)&\ldots&\g_1^{(i)}(t)\\
\vdots&\ddots&\vdots\\
\g_i'(t)&\ldots&\g_i^{(i)}(t)
\end{pmatrix}.
\]
Define the map $\Gamma:I^d\to\R^d$ given by,
\[
\Gamma(t_1,\ldots,t_d)=\sum_{i=1}^d\g(t_i).
\]
Then the Jacobian of $\Gamma$ is given by
\[
J_\Gamma(t_1,\ldots,t_d)=\Lambda_d(t_1,\ldots,t_d),
\]
where $\Lambda_j$ satisfies the recursive formula,
\begin{align*}
    \Lambda_1(t)=&\frac{L_{d-2}(t)L_d(t)}{L_{d-1}(t)^2}\\
    \Lambda_j(t_1,\ldots,t_j)=&\prod_{i=1}^j\frac{L_{d-j-1}(t_i)L_{d-j+1}(t_i)}{L_{d-j}(t_i)^2}\int_{t_1}^{t_2}\ldots \int_{t_{j-1}}^{t_{j}}\Lambda_{j-1}(s_1,\ldots,s_{j-1})ds_{j-1}\ldots ds_1.
\end{align*}
Here the convention $L_0(t)=L_{-1}(t)\equiv 1$ is used.
\end{prop}
As mentioned earlier, for simple curves the torsion $L_\g(t)=C_d\varphi^{(d)}(t)$ has a rather simple expression. Moreover, for each $i\times i$ minor we have $L_i(t)=C_i>0$. This gives an immediate corollary of Proposition \ref{DW-Prop} which simplifies the recursive formula. It is this simplification which is exploited below in giving an independent proof of the geometric inequality for simple curves.
\begin{corollary}\label{DW-Corollary}
Let $\varphi\in C^d(I)$, and let $\g:I\to\R^d$ be a simple curve of the form
\[
\g(t)=\left(t,t^2,\ldots,t^{d-1},\varphi(t)\right).
\]
Then following the notation of Proposition \ref{DW-Prop},
\begin{equation*}
    J_\Gamma(t_1,\ldots,t_d)=\Lambda_d(t_1,\ldots,t_d),
\end{equation*}
where the $\Lambda_j$ satisfies the simplified recursive formula,
\begin{align*}
    \Lambda_1(t)=C_d\varphi^{(d)}(t),\quad
    \Lambda_j(t_1,\ldots,t_j)=C_{j,d}\int_{t_1}^{t_2}\ldots \int_{t_{j-1}}^{t_{j}}\Lambda_{j-1}(s_1,\ldots,s_{j-1})ds_{j-1}\ldots ds_1,
\end{align*}
where $C_{j,d}>0$ is a positive combinatorical constant only dependent on $j$ and $d$.
\end{corollary}

The following lemma will serve as a base case for the induction argument. It will also be used several times during the induction argument itself.
\begin{lemma}\label{SingleIntegralInequality}
Let $\alpha\in \mathbb{R}_+$ and $t<\tau$. Then for any $a\notin [t,\tau]$,
\begin{equation}\label{BaseCaseEq}
    \int_t^\tau|s-a|^\alpha ds\geq C_\alpha|t-a|^\frac{\alpha}{2}|\tau-a|^\frac{\alpha}{2}|\tau-t|.
\end{equation}
\begin{proof}
Since $a\notin [t,\tau]$, there exist integers $n,m\in\mathbb{Z}$ such that
\[
2^{n-1}\leq |\tau-a|<2^{n},\quad 2^{m-1}\leq |t-a|<2^{m}.
\]
If $a<t$, then $m\leq n$.
Assume first that $n\geq m+1$. Then
\begin{align*}
    \int_{t}^{\tau}|s-a|^{\alpha}ds
    \geq& |t-a|^{\frac{\alpha}{2}}\int_{t}^{\tau}|s-a|^{\frac{\alpha}{2}}ds\\
    =& \frac{2}{\alpha+2}|t-a|^{\frac{\alpha}{2}}\left(|\tau-a|^{\frac{\alpha}{2}+1}-|t-a|^{\frac{\alpha}{2}+1}\right)\\
    =& \frac{2}{\alpha+2}|t-a|^{\frac{\alpha}{2}}|\tau-a|^{\frac{\alpha}{2}+1}\left(1-\frac{|t-a|^{\frac{\alpha}{2}+1}}{|\tau-a|^{\frac{\alpha}{2}+1}}\right)\\
    \geq&
    \frac{2}{\alpha+2}|t-a|^{\frac{\alpha}{2}}|\tau-a|^{\frac{\alpha}{2}+1}\left(1-2^{\left(\frac{\alpha}{2}+1\right)(m-n)}\right)\\
    \geq&
    \frac{1}{\alpha+2}|t-a|^{\frac{\alpha}{2}}|\tau-a|^{\frac{\alpha}{2}}|\tau-t|,
\end{align*}
where we have used that $|\tau-a|\geq |\tau-t|$ since $a<t<\tau$.
This proves \eqref{BaseCaseEq} in the case $n\geq m+1$. If $n=m$, then
\begin{align*}
    \int_{t}^{\tau}|s-a|^{\alpha}ds
    \geq \frac{2^{n\frac{\alpha}{2}}2^{n\frac{\alpha}{2}}}{2^{\alpha}}(\tau-t)
    \geq \frac{1}{2^{\alpha}}|t-a|^\frac{\alpha}{2}|\tau-a|^\frac{\alpha}{2}|\tau-t|,
\end{align*}
which concludes the proof with
\begin{equation*}
    C_\alpha=\min\left\{\frac{1}{\alpha+2},\frac{1}{2^\alpha}\right\}.
\end{equation*}

If $a>\tau$, then $m\geq n$, and $|t-a|\geq |\tau-a|$. The proof then follows by a similar argument as for the case $a<t$.
\end{proof}
\end{lemma}
\begin{prop}\label{GeoIneq}
Let $\gamma:I\to\R^d$ be a simple curve of the form\[
\g(t)=\left(t,t^2,\ldots,t^{d-1},\varphi(t)\right),\]
for some $\varphi\in C^d(I)$.
Assume that there exists an interval $I_0\subset I$ such that $\varphi^{(d)}$ is single-signed, and that there exist constants $C_1,C_2>0$, $\kappa\in\mathbb{Z}_+$ and $a\in \mathbb{R}\backslash I_0$ such that for any $t\in I_0$ 
\[
C_1|t-a|^\kappa\leq |\varphi^{(d)}(t)|\leq C_2|t-a|^\kappa.
\]
Then for any $(t_1,\ldots,t_d)\in I_0^d$ 
\[
|J_\Gamma(t_1,\ldots,t_d)|\geq C\prod_{j=1}^d|\varphi^{(d)}(t_j)|^{\frac{1}{d}}\prod_{l<k}|t_k-t_l|.
\]
\end{prop}
\begin{proof}
Since rearranging $t_i$ in the Jacobian only affects the sign, we may without loss of generality assume $t_1\leq t_2\ldots\leq t_d$. Moreover, as $\varphi^{(d)}$ is singled-signed on $I_0$, we also have,
\[
|\Lambda_2(t_1,t_2)|=C_d\int_{t_1}^{t_2}|\varphi^{(d)}(s)|ds,
\]
and so we may safely assume that all $\Lambda_l$ are positive. 

By corollary \ref{DW-Corollary}, the proof is complete if we can show that
\begin{equation}\label{inductionStep}
\Lambda_l(t_1,\ldots,t_l)\geq C\prod_{j=1}^l|\varphi^{(d)}(t_j)|^\frac{1}{l}\prod_{1\leq i<k\leq l}|t_k-t_i|
\end{equation}
for all $l$. This will be verified with an induction argument.

We start with the base case $l=2$. This follows from Lemma \ref{SingleIntegralInequality}, since
\begin{align*}
    \Lambda_2(t_1,t_2)=C_d\int_{t_1}^{t_2}|\varphi^{(d)}(s)|ds
    \geq& C \int_{t_1}^{t_2}|s-a|^{\kappa}ds\\
    \geq&
    C|t_1-a|^{\frac{\kappa}{2}}|t_2-a|^{\frac{\kappa}{2}}|t_2-t_1|
    \\
    \geq&
    C|\varphi^{(d)}(t_1)|^{\frac{1}{2}}|\varphi^{(d)}(t_2)|^{\frac{1}{2}}|t_2-t_1|.
\end{align*}


Assume now that \eqref{inductionStep} holds for some $l-1$. Then
\begin{align}\label{LambaIntegral1}
    \Lambda_l(t_1,\ldots,t_l)
    =&C
    \int_{t_{l-1}}^{t_l}\ldots\int_{t_1}^{t_2}\Lambda_{l-1}(s_1,\ldots,s_{l-1})ds_1\ldots ds_{l-1}\nonumber\\ 
    \geq&C
    \int_{t_{l-1}}^{t_l}\ldots\int_{t_1}^{t_2}\prod_{j=1}^{l-1}|\varphi^{(d)}(t_j)|^\frac{1}{l-1}\prod_{1\leq i<k\leq l-1}|s_k-s_i|ds_1\ldots ds_{l-1}\nonumber\\
    \geq& C
    \int_{t_{l-1}''}^{t_l'}\ldots\int_{t_1''}^{t_2'}\prod_{j=1}^{l-1}|s_j-a|^\frac{\kappa}{l-1}\prod_{1\leq i<k\leq l-1}|s_k-s_i|ds_1\ldots ds_{l-1},
\end{align}
where the points $t_i'$ and $t_i''$ are defined in such a way that we only integrate over the middle third of each interval, that is
\begin{align*}
    t_i':=&\frac{2t_{i}+t_{i-1}}{3},\quad 2\leq i\leq l,  
    \\t_{i}'':=&\frac{t_{i+1}+2t_i}{3},\quad 1\leq i\leq l-1.
\end{align*}

For any choice of $1\leq i<j\leq l-1$, consider  $s_i\in[t_i'',t_{i+1}']$, and $s_j\in[t_j'',t_{j+1}']$. Since $j>i$, it then follows that
\[
s_j-s_i\geq t_{j}''-t_{i+1}'=\frac{t_{j+1}+2t_j}{3}-\frac{2t_{i+1}+t_{i}}{3}=\frac{t_{j+1}-t_i}{3}+2\frac{t_{j}-t_{i+1}}{3}
\geq \frac{t_{j+1}-t_i}{3},\]
where we used that $t_j\geq t_{i+1}$. This implies
\[
\prod_{1\leq i<j\leq l-1}|s_j-s_i|\geq 3^{-\frac{(l-1)(l-2)}{2}}\prod_{1\leq i<j\leq l-1}|t_{j+1}-t_i|,
\]
which is the part of the Vandermonde determinant for which the indices differ by at least two.
Inserted into \eqref{LambaIntegral1}, and applying Lemma \ref{SingleIntegralInequality} with $\alpha=\kappa/(l-1)$, we see that
\begin{align}\label{LambaIntegral2}
    \Lambda_l(t_1,\ldots,t_l)
    \geq&
    C\prod_{1\leq i<j\leq l-1}|t_{j+1}-t_i|\prod_{k=1}^{l-1}\int_{t''_k}^{t'_{k+1}}|s_k-a|^\frac{\kappa}{l-1}ds_k
    \nonumber\\
    \geq&
    C\prod_{1\leq i<j\leq l-1}|t_{j+1}-t_i|\prod_{k=1}^{l-1}|t_{k+1}'-a|^\frac{\kappa}{2(l-1)}|t_{k}''-a|^{\frac{\kappa}{2(l-1)}}|t'_{k+1}-t_{k}''|.
\end{align}
Note that for any $1\leq k\leq l-1$,
\[
t_{k+1}'-t_k''=\frac{1}{3}(2t_{k+1}+t_k-(t_{k+1}+2t_k))=\frac{t_{k+1}-t_k}{3},
\]
which reduces \eqref{LambaIntegral2} to
\begin{equation}\label{LambdaIntegral3}
    \Lambda_l(t_1,\ldots,t_l)
    \geq
    \frac{C}{3^{l-1}}\prod_{1\leq i<j\leq l-1}|t_{j}-t_i|\prod_{k=1}^{l-1}|t_{k+1}'-a|^\frac{\kappa}{2(l-1)}|t_{k}''-a|^{\frac{\kappa}{2(l-1)}}.
\end{equation}
Moreover, for fixed $k$ and any $0<\beta_k< 1$, we have
\begin{align*}
    (t'_{k+1}-a)^\frac{\kappa}{2(l-1)}=\left(\frac{(t_k-a)+2(t_{k+1}-a)}{3}\right)^\frac{\kappa}{2(l-1)}
\geq&
C_{\beta_k}\left(\beta_k (t_{k}-a)+(1-\beta_k)(t_{k+1}-a)\right)^\frac{\kappa}{2(l-1)}\\
\geq&
C_{\beta_k}(t_{k}-a)^{\beta_k\frac{\kappa}{2(l-1)}}(t_{k+1}-a)^{(1-\beta_k)\frac{\kappa}{2(l-1)}},
\end{align*}
by the arithmetic-geometric mean inequality. Here the constant $C_{\beta_k}$ is
\[
C_{\beta_k}=\min\left(\frac{3\beta_k}{2},3(1-\beta_k)\right)^\frac{\kappa}{2(l-1)}.
\]Similarly, we can write
\begin{equation}\label{tk-estimate}
\begin{aligned}
    (t''_{k}-a)^\frac{\kappa}{2(l-1)}=&\left(\frac{2(t_k-a)+(t_{k+1}-a)}{3}\right)^\frac{\kappa}{2(l-1)}\\
\geq&
C_{\beta_k}\left(\beta_k (t_{k}-a)+(1-\beta_k)(t_{k+1}-a)\right)^\frac{\kappa}{2(l-1)}\\
\geq&
C_{\beta_k}(t_{k}-a)^{\beta_k\frac{\kappa}{2(l-1)}}(t_{k+1}-a)^{(1-\beta_k)\frac{\kappa}{2(l-1)}}.
\end{aligned}
\end{equation}
Using \eqref{tk-estimate} to estimate the right hand side of \eqref{LambdaIntegral3} one obtains, for any values $0< \beta_i<1$,
\begin{align*}
    &\prod_{k=1}^{l-1}|t_{k+1}'-a|^\frac{\kappa}{2(l-1)}|t_{k}''-a|^{\frac{\kappa}{2(l-1)}}\\
    &\geq C |t_1-a|^{\frac{\kappa}{2(l-1)}2\beta_1}|t_l-a|^{\frac{\kappa}{2(l-1)}2(1-\beta_{l-1})}\prod_{i=2}^{l-1}|t_i-a|^{\frac{\kappa}{2(l-1)}2(1+\beta_i-\beta_{i-1})}.
\end{align*}
The proof would follow if we can choose each exponent equal to $\kappa/l$. This condition gives rise to a linear system of equations,
\begin{align*}
\beta_1=\frac{l-1}{l},\quad \beta_i=\frac{l-1}{l}-1+\beta_{i-1}=\beta_{i-1}-\frac{1}{l},\quad \beta_{l-1}=1-\frac{l-1}{l}=\frac{1}{l}.
\end{align*}
By recursion, the solution is given by 
\begin{equation}\label{BetaChoice}
    \beta_{i}=\frac{l-i}{l}\in (0,1),
\end{equation}
for each $1\leq i \leq l-1$.
Thus, choosing $\beta_i$ as in \eqref{BetaChoice} we conclude that
\[
\prod_{k=1}^{l-1}|t_{k+1}'-a|^\frac{\kappa}{2(l-1)}|t_{k}''-a|^{\frac{\kappa}{2(l-1)}}
\geq C\prod_{j=1}^l|t_j-a|^\frac{\kappa}{l},
\]
which inserted into \eqref{LambdaIntegral3} gives
\begin{equation*}
    \Lambda_l(t_1,\ldots,t_l)
    \geq
    \frac{C}{3^{l-1}}\prod_{1\leq i<j\leq l-1}|t_{j}-t_i|\prod_{j=k}^l|t_k-a|^\frac{\kappa}{l}\geq C\prod_{j=k}^l|\varphi^{(d)}(t_k)|^\frac{1}{l}\prod_{1\leq i<j\leq l-1}|t_{j}-t_i|.
\end{equation*}
This concludes the proof.
\end{proof}

\begin{remark}
Once the assumptions of Proposition \ref{GeoIneq} are met, the geometric inequality follows directly from the polynomial geometric inequality given in \cite{DW}. This has to do with the recursive formula. Let $\upsilon(t)=(t,\ldots,t^{d-1},p(t))$ denote the polynomial simple curve with $p^{(d)}(t)=(t-a)^\kappa$.
Moreover, let $\Lambda_j$ be as in Proposition \ref{GeoIneq}, and let $\Sigma_j$ denote the recursive integrals associated to the curve $\upsilon$. From the equivalence of $\varphi^{(d)}$ and $p^{(d)}$, it follows that
\begin{align*}
|J_\Gamma(t_1,\ldots,t_d)|=|\Lambda_d(t_1,\ldots,t_d)|\geq C|\Sigma_d(t_1,\ldots,t_d)|=C|J_{\Upsilon}(t_1,\ldots,t_d)|,
\end{align*}
where $\Upsilon(t)=\sum_{j=1}^d\upsilon(t_i)$. However, since there already exists a geometric inequality for polynomial curves, we know that
\[
|J_\Gamma(t_1,\ldots,t_d)|\geq C|J_{\Upsilon}(t_1,\ldots,t_d)|\geq C\prod_{i=1}^d|t_i-a|^\frac{\kappa}{d}\prod_{k>l}|t_i-t_k|
\geq C\prod_{i=1}^d|\varphi^{(d)}(t_i)|^\frac{1}{d}\prod_{k>l}|t_i-t_k|,
\]
which then proves the geometric inequality.
\end{remark}