\section{Obtaining the solution to the LTV model}
\label{appendix:B}
% \section{Solving the Differential equation in Section
%  \ref{sec:linear}}
\label{sec:B}
 Here, we develop the solution (Equation
(\ref{eq:6})), to the LTV model, (Equation \ref{eq:linear:model})), in
Section \ref{sec:linear}.  We start with Equation~\ref{eq:linear:model}: 
\begin{equation*}
 \frac{dF}{dt}+(\lambda - \omega t) F(t) = \Fnominal (\alpha - \beta t).
\end{equation*}
Multiplying both sides of this equation by the integrating factor $\omega(t) =
e^{\lambda t - \frac{\omega t^2}{2}}$ and combining terms, we obtain:
\begin{equation*}
\frac{d}{dt} \left( \frac{F}{\Fnominal} e^{\lambda t - \frac{\omega t^2}{2}}
      \right)=(\alpha-\beta t)  e^{\lambda t - \frac{\omega t^2}{2}}.
    \end{equation*}
    Integrating both sides of this equation with respect to $t$:
\begin{equation*}
 \frac{F(t)}{\Fnominal}  e^{\lambda t - \frac{\omega t^2}{2}} -
      \frac{F(0)}{\Fnominal}=\int_0^t (\alpha-\beta \tau) e^{\lambda
        \tau - \frac{\omega \tau^2}{2}} d\tau.
    \end{equation*}
    Completing the square in the exponent:
 \begin{equation*}
  \frac{F(t)}{\Fnominal}       = e^{\frac{\omega t^2}{2} - \lambda t}
      \left(
        \frac{F(0)}{\Fnominal} + e^{\frac{\lambda^2}{2\omega}}
        \int_0^t
        (\alpha-\beta\tau) e^{-(\frac{\lambda}{\sqrt{2\omega}} - \sqrt{\frac{\omega}{2}}\tau)^2 }
        d\tau
      \right).
\end{equation*}
With the change of variables setting the quadratic in the exponent to
$p^2$:
\begin{equation*}
  \frac{F(t)}{\Fnominal}       = e^{\frac{\omega t^2}{2} - \lambda t}
      \left(
        \frac{F(0)}{\Fnominal} + \sqrt{\frac{2}{\omega}}e^{\frac{\lambda^2}{2\omega}}
        \int_{-\frac{\lambda}{\sqrt{2\omega}}}^{\sqrt{\frac{\omega}{2}}t - \frac{\lambda}{\sqrt{2\omega}}}     
        \left(\alpha- \frac{\beta\lambda}{\omega} -
          \beta\sqrt{\frac{2}{\omega}}p \right) e^{-p^2 } d p
      \right).
\end{equation*}
The second term of the integral can be integrated immediately, and the
first term can be written in terms of the error function.  With
$\erf(z) = \frac{2}{\sqrt{\pi}} \int_0^z e^{-\tau^2} d\tau,$ the result is
% -------------------------------------------------------------------------------------------
% Solution in terms of erf(z) = \frac{2}{\sqrt{\pi} \int_0^z e^{-\tau^2} d\tau
% -------------------------------------------------------------------------------------------
  \begin{equation*}
    \frac{F(t)}{\Fnominal}=
e^{\frac{\omega t^2  }{2}-\lambda  t} \left(\frac{F(0)}{\Fnominal}+\frac{\sqrt{\frac{\pi }{2}} e^{\frac{\lambda
   ^2}{2 \omega }} (\alpha  \omega -\beta  \lambda ) \left(\text{erf}\left(\frac{\lambda
   }{\sqrt{2 \omega }}\right)+\text{erf}\left(\frac{t \omega
     -\lambda }{\sqrt{2 \omega }}\right)\right)}{\omega ^{3/2}}+\frac{\beta 
   \left(e^{\lambda  t-\frac{\omega t^2 }{2}}-1\right)}{\omega }\right).
\end{equation*}
% -------------------------------------------------------------------------------------------
% where
%\begin{equation*}
% \erf(z) = \frac{2}{\sqrt{\pi}} \int_0^z e^{-\tau^2} d\tau.
% \end{equation*}

