\documentclass{FeasibleOLG_main.tex}{subfiles}
\begin{document}



\subsection{Proof of \autoref{lem:2}}
\label{proof:lem2}
\begin{proof}



\begin{comment}
\begin{align*}
	(1+\Delta +\cdots +\Delta ^{n-1})^2\times\frac{d W(\Delta) }{d\Delta }&=\frac{(\sum _{k=1}^n\Delta ^{k-1})^2}{T\delta ^{T-1}}\times\frac{ d\frac{\sum _{k=1}^n\Delta ^{k-1}w_k}{\sum _{k=1}^n\Delta ^{k-1}}}{d\delta}\\	
	&=\sum _{k=1}^{n-1}\left \{\sum _{l=1}^k(k-l+1)\Delta ^{k+l-2}(w_{k+1}-w_l) \right \}.
\end{align*}
	
\end{comment}




For $a^{[n]} \in \mathcal{A}^{*}_{\lambda}(\Delta)$, denote the numerator of $\frac{\partial W_{ \lambda}}{\partial \Delta } (a^{[n]},\Delta )$ by $\eta(\Delta)$. We will show that $\eta (\Delta) \leq 0$, thereby $\frac{\partial W_{ \lambda}}{\partial \Delta } (a^{[n]},\Delta ) \leq 0$. From \eqref{eq:nn3}, observe that, for $u^{[n]} \in \mathcal{U}^{*}_{\lambda}(\Delta)$,
\begin{align*}
\eta (\Delta) &= \left (\sum_{k=1}^n \frac{d\Delta^{k-1} }{d\Delta }w_k (u^{[n]}) \right) \left(\sum_{m=1}^n \Delta^{m- 1} \right) - \left( \frac{d \sum_{m=1}^{n} \Delta^{m-1}} { d\Delta}\right)  \sum_{k=1}^n \Delta^{k-1} w_k(u^{[n]})\\
&=\left (\sum_{k=1}^n (k-1)\Delta^{k-2} w_k(u^{[n]}) \right) \left(\sum_{m=1}^n \Delta^{m-1} \right) - \left(\sum_{k=m}^{n} (m-1) \Delta^{m-2}\right)  \sum_{k=1}^n \Delta^{k-1} w_k(u^{[n]})\\
&=\sum_{k=1}^n \left ((k-1) \Delta^{k-2} \sum_{m=1}^{n} \Delta^{m-1} - \left( \sum_{m=1}^n (m-1) \Delta^{m-1}  \right) \Delta^{k-2}  \right) w_k(u^{[n]})\\
&=\sum_{k=1}^n  \left( \sum_{m=1}^n (k-m) \Delta^{k+m-3} \right)w_k(u^{[n]}).
\end{align*}
Recall $m$-th constraint, $m \in \{ 1, \dots, n-1\}$, is
$$-\sum_{k=1}^m \Delta^{k-1} w_k (u^{[n]})  + \sum_{k=1}^m \Delta^{k-1} w_{n-m+k} (u^{[n]})\leq 0   \quad (\# m)$$
We will show that 
$$\eta (\Delta) = \sum _{m=1}^{n-1}p_m\times (\text{LHS of } \# m),$$
where for $1\leq m\leq n-1$
$$p_m \equiv \Delta ^{n-2}+\Delta ^{n-3}+\cdots +\Delta ^{n-m-1}.$$
Note that as $p_m \geq 0$, this implies $\eta (\Delta) \leq 0$. To see the equality, fix $j \in \{ 1,\dots, n\}$. Observe for any constraint $m\geq j$, there exists a non-positive term $- \Delta^{j-1}w_j (u^{[n]})$. And for any constraint $m$ with $j \geq n-m+1$, there exists a non-negative term $\Delta^{j-n+m-1} w_j (u^{[n]})$. Therefore the coefficient of $w_j (u^{[n]})$ is 
\begin{align*}
&\sum_{m = j}^{n-1} p_m (-\Delta ^{j-1} ) + \sum_{m =n+1-j}^{n-1} p_m \Delta^{j-n+m-1}\\
&=\sum_{m = j}^{n-1} (\Delta^{n-2} + \cdots + \Delta^{n-m-1}) (-\Delta^{j-1}) + \sum_{ m=n+1-j}^{n-1} (\Delta^{n-2} + \cdots + \Delta^{n-m-1}) \Delta^{j-n+m-1} \\
&=\sum_{ m=j}^{n-1} (-\Delta^{n+j-3} - \cdots - \Delta^{n-m+j-2})  + \sum_{m=n+1-j}^{n-1} (\Delta^{j+m-3} +\cdots + \Delta^{j-2})\\
&=(- \Delta^{n+j-3}- \cdots - \Delta^{n-2}) + (- \Delta^{n+j-3} - \cdots - \Delta^{n-1}) + \cdots + (-\Delta^{n+j-3} - \cdots - \Delta^{j-1})  \\
&+ (\Delta^{n-2} + \cdots + \Delta^{j-2}) + (\Delta^{n-1} + \cdots + \Delta^{j-2})  + \cdots + (\Delta^{j+n-4} + \cdots + \Delta^{j-2})\\
&=- \Delta^{n+j-3} ((n-j)-0) - \Delta^{n+j-4} ((n-j)-1)- \cdots - \Delta^{n-2} ((n-j) -(j-1))\\
&- \Delta^{n-3} ((n-j-1)- (j-1))- \cdots - \Delta^{j-1} (1- (j-1))- \Delta^{j-2} (0-(j-1))\\
&=\sum_{m=1}^n (j-m) \Delta^{j+m-3}.
\end{align*}


\begin{comment}
	Observe that
$$a + b \delta \geq b + c \delta$$
$$\iff a-c + b \delta \geq b-c + c\delta $$
$$\iff a-c \geq   (b-c) (1- \delta) $$
$$\iff \delta (a-c) \geq (\delta-\delta^2)(b-c)$$
Observe also 
$$\delta^2 (c-b) + 2 \delta (c-a) + b-a$$
$$\leq \delta ^2 (c-b) + 2 \delta (c-a) + \delta (b-c) = (\delta-\delta^2) (b-c) + 2\delta (c-a)$$
$$\leq \delta (a-c) + 2 \delta (c-a) = \delta (c-a) \leq 0.$$	
where the first inequality comes from item 2 of the lemma. The last inequality comes from item 1 of the lemma.

\end{comment}
\end{proof}



\end{document}
