\input{inputs/propositions.tex}
\customparagraph{Proof of propositions}
    \setcounter{proposition}{1}
    \begin{proof}[Proof of Proposition~\ref{prop:conditionalProbMinimum}]
        Let \( M_V = \min\limits_{v = 1, \dots, V} \{ k_v \} \), then we need to prove that
        \begin{align}
            \Prob(M_{V+1} \le M_V \mid k_1, \dots, k_V) = 1.
        \end{align}
        Due to the properties of the minimum operator, we have
        \begin{align}
            \begin{cases}
                M_{V+1} = M_V, \quad&\text{if } k_{V+1} \ge M_V \\
                M_{V+1} < M_V, &\text{otherwise}
            \end{cases}.
        \end{align}
        Hence, \( M_{V+1} \le M_V \) regardless of the value of \( k_{V+1} \), which gives
        \begin{align}
            \Prob(M_{V+1} \le M_V \mid k_1, \dots, k_V) = 1.
        \end{align}
    \end{proof}

    \begin{proof}[Proof of Proposition~\ref{prop:expectationMinimum}]
        Let \( M_V = \min\limits_{v = 1, \dots, V} \{ k_v \} \), then
        \begin{align}
            F_{M_V}(x) &\coloneqq \Prob(M_V \le x) = 1 - \Prob(M_V > x) \\
            &= 1 - \Prob(k_1 > x \cap \dots \cap k_V > x) \\
            &= 1 - (1 - F_{k_v}(x))^V
        \end{align}
        where \( F_{k_v}(x) = \Prob(k_v \le x) \).

        Since \( M_V \) is a non-negative random variable, we have
        \begin{align}
            \E(M_V) = \sums{x=0}{\infty}(1 - F_{M_V}(x)) = \sums{x=0}{\infty}(1 - F_{k_v}(x))^V.
        \end{align}
        Hence
        \begin{align}
            \nonumber
            &\E(M_V) - \E(M_{V+1}) \\
            &= \sums{x=0}{\infty}(1 - F_{k_v}(x))^V - \sums{x=0}{\infty}(1 - F_{k_v}(x))^{V+1} \\
            &= \sums{x=0}{\infty}(1 - F_{k_v}(x))^V (1 - (1 - F_{k_v}(x))) \\
            &= \sums{x=0}{\infty}
                \underbrace{(1 - F_{k_v}(x))^V}_{\ge 0}
                \underbrace{F_{k_v}(x) }_{\ge 0} \ge 0
        \end{align}
        which is a sum of non-negative terms, since \( F_{k_v}(x) \in [0, 1] \) is a probability.
        This gives
        \begin{align}
            \E(M_{V+1}) \le \E(M_V)
        \end{align}
    \end{proof}