\subsection{Sub-optimality for CCB-PV with Extended Policy Class}\label{proof:extended PV Subopt}
For CCP-PV with extended policy class, we define event $\cE$ by
\begin{align}
    \cE &= \Big\{\abr{\EE_{\cD_k}\sbr{\alpha^\pie_k(\vh, \cY_k) \theta_k(\cZ_k)} - \EE_{\mu_k}\sbr{\alpha^\pie_k(\vh, \cY_k) \theta_k(\cZ_k)}} \le \eta_k\rbr{L_\alpha\nbr{\theta_k}_{\mu_k, 2}+\eta_k},\nend
    &\quad \abr{\norm{\theta_k}^2_{\cD_k, 2}-\norm{\theta_k}^2_{\mu_k, 2}}\le \frac 1 2\rbr{\norm{\theta_k}^2_{\mu_k, 2}+\eta_k^2}, 
    \forall \vh\in \vH, \forall \pie\in\Pie, \forall \theta_k\in\Theta_k, \forall k\in\{1, \cdots, K\}\Big\}, \label{def:extended cE}
\end{align}
where $\eta$ bounds the critical radius for $\alpha^\pie_k(\vh, \cY_k) \theta_k(\cZ_k)$ and $\theta_k$.
In contrast to the definition in \eqref{def:cE}, $\eta$ also bounds the critical radius of the policy class $\Pie$.
We remark that Theorem \ref{thm:Fast rate} still holds on the event defined by \eqref{def:extended cE}.
Similarly, we define the pessimistic $\gpessi{\pie}$ by
\begin{align}
    \gpessi{\pie}=\arg\inf_{g\in\CICATE^\pie(e_\cD)} v(g). \label{def:extended gpessi}
\end{align}
The sub-optimality of policy $\piepessi$ is given by
\begin{align}\label{eq:extended regret}
    \text{SubOpt}(\piepessi) &=v^{\piestar}-v^{\piepessi} \nend
    &= \underbrace{v^{\piestar} - v(\gpessi{\piestar})}_{\text{(i)}} + \underbrace{v(\gpessi{\piestar}) - v(\gpessi{\piepessi})}_{\text{(ii)}} + \underbrace{v(\gpessi{\piepessi}) - v(\gH{\piepessi})}_{\text{(iii)}} + \underbrace{v(\gH{\piepessi}) - v^{\piepessi}}_{\text{(iv)}}\nend
    &\overset{\cE}{\lesssim} \underbrace{v^{\piestar} - v(\gpessi{\piestar})}_{\text{(i)}} + \underbrace{v(\gH{\piepessi}) - v^{\piepessi}}_{\text{(iv)}}, 
\end{align}
where $\text{(ii)}\le 0$ holds by the definition of $\piepessi$ in \eqref{def:extended piepessi} and $\text{(iii)} \overset{\cE}{\lesssim} 0$ holds by definition of $\gpessi{\pie}$ in \eqref{def:extended gpessi} and the fact that $\gH{\piepessi}\in\CICATE^\piepessi(e_\cD)$ on event $\cE$ by theorem \ref{thm:Fast rate}. Following \eqref{eq:iv upper}, we have,
\begin{align*}
    \text{(iv)} &= v(\gH{\piepessi}) - v^{\piepessi}\nend
    & = \int_{\cX\times\cA}\rbr{\gH{\piepessi}(X) - g^\piepessi(X)}\tpr(x)\rd x\rd a\nend
    & \le \sup_{\pie\in\Pie}\nbr{\gH{\pie}-g^\pie}_{ \tpr, 2}\le \vareH.
\end{align*}
Similar to \S\ref{proof: subopt of PV}, we give a brief proof to bound (i) in \eqref{eq:extended regret}.
We first study the difference between $\hpessik{2}{\piestar}$ and $\h{2}{\piestar}$ by
\begin{align}
    &\EEob\sbr{\h{2}{\piestar}(A, W, X)-\hpessik{2}{\piestar}(A, W, X)\given A, X, Z, (R_X, R_Z)=\ind}\nend
    &=\EEob\sbr{\EEob\sbr{\h{2}{\piestar}(A, W, X)-\hpessik{2}{\piestar}(A, W, X)\given A, W, X, Z, (R_W, R_X, R_Z)=\ind}\given A, X, Z, (R_X, R_Z)=\ind}\nend
    &=\EEob\sbr{\h{1}{\piestar}(Y, A, X, Z)  -\hpessik{1}{\piestar}(Y, A, X, Z) \given A, X, Z, (R_X, R_Z)=\ind} \nend
    &\quad + \EEob\sbr{\EEob\sbr{\hpessik{1}{\piestar}(Y, A, X, Z)-\hpessik{2}{\piestar}(A, W, X)\given A, W, X, Z, (R_W, R_X, R_Z)=\ind}\given A, X, Z, (R_X, R_Z)=\ind}\nend
    &=- \cT_1\vhpessi{\piestar}(A, X, Z) - \EEob\sbr{\cT_2\vhpessi{\piestar}(A, W, X, Z)\given A, X, Z, (R_X, R_Z)=\ind}, \label{eq:extended PV 1}
\end{align}
which is identical to the proof in \S\ref{proof: subopt of PV} and the equality holds following the same reasons for \eqref{eq:PV 1}. 
For the error in the estimated CATE, we have
\begin{align*}
    &g^\piestar(X)-\gpessi{\piestar}(X)\nend
    &=\EEob\sbr{\rbr{\h{3}{\piestar}(Y, A, X) - \hpessik{3}{\piestar}(Y, A, X)} + \rbr{\hpessik{3}{\piestar}(Y, A, X)-\gpessi{\piestar}(X)}\given X, R_X=1}\nend
    &=\EEob\sbr{\EEob\sbr{\h{3}{\piestar}(Y, A, X)-\hpessik{3}{\piestar}(Y, A, X)\given A, W, X, (R_W, R_X)=\ind}\given X, R_X=1} - \cT_4\vhpessi{\piestar}(X),
\end{align*}
where the first equality holds by \eqref{eq:PV ID extension 4} which states that 
$$\EEob\sbr{g^\piestar(X, A') - \h{3}{\piestar}(Y, A, X, A')\given X, A', R_X=1}=0.$$
The second equality holds also by noting that $R_W\indep (Y, R_X)\given(A, X, W)$ and the definition of $\cT_4$ in the CCB-PV case. We continue with \eqref{eq:PV ID extension 3} which states that
$$\EEob\sbr{\h{3}{\piestar}(Y, A, X)-\sum_{a'\in\cA}\h{2}{\piestar}(a', W, X)\given A, W, X, (R_W, R_X)=\ind}=0, $$
and it holds for $g^\piestar(X)-\gpessi{\piestar}(X)$ that
\begin{align}
    &g^\piestar(X)-\gpessi{\piestar}(X)\nend
    &=\EEob\sbr{\EEob\sbr{\sum_{a'\in\cA}\rbr{\h{2}{\piestar}(a', W, X)-\hpessik{2}{\piestar}(a', W, X)}\given A, W, X, (R_W, R_X)=\ind}\given X, R_X=1}\nend
    &\quad + \EEob\sbr{\EEob\sbr{\sum_{a'\in\cA}\hpessik{2}{\piestar}(a', W, X)-\hpessik{3}{\piestar}(Y, A, X)\given A, W, X, (R_W, R_X)=\ind}\given X, R_X=1}\nend
    &\quad  - \cT_4\vhpessi{\piestar}(X)\nend
    &=\sum_{a'\in\cA}\EEob\sbr{\h{2}{\piestar}(a', W, X)-\hpessik{2}{\piestar}(a', W, X)\given X, R_X=1} \nend
    &\quad -\EEob\sbr{\cT_3\vhpessi{\piestar}(A, W, X)\given X, R_X=1} -\cT_4\vhpessi{\piestar}(X),\label{eq:extended PV 2}
\end{align}
where the second equality holds by definition of $\cT_3$ in the CCB-PV case. 
Now we plug \eqref{eq:extended PV 2} into (i) of \eqref{eq:extended regret} and it follows that
\begin{align}
    \text{(i)} &= v^{\piestar} - v(\gpessi{\piestar})\nend
    &=\int_{\cX} \rbr{g^\piestar(x)-\gpessi{\piestar}(x)}\tpr(x)\rd x\nend
    &=\underbrace{\int_{\cX}\EEob\sbr{\sum_{a'\in\cA}\rbr{\h{2}{\piestar}(a', W, X)-\hpessik{2}{\piestar}(a', W, X)}\given X=x,  R_X=1} \tpr(x)\rd x}_{(a)} \nend
    &\quad \underbrace{-\int_{\cX}\EEob\sbr{\cT_3\vhpessi{\piestar}(A, W, X)\given X=x, R_X=1} \tpr(x)\rd x}_{(b)} \underbrace{-\int_{\cX}\cT_4\vhpessi{\piestar}(x) \tpr(x)\rd x}_{(c)}.\label{eq:extended PV 3}
\end{align}
To upper bound (b) and (c), we define two ratio functions $b_4:\cX\times\cA\rightarrow \RR$ and $b_3:\cW\times\cX\times\cA\times\cA'\rightarrow \RR$ by
\begin{gather}
    b_4(x, a') = \frac{\tpr(x)}{\pob(x\given R_X=1)}, \label{eq:extended PV b4}\\
    b_3(w, x, a, a') = \frac{\tpr(x)\pob(a, w\given x, R_X=1)}{\pob(x, a, w\given (R_W, R_X)=\ind)}.\label{eq:extended PV b3}
\end{gather}
For (b), with $b_3$ defined in \eqref{eq:extended PV b3} we have
\begin{align}
    (b) = -\EEob\sbr{\cT_3\vhpessi{\piestar}(A, W, X, A')b_3(W, X, A, A')\given (R_W, R_X)=\ind}\le \nbr{\cT_3\vhpessi{\piestar}}_{\mu_3, 2}\nbr{b_3}_{\mu_3, 2}. \label{eq:extended PV (b)}
\end{align}
Similarly, for (c) with $b_4$ defined in \eqref{eq:extended PV b4} we have
\begin{align}
    (c) = \EEob\sbr{-\cT_4\vhpessi{\piestar}(X, A')b_4(X, A')\given R_X=1}\le \nbr{\cT_4\vhpessi{\piestar}}_{\mu_4, 2}\nbr{b_4}_{\mu_4, 2}.\label{eq:extended PV (c)}
\end{align}
In addition, it holds for (a) that
\begin{align}
    (a)&=\int_{\cX}\EEob\sbr{\sum_{a'\in\cA}\rbr{\h{2}{\piestar}(a', W, X)-\hpessik{2}{\piestar}(a', W, X)}\given X=x,  R_X=1} \tpr(x)\rd x\nend
    &=\int_{\cX}\EEob\sbr{\sum_{a'\in\cA}\EEob\sbr{\h{2}{\piestar}(A, W, X)-\hpessik{2}{\piestar}(A, W, X)\given X, U, A=a, (R_X, R_Z)=\ind}\given X=x, R_X=1}
    \nend
    &\quad \cdot \tpr(x) \rd x \nend
    &= \EEob\bigg[\EEob\sbr{\h{2}{\piestar}(A, W, X)-\hpessik{2}{\piestar}(A, W, X)\given X, U, A, (R_X, R_Z)=\ind} \nend
    &\quad \cdot \frac{\pob(U\given X, R_x=1)\tpr(X)}{\pob(U, X, A\given (R_X, R_Z)=\ind)}\given (R_X, R_Z)=\ind\bigg], \label{eq:extended PV 4}
\end{align}
where the second equality holds by noting that $R_X\indep W\given X$, $A\indep W\given (X, U)$, and $(R_X, R_Z)\indep W\given (A, U, X)$. 
which prompts us to introduce another ratio function. 
Since $Z$ is overcomplete over $U$, there exists $b_1: \cX\times\cA\times\cZ\rightarrow \RR$ such that
\begin{align}
    \EEob\sbr{b_1(X, A, Z)\given X, U, A, (R_X, R_Z)=\ind} = \frac{\pob(U\given X, R_x=1)\tpr(X)}{\pob(U, X, A\given (R_X, R_Z)=\ind)}.\label{eq:extended PV 5}
\end{align}
Plugging \eqref{eq:extended PV 5} into \eqref{eq:extended PV 4}, it holds that
\begin{align*}
    (a) 
    &= \EEob\bigg[\EEob\sbr{\h{2}{\piestar}(A, W, X)-\hpessik{2}{\piestar}(A, W, X)\given X, U, A, (R_X, R_Z)=\ind}\nend
    & \quad \cdot \EEob\sbr{b_1(X, A, Z)\given X, U, A, (R_X, R_Z)=\ind}\given (R_X, R_Z)=\ind\bigg]\nend
    & = \EEob\sbr{\rbr{\h{2}{\piestar}(A, W, X)-\hpessik{2}{\piestar}(A, W, X)}b_1(X, A, Z)\given  (R_X, R_Z)=\ind}\nend
    & = \EEob\sbr{\EEob\sbr{\h{2}{\piestar}(A, W, X)-\hpessik{2}{\piestar}(A, W, X)\given X, A, Z, (R_X, R_Z)=\ind} b_1(X, A, Z)\given  (R_X, R_Z)=\ind},
\end{align*}
where the second equality holds by noting that $W\indep (Z, R_Z)\given (X, A, U, R_X)$. Now plugging in \eqref{eq:extended PV 1}, we have
\begin{align*}
    (a) &= -\EEob\bigg[\rbr{\cT_1\vhpessi{\piestar}(A, X, Z) + \EEob\sbr{\cT_2\vhpessi{\piestar}(A, W, X, Z)\given A, X, Z, (R_X, R_Z)=\ind}}\nend
    &\quad \cdot b_1(X, A, Z)\given (R_X, R_Z)=\ind\bigg]\nend
    &= -\EEob\sbr{\cT_1\vhpessi{\piestar}(A, X, Z) b_1(X, A, Z)\given (R_X, R_Z)=\ind}\nend
    &\quad - \EEob\sbr{\EEob\sbr{\cT_2\vhpessi{\piestar}(A, W, X, Z)b_1(X, A, Z)\given A, W, X, (R_W, R_X, R_Z)=\ind}\given (R_X, R_Z)=\ind}\nend
    &= -\EEob\sbr{\cT_1\vhpessi{\piestar}(A, X, Z) b_1(X, A, Z)\given (R_X, R_Z)=\ind}\nend
    &\quad - \EEob\sbr{\cT_2\vhpessi{\piestar}(A, W, X, Z)b_1(X, A, Z)\frac{\pob(A, W, X\given (R_X, R_Z)=\ind)}{\pob(A, W, X\given (R_W, R_X, R_Z)=\ind)}\given (R_W, R_X, R_Z)=\ind} ,
\end{align*}
where the second equality holds by $R_W\indep (Z, R_X, R_Z)\given (A, W, X)$.
We thereby define $b_2: \cA\times\cW\times\cX\times\cZ\rightarrow \RR$ by
\begin{align*}
    b_2(A, W, X, Z) = b_1(X, A, Z)\frac{\pob(A, W, X\given (R_X, R_Z)=\ind)}{\pob(A, W, X\given (R_W, R_X, R_Z)=\ind)}.
\end{align*}
We then arrive at
\begin{align}
    (a)&=-\EEob\sbr{\cT_1\vhpessi{\piestar}(A, X, Z) b_1(X, A, Z)\given (R_X, R_Z)=\ind}\nend
    &\quad - \EEob\sbr{\cT_2\vhpessi{\piestar}(A, W, X, Z)b_2(A, W, X, Z)\given (R_W, R_X, R_Z)=\ind}\nend
    &\le \nbr{\cT_1\vhpessi{\piestar}}_{\mu_1, 2}\nbr{b_1}_{\mu_1, 2} + \nbr{\cT_2\vhpessi{\piestar}}_{\mu_2, 2}\nbr{b_2}_{\mu_2, 2}, \label{eq:extended PV (a)}
\end{align}
Combining \eqref{eq:extended PV (a)}, \eqref{eq:extended PV (b)} and \eqref{eq:extended PV (c)} with \eqref{eq:extended PV 3}, we have
\begin{align*}
    v^{\piestar} - v(\gpessi{\piestar})
    \le \sum_{k=1}^4 \nbr{\cT_k\vhpessi{\piestar}}_{\mu_k, 2}\nbr{b_k}_{\mu_k, 2} \le \max_{k\in\{1, 2, 3,4\}}\nbr{\cT_k\vhpessi{\piestar}}_{\mu, 2}  \sum_{k=1}^4\nbr{b_k}_{\mu_k, 2}, 
\end{align*}
Therefore, for the sub-optimality given in \eqref{eq:extended regret}, it holds by the conclusion of Theorem \ref{thm:Fast rate} that
\begin{align*}
    \SubOpt(\piepessi)\overset{\cE}{\lesssim} \sum_{k=1}^4 \nbr{b_k}_{\mu_k, 2} \cdot \big(\cO(\vareTheta) + \cO(\vareH) + \cO\rbr{\sqrt{e_\cD}} +  \cO\rbr{\eta}\big),
\end{align*}
which completes the proof of Theorem \ref{thm:extended PV subopt}.