\subsection{Proof of \Cref{thm:scg_bound}}\label{apx:thm2}
We first make use the following lemma from Mokhtari et al. which bounds the variance in momentum error:
\begin{lemma}{(Mokhtari et al. 2018, Lemma 2)}
Given a momentum parameter $p_t = \frac{4}{(t+8)^{2/3}}$, the gradient estimates $\gb_t$ have the following property:
\begin{equation*}
    \mathbb{E}\left[\norm{\nabla F(\x_t) - \gb_t}^2\right] \leq \frac{Q}{(t+9)^{2/3}}
\end{equation*}
\end{lemma}
We note that as a corollary to this lemma, the Chebyshev inequality gives us the following high probability bound:
\begin{equation}
    \mathbb{P}\left(\norm{\nabla F(\x_t) - \gb_t} \geq \delta\sqrt{\frac{Q}{(t+9)^{2/3}}}\right) \leq \frac{1}{\delta^2}
\end{equation}
Squaring both terms inside the condition:
\begin{equation}
    \mathbb{P}\left(\norm{\nabla F(\x_t) - \gb_t}^2 \geq \delta^2\frac{Q}{(t+9)^{2/3}}\right) \leq \frac{1}{\delta^2}
\end{equation}
Now we are ready to begin the proof of \cref{thm:scg_bound}.
\begin{proof}
Starting with the following inequality derived in \cite{mokhtari2018conditional} (Mokhtari et al. 2018, eq. 20)  we have:
\begin{equation*}
    F(\x_{t+1}) - F(\x_t) \geq \frac{1}{T}(F(\x^*)-F(\x_t)) - \frac{LD^2}{2T^2} - \frac{1}{2T}(4\beta_t D^2 + \frac{\norm{\nabla F(\x_t) - \gb_t}^2}{\beta_t})
\end{equation*}

Instead of taking the expectations of both sides as in \cite{mokhtari2018conditional}, we immediately apply the inequality recursively from $t=0,1,\dots,T-1$ to get
\begin{equation*}
    F(\x^*)-F(\x_T) \leq (1-\frac{1}{T})^T (F(\x^*)-F(\x_0)) + \sum_{t=0}^{T-1} \frac{1}{2T}\left[4\beta_tD^2 + \frac{\norm{\nabla F(\x_t) - \gb_t}^2}{\beta_t}\right] + \frac{LD^2}{2T^2} 
\end{equation*}
Looking at the term $\sum_{t=0}^{T-1}\norm{\nabla F(\x_t) - \gb_t}^2$, we can use the union bound as follows:
\begin{equation*}
    \mathbb{P}(\sum_{t=0}^{T-1}\norm{\nabla F(\x_t) - \gb_t}^2 \geq \delta^2 \sum_{t=0}^{T-1}\frac{Q}{(t+9)^{2/3}}) \leq \sum_t \frac{1}{\delta^2} = \frac{T}{\delta^2}
\end{equation*}
Therefore we know that with probability at least $1-\frac{T}{\delta^2}$ that the inequality in the opposite direction is true.

Then choosing $\beta_t = \frac{\delta \sqrt{Q}}{2D(t+9)^{1/3}}$, we get the upper bound:
\begin{equation}
        F(\x^*)-F(\x_T) \leq \frac{1}{e} (F(\x^*)-F(\x_0)) + \sum_{t=0}^{T-1} \delta \frac{2Q^{1/2}D}{(t+9)^{1/3}T} + \frac{LD^2}{2T^2}
\end{equation}
Therefore with probability greater than $1-\frac{T}{\delta^2}$ we have the following bound:
\begin{equation}
        F(\x^*)-F(\x_T) \leq \frac{1}{e} (F(\x^*)-F(\x_0)) +  \delta\frac{2Q^{1/2}D}{T^{1/3}} + \frac{LD^2}{2T^2} 
\end{equation}
Some more manipulation, and we have with probability greater than $1-\frac{T}{\delta^2}$
\begin{equation}
    F(\x_T) \geq (1-\frac{1}{e})F(\x^*) - \delta\frac{2Q^{1/2}D}{T^{1/3}} -\frac{LD^2}{2T^2}
\end{equation}
\end{proof}



