\subsection{Proof of \Cref{thm:scg_plus}}\label{sec:proof_scg_plus}
Similarly to the proof of \cref{thm:scg_bound}, we first utilize a bound on the variance of the gradient approximation:
\begin{lemma}{(Hassani et al. 2020, Lemma 2)}
Given the gradient approximations $g_t$ as calculated in \cref{alg:scg_plus}, target error $\epsilon$, and batch size $|\mathcal{M}|=1/\epsilon$, we have
\begin{equation*}
    \mathbb{E}\left[\norm{\nabla F(\x_t) - \gh_t}^2\right] \leq (1+\epsilon t) L^2 D^2 \epsilon^2
\end{equation*}
\end{lemma}
Larger batch sizes mean more queries of our stochastic oracle, but have the benefit of reducing the target error $\epsilon$. If we choose $\epsilon = 1/t$ we get the bound:
\begin{equation*}
    \mathbb{E}\left[\norm{\nabla F(\x_t) - \gh_t}^2\right] \leq \frac{2L^2D^2}{t^2}
\end{equation*}
Notice that the residuals between the true gradient and these new estimates decay much more rapidly. Using the Chebyshev inequality we have
\begin{equation}
    \mathbb{P}\left(\norm{\nabla F(\x_t) - \gh_t}^2 \geq \delta^2\frac{2L^2D^2}{t^2}\right) \leq \frac{1}{\delta^2}
\end{equation}
The union bound is likewise
\begin{equation}
    \mathbb{P}\left(\sum_{t=0}^{T-1}\norm{\nabla F(\x_t) - \gh_t}^2 \geq \delta^2\sum_{t=0}^{T-1}\frac{2L^2D^2}{t^2}\right) \leq \frac{T}{\delta^2}
\end{equation}
Now we will begin the proof of \cref{thm:scg_plus}.
\begin{proof}
We intervene at the following inequality found in the original SCG++ expectation bound proof (Hassani et al. 2020, eq. 33):
\begin{equation*}
    F(\x^*)-F(\x_T) \leq (1-\frac{1}{T})^T (F(\x^*)-F(\x_0)) + \sum_{t=0}^{T-1} \frac{1}{2T}\left[\beta_tD^2 + \frac{\norm{\nabla F(\x_t) - \gh_t}^2}{\beta_t}\right] + \frac{LD^2}{2T^2} 
\end{equation*}
This time setting $\beta_t = \frac{\sqrt{2}\delta L}{t}$ we know with probability at least $1-\frac{T}{\delta^2}$
\begin{equation}
        F(\x^*)-F(\x_T) \leq \frac{1}{e} (F(\x^*)-F(\x_0)) + \sum_{t=0}^{T-1} \delta\frac{\sqrt{2}LD^2}{tT} + \frac{LD^2}{2T^2}
\end{equation}
With some rearrangement and simplification
\begin{equation}
    F(\x_T) \geq (1-\frac{1}{e})F(\x^*) - \delta \frac{LD^2}{T} -\frac{LD^2}{2T^2}
\end{equation}
\end{proof}

