

Here we list all the splitting functions, including ultra-collinear ones. Some of them have a $\zb$ pole and therefore they introduce divergences in the DGLAP equations when $z_{\rm max}=1$. To deal with such divergences, we use the $+$ distribution, defined as
%
\begin{equation}
\int_x^1 dz\frac{f(z)}{(1-z)_+} = \int_x^1 dz\frac{f(z)-f(1)}{1-z}-f(1)\int_0^x\frac{dz}{1-z} = \int_x^1 dz\frac{f(z)-f(1)}{1-z}+f(1)\log(1-x)~. \label{eq:def+}
\end{equation}
%
As already discussed, since the SM is a chiral theory we separate vector polarizations and fermion helicities in the splitting functions.

\subsection{Massless splitting functions}
We start with the splitting functions of the form in Eq.~\eqref{eq:ampl_splitting_generic_massless}. Here $f$ labels a fermion, $V$ a gauge boson and $h$ a scalar. We do not specify the polarization of the particle $C$, since in the computation we sum over it.

\be\begin{split}
    P_{ff}^V(z)  &\equiv P_{f_Lf_L}^V(z) = P_{f_Rf_R}^V(z) = \frac{1+z^2}{\zb_+} ~,\\
    P_{V_+f_L}^{f}(z) &= P_{V_-f_R}^{f}(z) = \frac{\zb^2}{z}~,\\
    P_{V_-f_L}^{f}(z) &= P_{V_+f_R}^{f}(z) = \frac{1}{z}~,\\
    P_{f_LV_+}^{f}(z) &= P_{f_RV_-}^{f}(z) = \zb^2~,\\
    P_{f_LV_-}^{f}(z) &= P_{f_RV_+}^{f}(z) = z^2~,\\
\end{split}\ee
%
\be\begin{split}
    P_{ff}^h(z) &\equiv P_{f_Lf_R}^h(z) = P_{f_Rf_L}^h(z) = \frac{\zb}{2}~,\\
    P_{hf}^f(z) &\equiv P_{hf_L}^{f}(z) = P_{hf_R}^{f}(z) = \frac{z}{2}~,\\
    P_{fh}^f(z) &\equiv P_{f_Lh}^{f}(z) = P_{f_Rh}^{f}(z) = \frac{1}{2}~,\\
\end{split}\ee
%    
\be\begin{split}
    P_{V_\pm h}^h(z) &= \frac{\zb}{z}~,\\
    P_{Vh}^h(z) &\equiv P_{V_+ h}^h(z)+P_{V_- h}^h(z) = \frac{2\zb}{z}~,\\
    P_{hh}^V(z) &= \frac{2z}{\zb_+}~,\\
    P_{hV}^h(z) &\equiv P_{hV_+}^h(z) = P_{hV_-}^h(z) = z\zb~,\\
\end{split}\ee
%
\be\begin{split}
    P_{V_+V_+}^V(z) &= P_{V_-V_-}^V(z) = \frac{1+z^4}{z\zb_+}~,\\
    P_{V_+V_-}^V(z) &= P_{V_-V_+}^V(z) =\frac{\zb^3}{z}~.\\
\end{split}
\ee
%
Since QED and QCD are vectorlike theories, we also define the splitting functions properly summed over the vector polarizations and fermion helicities:
%
\be\begin{split}
    P_{Vf}^f(z) &\equiv \frac{P_{V_+f_L}^{f}(z)+P_{V_+f_R}^{f}(z)+P_{V_-f_L}^{f}(z)+P_{V_-f_R}^{f}(z)}{2}= \frac{1+\zb^2}{z}~,\\
    P_{fV}^f(z) &\equiv \frac{P_{f_LV_+}^{f}(z)+P_{f_RV_+}^{f}(z)+P_{f_LV_-}^{f}(z)+P_{f_RV_-}^{f}(z)}{2} = z^2 + \zb^2~,\\
    P_{VV}^V(z) &\equiv \frac{P_{V_+V_+}^V(z)+P_{V_+V_-}^V(z)+P_{V_-V_+}^V(z)+P_{V_-V_-}^V(z)}{2} = 2\frac{(1-z\zb)^2}{z\zb_+}~.
\end{split}\ee
%
%
Finally, we report here the integrals appearing in Eq.~\eqref{eq:appr_QED_sol}:
\be\begin{split}
	I_{fVVf}(x) &= \int_x^1 \frac{dz}{z} P_{fV}^f(z) P_{Vf}^f\left(\frac{x}{z}\right) = \frac{4+3x-3x^2-4x^3}{3x}+2(1+x) \log x~,\\
	I_{Vfff}(x) &= \int_x^1 \frac{dz}{z} P_{Vf}^f\left(\frac{x}{z}\right) P_{ff}^V(z) = \\
	&= 2\log(1-x) P_{Vf}^f(x)+\frac{(1-x)(2x-3)}{x}+(2-x) \log x~,\\
	I_{ffff}(x) &= \int_x^1 \frac{dz}{z} P_{ff}^V\left(\frac{x}{z}\right) P_{ff}^V(z) = \\
	&= \frac{-2(1-x)^2+4(1+x^2)\log(1-x)-(1+3x^2)\log x}{1-x}~.
    \label{eq:appr_QED_integrals}
\end{split}\ee

%-------------------------------------
\subsection{Ultra-collinear splitting functions}

 The top quark is explicitly written, while for other fermions we write $f$. $s=L,R$ is the helicity of the fermion, $T=\pm$ is a transverse polarization of the gauge bosons. If inside a splitting we write $f_sf_{-s}$ it means that the two fermions have opposite helicity (same for the gauge bosons). $N_c^f$ is $1$ for leptons and $N_c$ for quarks.\\

\noindent Splitting $f\to f+V_T$ ($f = t,b$):
%
\be\begin{split}
    U_{\tr\bl}^{\wm^-}(z)  &= U_{\trb\blb}^{\Wp^+}(z)  = \frac{1}{2}g_2^2y_t^2\zb ~,\\
    U_{\wm^-\bl}^{\tr}(z)  &= U_{\Wp^+\blb}^{\trb}(z)  = \frac{1}{2}g_2^2y_t^2z ~,\\
    U_{\bl\tr}^{\Wp^+}(z)  &= U_{\blb\trb}^{\wm^-}(z)  = \frac{1}{2}g_2^2y_t^2\zb z^2~,\\
    U_{\Wp^+\tr}^{\bl}(z)  &= U_{\wm^-\trb}^{\blb}(z)  = \frac{1}{2}g_2^2y_t^2z \zb^2 ~,
\end{split}\ee
\be\begin{split}
    U_{tt}^{g}(z)&\equiv U_{\tr\tl}^{g_-}(z)  = U_{\trb\tlb}^{g_+}(z)  = U_{\tl\tr}^{g_+}(z)  = U_{\tlb\trb}^{g_-}(z)  = C_Fg_3^2y_t^2\zb^3 ~,\\
    U_{g t}^{t}(z)&\equiv U_{g_-\tl}^{\tr}(z)  = U_{g_+\tlb}^{\trb}(z)  = U_{g_+\tr}^{\tl}(z)  = U_{g_-\trb}^{,\tlb}(z)  = C_Fg_3^2y_t^2z^3 ~,\\
    U_{tt}^{\g}(z)&\equiv U_{\tr\tl}^{\gm}(z)  = U_{\trb\tlb}^{,\gp}(z)  = U_{\tl\tr}^{\gp}(z)  = U_{\tlb\trb}^{\gm}(z)  = Q_u^2e^2y_t^2\zb^3 ~,\\
    U_{\g t}^{t}(z)&\equiv U_{\gm\tl}^{\tr}(z)  = U_{\gp\tlb}^{\trb}(z)  = U_{\gp\tr}^{\tl}(z)  = U_{\gm\trb}^{\tlb}(z)  = Q_u^2e^2y_t^2z^3 ~,
\end{split}\ee
\be\begin{split}
    U_{\tr\tl}^{\zm}(z)  &= U_{\trb\tlb}^{\zp}(z)  = \frac{g_2^2y_t^2}{c_W^2}\zb\left(\frac{1}{2}-Q_us_W^2\zb\right)^2 ~,\\
    U_{\zm\tl}^{\tr}(z)  &= U_{\zp\tlb}^{\trb}(z)  = \frac{g_2^2y_t^2}{c_W^2}z\left(\frac{1}{2}-Q_us_W^2z\right)^2 ~,\\
    U_{\tl\tr}^{\zp}(z)  &= U_{\tlb\trb}^{\zm}(z)  = \frac{g_2^2y_t^2}{c_W^2}\zb\left(\frac{z}{2}+Q_us_W^2\zb\right)^2 ~,\\
    U_{\zp\tr}^{\tl}(z)  &= U_{\zm\trb}^{\tlb}(z)  = \frac{g_2^2y_t^2}{c_W^2}z\left(\frac{\zb}{2}+Q_us_W^2z\right)^2 ~,\\
    U_{\zgm\tl}^{\tr}(z)  &= U_{\zgp\tlb}^{\trb}(z)  = 2Q_u\frac{eg_2}{c_W}y_t^2z^2\left(\frac{1}{2}-Q_us_W^2z\right) ~,\\
    U_{\zgp\tr}^{\tl}(z)  &= U_{\zgm\trb}^{\tlb}(z)  = -2Q_u\frac{eg_2}{c_W}y_t^2z^2\left(\frac{\zb}{2}+Q_us_W^2z\right) ~.\\
\end{split}
\ee
%
Splitting $V_T\to f+\bar{f}$ ($f = t,b$):
%
\be\begin{split}
    U_{\bl\wm^-}^{\trb}(z)  &= U_{\blb\Wp^+}^{\tr}(z)  = \frac{N_c}{2}g_2^2y_t^2z^2 ~,\\
    U_{\trb\wm^-}^{\bl}(z)  &= U_{\tr\Wp^+}^{\blb}(z)  = \frac{N_c}{2}g_2^2y_t^2\zb^2 ~,\\
\end{split}
\ee
\be\begin{split}
    U_{tg}^{t}(z)&\equiv U_{\tl g_-}^{\trb}(z)  = U_{\trb g_-}^{\tl}(z)  = U_{\tr g_+}^{\tlb}(z)  = U_{\tlb g_+}^{\tr}(z)  = T_Fg_3^2y_t^2 ~,\\
    U_{t\g}^{t}(z)&\equiv U_{\tl\gm}^{\trb}(z)  = U_{\trb\gm}^{\tl}(z)  = U_{\tr\gp}^{\tlb}(z)  = U_{\tlb\gp}^{\tr}(z)  = N_c Q_u^2e^2y_t^2 ~,\\
    \end{split}
\ee
\be\begin{split}
    U_{\tl\zm}^{\trb}(z)  &= U_{\tlb\zp}^{\tr}(z)  = N_c\frac{g_2^2y_t^2}{c_W^2}\left(\frac{z}{2}-Q_us_W^2\right)^2 ~,\\
    U_{\trb\zm}^{\tl}(z)  &= U_{\tr\zp}^{\tlb}(z)  = N_c\frac{g_2^2y_t^2}{c_W^2}\left(\frac{\zb}{2}-Q_us_W^2\right)^2 ~,\\
    U_{\tl\zgm}^{\trb}(z)  &= U_{\tlb\zgp}^{\tr}(z)  = N_cQ_ue\frac{g_2}{c_W}y_t^2\left(\frac{z}{2}-Q_us_W^2\right) ~,\\
    U_{\trb\zgm}^{\tl}(z)  &= U_{\tr\zgp}^{\tlb}(z)  = N_cQ_ue\frac{g_2}{c_W}y_t^2\left(\frac{\zb}{2}-Q_us_W^2\right) ~.\\
\end{split}\ee
%
Splitting $f\to f + V_L$:
%
\be\begin{split}
    U_{f_Lf_L}^{\zl}(z) &= U_{\fbar_L\fbar_L}^{\zl}(z)  = \left(T_3 y_f^2\zb^2+\frac{g_2^2}{c_W^2}Q^Z_{f_L}z\right)^2\frac{1}{\zb_+} ~,\\
    U_{Z_Lf_L}^{\fl}(z) &= U_{Z_L\fbar_L}^{\flb}(z) = \left(T_3 y_f^2z^2+\frac{g_2^2}{c_W^2}Q^Z_{f_L}\zb\right)^2\frac{1}{z} ~,\\
    U_{f_Rf_R}^{\zl}(z) &= U_{\fbar_R\fbar_R}^{\zl}(z)  = \left(T_3 y_f^2\zb^2-\frac{g_2^2}{c_W^2}Q^Z_{f_R}z\right)^2\frac{1}{\zb_+} ~,\\
    U_{Z_Lf_R}^{\fr}(z) &= U_{Z_L\fbar_R}^{\frb}(z) = \left(T_3 y_f^2z^2-\frac{g_2^2}{c_W^2}Q^Z_{f_R}\zb\right)^2\frac{1}{z} ~,\\
    U_{f^{(2)}_Lf^{(1)}_L}^{\wl}(z) &= U_{\fbar^{(2)}_L\fbar^{(1)}_L}^{\wl}(z)  = \left(y_{f_1}^2z\zb-y_{f_2}^2\zb-g_2^2z\right)^2\frac{1}{2\zb_+} ~,\\
    U_{W_Lf^{(1)}_L}^{f^{(2)}_L}(z) &= U_{W_L\fbar^{(1)}_L}^{\fbar^{(2)}_L}(z) = \left(y_{f_1}^2z\zb-y_{f_2}^2z-g_2^2\zb\right)^2\frac{1}{2z} ~.\\
\end{split}
\ee
%
Splitting $V_L\to f+\bar{f}$:
%
\be\begin{split}
    U_{f_LZ_L}^{\flb}(z) &= U_{\fbar_LZ_L}^{\fl}(z)  = N_c^f\left(T_3 y_f^2-\frac{g_2^2}{c_W^2}Q^Z_{f_L}z\zb\right)^2 ~,\\
    U_{f_RZ_L}^{\frb}(z) &= U_{\fbar_RZ_L}^{\fr}(z)  = N_c^f\left(T_3 y_f^2-\frac{g_2^2}{c_W^2}Q^Z_{f_R}z\zb\right)^2 ~,\\
    U_{f^{(1)}_LW_L}^{\fbar^{(2)}_L}(z) &= U_{\fbar^{(1)}_LW_L}^{f^{(2)}_L}(z)  = \frac{N_c^f}{2}\left(y_{f_1}^2\zb+y_{f_2}^2z-g_2^2z\zb\right)^2 ~.\\
\end{split}
\ee
%
Splitting $t\to t+h$:
%
\be\begin{split}
    U_{tt}^{h}(z)&\equiv U_{\tl\tl}^{h}(z)  = U_{\tr\tr}^{h}(z)  = U_{\trb\trb}^{h}(z)  = U_{\tlb\tlb}^{h}(z)  = \frac{y_t^4}{4}\zb(1+z)^2 ~,\\
    U_{ht}^{t}(z)&\equiv U_{h\tl}^{\tl}(z)  = U_{h\tr}^{\tr}(z)  = U_{h\trb}^{\trb}(z)  = U_{h\tlb}^{\tlb}(z)  = \frac{y_t^4}{4}z(1+\zb)^2 ~.\\
\end{split}
\ee
%
Splitting $h\to t+\bar{t}$:
%
\be
    U_{th}^{t}(z)\equiv  U_{\tl h}^{\tlb}(z)  = U_{\tr h}^{\trb}(z)  = U_{\trb h}^{\tr}(z)  = U_{\tlb h}^{\tl}(z)  = N_c\frac{y_t^4}{4}(\zb-z)^2.
\ee
%
Splitting $V_T\to V_L+V_T$:
%
\be\begin{split}
    U_{\wl\wt}^{\gt}(z)  &= e^2g_2^2\frac{\zb^3}{z} ~,\\
    U_{\gt\wt}^{\wl}(z)  &= e^2g_2^2\frac{z^3}{\zb_+} ~,\\
    U_{\wl\wt}^{\zt}(z)  &= \frac{1}{4}c_W^2g_2^4(1+\zb+t_W^2z)^2\frac{\zb}{z} ~,\\
    U_{\zt \wt}^{\wl}(z)  &= \frac{1}{4}c_W^2g_2^4(1+z+t_W^2\zb)^2\frac{z}{\zb_+}~,\\
    U_{\zgt \wt}^{\wl}(z)  &= c_Weg_2^3(1+z+t_W^2\zb)\frac{z^2}{\zb_+}~,\\
    U_{\zl\wt}^{\wt}(z)  &= \frac{1}{4}g_2^4(1+\zb)^2\frac{\zb}{z} ~,\\
    U_{\wt \wt}^{\zl}(z)  &= \frac{1}{4}g_2^4(1+z)^2\frac{z}{\zb_+}~,\\
    U_{\wl\gt}^{\wt}(z)  &= e^2g_2^2\frac{\zb}{z} ~,\\
    U_{\wt\gt}^{\wl}(z)  &= e^2g_2^2\frac{z}{\zb_+} ~,\\
    U_{\wl \zt}^{\wt}(z)  &= \frac{1}{4}c_W^2g_2^4(1+\zb-t_W^2z)^2\frac{\zb}{z}~,\\
    U_{\wt \zt}^{\wl}(z)  &= \frac{1}{4}c_W^2g_2^4(1+z-t_W^2\zb)^2\frac{z}{\zb_+}~,\\
    U_{\wl \zgt}^{\wt}(z)  &= \frac{1}{2}c_Weg_2^3(1+\zb-t_W^2z)\frac{\zb}{z}~,\\
    U_{\wt \zgt}^{\wl}(z)  &= \frac{1}{2}c_Weg_2^3(1+z-t_W^2\zb)\frac{z}{\zb_+}~.\\
\end{split}
\ee
%
Splitting $V_L\to V_T+V_{-T}$:

\be\begin{split}
    U_{\gt \wl}^{\wtm}(z)  &= e^2g_2^2z^3\zb~,\\
    U_{\wt \wl}^{\gtm}(z)  &= e^2g_2^2z\zb^3~,\\
    U_{\zt \wl}^{\wtm}(z)  &= \frac{1}{4}c_W^2g_2^4z\zb(\zb -z+t_W^2)^2~,\\
    U_{\wt \wl}^{\ztm}(z)  &= \frac{1}{4}c_W^2g_2^4z\zb(z -\zb+t_W^2)^2~,\\
    U_{\zgt \wl}^{\wtm}(z)  &= -c_Weg_2^3z^2\zb(\zb -z+t_W^2) ~,\\
    U_{\wt \zl}^{\wtm}(z)  &= \frac{1}{4}g_2^4z\zb(\zb -z)^2~.\\
\end{split}
\ee
%
Splitting $V_T\to h+V_T$:
%
\be\begin{split}
    U_{h\wt}^{\wt}(z) &= U_{\wt\wt}^{h}(z) = \frac{1}{4}g_2^4z\zb~,\\
    U_{h\zt}^{\zt}(z) &= U_{\zt\zt}^{h}(z) = \frac{1}{4}\frac{g_2^4}{c_W^4}z\zb~.\\
\end{split}
\ee
%
Splitting $h\to V_T+V_{-T}$:
%
\be\begin{split}
    U_{\wt h}^{\wtm}(z)  &= \frac{1}{4}g_2^4z\zb~,\\
    U_{\zt h}^{\ztm}(z)  &= \frac{1}{8}\frac{g_2^4}{c_W^4}z\zb~.\\
\end{split}
\ee
%
Splitting $V_L\to V_L+V_L$:
%
\be\begin{split}
    U_{\zl\wl}^{\wl}(z) &= \frac{1}{16}g_2^4[(\zb-z)(2+z\zb)-t_W^2\zb(1+\zb)]^2\frac{1}{z\zb_+}~,\\
    U_{\wl\wl}^{\zl}(z) &= \frac{1}{16}g_2^4[(z-\zb)(2+z\zb)-t_W^2z(1+z)]^2\frac{1}{z\zb_+}~,\\
    U_{\wl\zl}^{\wl}(z) &= \frac{1}{16}g_2^4(z-\zb)^2(2+z\zb-t_W^2z\zb)^2\frac{1}{z\zb_+}~.\\
\end{split}
\ee
%
Splitting $h\to V_L+V_L$:
%
\be\begin{split}
    U_{\zl h}^{\zl}(z) &= \frac{1}{8}\left[\frac{g_2^2}{c_W^2}(1-z\zb)-4\lambda_hz\zb\right]^2\frac{1}{z\zb_+}~,\\
    U_{\wl h}^{\wl}(z) &= \frac{1}{4}[g_2^2(1-z\zb)-4\lambda_hz\zb]^2\frac{1}{z\zb_+}~.\\
\end{split}
\ee
%
Splitting $V_L\to h+V_L$:
%
\be\begin{split}
    U_{h \zl}^{\zl}(z) &= \frac{1}{4}\left[\frac{g_2^2}{c_W^2}(1-z\zb)+4\lambda_h\zb\right]^2\frac{z}{\zb_+}~,\\
    U_{\zl \zl}^{h}(z) &= \frac{1}{4}\left[\frac{g_2^2}{c_W^2}(1-z\zb)+4\lambda_hz\right]^2\frac{\zb}{z}~,\\
    U_{h\wl}^{\wl}(z) &= \frac{1}{4}[g_2^2(1-z\zb)+4\lambda_h\zb]^2\frac{z}{\zb_+}~,\\
    U_{\wl\wl}^{h}(z) &= \frac{1}{4}[g_2^2(1-z\zb)+4\lambda_hz]^2\frac{\zb}{z}~.\\
\end{split}
\ee
%
Splitting $h\to h+h$:
%
\be
U_{h h}^{h}(z) = 18\lambda_h^2z\zb~.
\ee
%
Splitting involving the mixed state $hZ_L$:
%
\be\begin{split}
     U_{hZ_L\tl}^{\tl}(z) &= -U_{hZ_L\tlb}^{\tlb}(z) =y_t^2(1+\zb)\left(\frac{y_t^2}{2}z^2+g_Z^2 Q^Z_{\tl}\zb\right) ~,\\
     U_{hZ_L\tr}^{\tr}(z) &= -U_{hZ_L\trb}^{\trb}(z) =-y_t^2(1+\zb)\left(\frac{y_t^2}{2}z^2-g_Z^2Q^Z_{\tr}\zb\right) ~,\\
     U_{\tl hZ_L}^{\tlb}(z) &= U_{\tlb hZ_L}^{\tl}(z) =-\frac{y_t^2}{2}(\zb-z)\left(\frac{y_t^2}{2}-g_Z^2Q^Z_{\tl}z\zb\right) ~,\\
     U_{\tr hZ_L}^{\trb}(z) &= U_{\trb hZ_L}^{\tr}(z) =\frac{y_t^2}{2}(\zb-z)\left(\frac{y_t^2}{2}-g_Z^2Q^Z_{\tr}z\zb\right) ~,\\
     \end{split}
\ee
    \be\begin{split}
    U_{hZ_L\wl}^{\wl}(z) &\equiv U_{hZ_L\wl^+}^{\wl^+}(z) = -U_{hZ_L\wl^-}^{\wl^-}(z)\\
    &=\frac{g_2^2}{4}[g_2^2(1-z\zb)+4\lambda_h\zb][(\zb -z)(2+z\zb)-t_W^2\zb(1-\zb)]\frac{1}{\zb_+}~,\\
    U_{\wl hZ_L}^{\wl}(z) &\equiv U_{\wl^+ hZ_L}^{\wl^-}(z) = -U_{\wl^- hZ_L}^{\wl^+}(z) \\
    &= \frac{g_2^2}{8}[g_2^2(1-z\zb)-4\lambda_h z\zb](\zb-z)[(2+(1-t_W^2)z\zb]\frac{1}{z\zb_+}~,\\
    \end{split}
\ee
    \be\begin{split}
    U_{hZ_L\wt}^{\wt}(z) &\equiv U_{hZ_L\wt^+}^{\wt^+}(z) = U_{hZ_L\wt^-}^{\wt^-}(z)= \frac{g_2^4}{2}\zb(1+\zb)~,\\
    U_{\wt hZ_L}^{\wt}(z) &\equiv U_{\wt^+ hZ_L}^{\wt^-}(z) = -U_{\wt^- hZ_L}^{\wt^+}(z)= -\frac{g_2^4}{4}z\zb(\zb-z)~.\\
\end{split}
\ee
%
