
Let $G_{sc} = \Sp(V)$ be simply connected and simple of type $C_{\ell}$. In this section, we will describe the Jordan block sizes of unipotent elements $u \in G_{sc}$ acting on $\g_{ad}$. Our approach is to describe the Jordan block sizes of $u$ on $\g_{ad}$ in terms of the Jordan block sizes on $[\g_{ad}, \g_{ad}]$, using Lemma \ref{jordanrestrictionNIL}. Since the Jordan block sizes of $u$ on $[\g_{ad}, \g_{ad}] \cong \g_{sc}/Z(\g_{sc})$ (Lemma \ref{lemma:gmodZisgadgad}) are known by the results of Section \ref{section:unipgmodZ}, we then get an explicit description of the Jordan block sizes of $u$ on $\g_{ad}$.

Throughout this section we will consider $\g_{ad}$ as constructed in Section \ref{subsection:chevalleyC} -- \ref{subsection:symsquareC}, and we use the notation established there.

\begin{lemma}\label{lemma:deltaWLunip}
Let $u \in \Sp(V)$ be the reduction modulo $p$ of $u_{\Z} = x_{\Z}^{(\alpha_1)} \cdots x_{\Z}^{(\alpha_{\ell-1})}$ as in Section \ref{subsection:unipotentroots}, so that $V \downarrow K[u] = W(\ell)$. Then the following hold:
	\begin{enumerate}[\normalfont (i)]
		\item $(u_{\Z} - 1) \cdot \delta = 0$.
		\item There exists $v \in L_{sc}$ such that $(u_{\Z} - 1) \cdot (\delta + v) \equiv 2 \delta \mod{2 L_{sc}}$ if and only if $\ell$ is even.
	\end{enumerate}
\end{lemma}

\begin{proof}
For claim (i), consider $X_{\alpha_i} = E_{i,i+1} - E_{n-i,n-i+1}$ for $1 \leq i \leq \ell-1$ from the Chevalley basis of $\mathfrak{sp}(V_{\C})$. It is clear that $X_{\alpha_i} \cdot \delta = 0$, so $x_{\Z}^{(\alpha_i)} \cdot \delta = \delta$ for all $1 \leq i \leq \ell-1$, from which (i) follows.

For (ii), we have $(u_{\Z} - 1) \cdot (\delta + v) = (u_{\Z} - 1) \cdot v$ for all $v \in L_{sc}$ by (i). By Lemma \ref{lemma:imZforUZ}, there exists $v \in L_{sc}$ such that $(u_{\Z} - 1) \cdot (v) \equiv 2 \delta \mod{2 L_{sc}}$ if and only if $\operatorname{Im}(\widehat{u} - 1) \supseteq Z(\g_{sc})$, where $\widehat{u}$ is the action of $u$ on $\g_{sc}$. It follows from Proposition \ref{prop:unipKeraction} and Lemma \ref{jordanquotientNIL} that $\operatorname{Im}(\widehat{u} - 1) \supseteq Z(\g_{sc})$ if and only if $\ell$ is even, so we conclude that (ii) holds.\end{proof}

\begin{lemma}\label{lemma:deltaV2Lunip}
Assume that $\ell$ is odd. Let $u \in \Sp(V)$ be the reduction modulo $p$ of $u_{\Z} = x_{\Z}^{(\alpha_1)} \cdots x_{\Z}^{(\alpha_{\ell})}$ as in Section \ref{subsection:unipotentroots}, so that $V \downarrow K[u] = V(2\ell)$. Then the following hold:

	\begin{enumerate}[\normalfont (i)]
		\item There exists $v \in L_{sc}$ such that $(u_{\Z} - 1) \cdot (\delta + v) \equiv 2 \delta \mod{2 L_{sc}}$.
		\item There does not exist $v \in L_{sc}$ such that $(u_{\Z} - 1) \cdot (\delta + v) \equiv 0 \mod{2 L_{sc}}$.
	\end{enumerate}

\end{lemma}

\begin{proof}
For (i), first we calculate \begin{align*} u_{\Z} \cdot \delta &= x_{\Z}^{(\alpha_1)} \cdots x_{\Z}^{(\alpha_{\ell-1})} \cdot ( \delta + \frac{1}{2} v_{\ell}^2 ) & (\text{by } x_{\Z}^{(\alpha_{\ell})} \cdot \delta = \delta + \frac{1}{2} v_{\ell}^2) \\ &= \delta + \frac{1}{2} \left(v_1 + \cdots + v_{\ell} \right)^2 & (\text{by Lemma \ref{lemma:deltaWLunip} (i)}) \\ &= \delta + \sum_{1 \leq i \leq \ell} \frac{1}{2} v_i^2 + \sum_{1 \leq i < j \leq \ell} v_iv_j.\end{align*}

Furthermore $$u_{\Z} \cdot \frac{1}{2} v_{\ell+1}^2 = \frac{1}{2} \left(v_1 + \cdots + v_{\ell+1} \right)^2 = \sum_{1 \leq i \leq \ell+1} \frac{1}{2}v_i^2 + \sum_{1 \leq i < j \leq \ell+1} v_iv_j,$$ so \begin{equation}\label{eq:firsteqV2ldelta}u_{\Z} \cdot \left(\delta + \frac{1}{2} v_{\ell+1}^2\right) \equiv \delta + \frac{1}{2} v_{\ell+1}^2 + \sum_{1 \leq i \leq \ell} v_iv_{\ell+1} \mod{2L_{sc}}.\end{equation} Next define $$\gamma := \sum_{1 \leq j \leq (\ell-1)/2} v_{2j}\left(v_{n-2j+1} + v_{n-2j+2}\right).$$ For $1 \leq j \leq (\ell-1)/2$, we denote $s_j := \sum_{1 \leq t \leq 2j} v_t v_{n-2j}$. Then modulo $2L_{sc}$, we have \begin{align*} u_{\Z} \cdot \gamma &\equiv \sum_{1 \leq j \leq (\ell-1)/2} \left( \sum_{1 \leq t \leq 2j} v_t \right) \left(v_{n-2j+2} + v_{n-2j} \right) \\ &\equiv \sum_{1 \leq j \leq (\ell-1)/2}\left( s_j + s_{j-1} + v_{2j-1}v_{n-2j+2} + v_{2j}v_{n-2j+2} \right) \\ &\equiv s_{(\ell-1)/2} + \sum_{1 \leq j \leq (\ell-1)/2} v_{2j-1} v_{n-2j+2} + \sum_{1 \leq j \leq (\ell-1)/2} v_{2j} v_{n-2j+2} \\ &\equiv s_{(\ell-1)/2} + \sum_{1 \leq j \leq (\ell-1)/2} v_{2j-1} v_{n-2j+2} + \left( \gamma + \sum_{1 \leq j \leq (\ell-1)/2} v_{2j} v_{n-2j+1} \right) \\ &\equiv \gamma + s_{(\ell-1)/2} + \sum_{1 \leq j \leq \ell-1} v_j v_{n-j+1} \\ &\equiv \gamma + s_{(\ell-1)/2} + \left(2\delta + v_{\ell}v_{\ell+1} \right) \\ &\equiv \gamma + 2 \delta + \sum_{1 \leq j \leq \ell} v_jv_{\ell+1}.\end{align*} Combining this with~\eqref{eq:firsteqV2ldelta}, we get $$u_{\Z} \cdot \left(\delta + \frac{1}{2} v_{\ell+1}^2 + \gamma\right) \equiv \delta + \frac{1}{2} v_{\ell+1}^2 + \gamma + 2 \delta \mod{2L_{sc}}.$$ We conclude then that (i) holds, with $v = \frac{1}{2} v_{\ell+1}^2 + \gamma$.

For claim (ii), suppose for the sake of contradiction that there exists $v \in L_{sc}$ such that $(u_{\Z} - 1) \cdot (\delta + v) \equiv 0 \mod{2 L_{sc}}$. Then it follows from (i) that there exists $w \in L_{sc}$ such that $(u_{\Z} - 1) \cdot w \equiv 2 \delta \mod{2 L_{sc}}$. By Lemma \ref{lemma:imZforUZ}, we have $\operatorname{Im}(\widehat{u} - 1) \supseteq Z(\g_{sc})$, where $\widehat{u}$ is the action of $u$ on $\g_{sc}$. On the other hand $\operatorname{Im}(\widehat{u} - 1) \not\supseteq Z(\g_{sc})$ by Proposition \ref{prop:unipKeraction} and Lemma \ref{jordanquotientNIL}, so we have a contradiction.\end{proof}




\begin{lemma}\label{lemma:GADoddsumofWs}
Let $u \in \Sp(V)$ be unipotent such that $V \downarrow K[u] = \sum_{1 \leq i \leq t} W(\ell_i)$, where $\ell_i \geq 1$ for all $1 \leq i \leq t$. Then $\Ker(\widetilde{u}-1) \not\subseteq [\g_{ad},\g_{ad}]$.
\end{lemma}

\begin{proof}
Follows from Lemma \ref{lemma:GADreduce} (i) and Lemma \ref{lemma:deltaWLunip} (i).
\end{proof}

\begin{lemma}\label{lemma:GADoddsumofVsandWs}
Let $u \in \Sp(V)$ be unipotent such that $V \downarrow K[u] = \sum_{1 \leq i \leq t} W(m_i) \perp \sum_{1 \leq j \leq s} V(2k_j)$, where $k_j \geq 1$ is odd for all $1 \leq j \leq s$. Assume that $s > 0$. 

Denote the action of $u$ on $\g_{ad}$ by $\widetilde{u}$. Then $\Ker(\widetilde{u}-1) \not\subseteq [\g_{ad},\g_{ad}]$ if and only if $m_i$ is even for all $1 \leq i \leq t$.
\end{lemma}

\begin{proof}
In view of Lemma \ref{lemma:deltaV2Lunip} (ii) and Lemma \ref{lemma:GADreduce} (i), we have $\Ker(\widetilde{u}-1) \not\subseteq [\g_{ad},\g_{ad}]$ if and only if Lemma \ref{lemma:GADreduce} (i)(b) holds. Then by Lemma \ref{lemma:deltaWLunip} (ii), we conclude that $\Ker(\widetilde{u}-1) \not\subseteq [\g_{ad},\g_{ad}]$ if and only if $m_i$ is even for all $1 \leq i \leq t$.\end{proof}

\begin{lemma}\label{lemma:GADindecompV2l}
Let $u \in \Sp(V)$ be unipotent such that $V \downarrow K[u] = V(2\ell)$. Let $\widetilde{u}$ be the action of $u$ on $\g_{ad}$, and denote $\alpha = \nu_2(\ell)$. Then the following hold:
	\begin{enumerate}[\normalfont (i)]
		\item $\Ker(\widetilde{u}-1)^{2^{\alpha}-1} \subseteq [\g_{ad}, \g_{ad}]$.
		\item $\Ker(\widetilde{u}-1)^{2^{\alpha}} \not\subseteq [\g_{ad}, \g_{ad}]$.
	\end{enumerate}
\end{lemma}

\begin{proof}We begin with the proof of (i), which is trivially true when $\alpha = 0$, so suppose that $\alpha > 0$.

We first consider $\alpha = 1$, in which case $\ell \equiv 2 \mod{4}$. Then \begin{align*} \dim \g_{ad}^u &\leq \dim \g_{sc}^u &&\text{by Lemma \ref{lemma:regularl2mod4ineq}} \\ &= \dim [\g_{ad},\g_{ad}]^u &&\text{by Lemma \ref{lemma:gmodZisgadgad} and Proposition \ref{prop:unipKeraction} } \\ &\leq \dim \g_{ad}^u. &&\end{align*} Thus we conclude that $\dim \g_{ad}^u = \dim \g_{sc}^u = \dim [\g_{ad},\g_{ad}]^u.$ It follows then from Lemma \ref{jordanrestrictionNIL} that $\Ker(\widetilde{u}-1) \subseteq [\g_{ad}, \g_{ad}]$, as claimed by (i).

Suppose then that $\alpha > 1$. We have $V \downarrow K[u^{2^{\alpha-1}}] = V(\ell/2^{\alpha-2})^{2^{\alpha-1}}$ by \cite[Lemma 6.13]{Korhonen2020Hesselink}. It follows then from Lemma \ref{lemma:GADreduce} (ii) and the case $\alpha = 1$ that $$\Ker(\widetilde{u}-1)^{2^{\alpha-1}} = \Ker(\widetilde{u}^{2^{\alpha-1}} - 1) \subseteq [\g_{ad}, \g_{ad}].$$ In particular, we have \begin{equation}\label{eq:kerisin}\Ker(\widetilde{u}-1) \subseteq [\g_{ad}, \g_{ad}].\end{equation} Next we note that it follows from Lemma \ref{lemma:gmodZisgadgad}, Proposition \ref{prop:unipKeraction}, and Lemma \ref{lemma:smallesblockunipS2} that the smallest Jordan block size of $u$ on $[\g_{ad}, \g_{ad}]$ is equal to $2^{\alpha}-1$. In particular, there are no Jordan blocks of size $1 \leq d < 2^{\alpha}-1$ for $u$ on $[\g_{ad}, \g_{ad}]$, which combined with Lemma \ref{jordanrestrictionNIL} and~\eqref{eq:kerisin} implies $\Ker(\widetilde{u}-1)^{2^{\alpha}-1} \subseteq [\g_{ad}, \g_{ad}]$.

For (ii), note that $V \downarrow K[u^{2^{\alpha}}] = V(\ell/2^{\alpha-1})^{2^{\alpha}}$ by \cite[Lemma 6.13]{Korhonen2020Hesselink}. Thus it follows from Lemma \ref{lemma:GADoddsumofVsandWs} that $\Ker(\widetilde{u}-1)^{2^{\alpha}} = \Ker(\widetilde{u}^{2^{\alpha}} - 1) \not\subseteq [\g_{ad}, \g_{ad}]$.\end{proof}


\begin{prop}\label{prop:unipgadaction}
Let $u \in \Sp(V)$ be unipotent, with orthogonal decomposition $V \downarrow K[u] = \sum_{1 \leq i \leq t} W(m_i) \perp \sum_{1 \leq j \leq s} V(2k_j)$. Assume that $s > 0$, and let $\alpha = \max_{1 \leq j \leq s} \nu_2(k_j)$. Let $\widetilde{u}$ be the action of $u$ on $\g_{ad}$. Then the following statements hold:

	\begin{enumerate}[\normalfont (i)]
		\item $\Ker(\widetilde{u} - 1)^{2^{\alpha}-1} \subseteq [\g_{ad}, \g_{ad}]$. 
		\item $\Ker(\widetilde{u} - 1)^{2^{\alpha}} \not\subseteq [\g_{ad}, \g_{ad}]$ if and only if $\alpha = \nu_2(k_j)$ for all $1 \leq j \leq s$, and $\nu_2(m_i) > \alpha$ for all $1 \leq i \leq t$.
		\item $\Ker(\widetilde{u} - 1)^{2^{\alpha}+1} \not\subseteq [\g_{ad}, \g_{ad}]$. 

	\end{enumerate}
\end{prop}

\begin{proof}
Claim (i) follows from Lemma \ref{lemma:GADreduce} and Lemma \ref{lemma:GADindecompV2l}.

Next we will prove (ii). In the case where $\alpha = 0$ we have $k_j$ odd for all $1 \leq j \leq s$. Then the claim of (ii) is that $\Ker(\widetilde{u} - 1) \not\subseteq [\g_{ad}, \g_{ad}]$ if and only if $m_i$ is even for all $1 \leq i \leq t$, which is precisely Lemma \ref{lemma:GADoddsumofVsandWs}.

Suppose then that $\alpha > 0$. Write $m_i = m_i' 2^{\alpha} + m_i''$ with $0 \leq m_i'' < 2^{\alpha}$ and $k_j = k_j' 2^{\alpha-1} + k_j''$ with $0 \leq k_j'' < 2^{\alpha-1}$. Then for the restrictions of the summands in $V \downarrow K[u^{2^{\alpha}}]$, we have \begin{align*}W(m_i) \downarrow K[u^{2^{\alpha}}] &= W(m_i')^{2^{\alpha}-m_i''} \perp W(m_i'+1)^{m_i''} \\ V(2k_j) \downarrow K[u^{2^{\alpha}}] &= \begin{cases} V(k_j/2^{\alpha-1})^{2^{\alpha}}, & \text{ if } \nu_2(k_j) = \alpha. \\ W(k_j')^{2^{\alpha-1}-k_j''} \perp W(k_j'+1)^{k_j''}, & \text{ if } \nu_2(k_j) < \alpha. \end{cases} \end{align*} for all $1 \leq i \leq t$ and $1 \leq j \leq s$, by \cite[Lemma 3.1, Lemma 6.12, Lemma 6.13]{Korhonen2020Hesselink}. In the above we denote $W(0) = 0$.

We have $\alpha = \nu_2(k_j)$ for some $j$, so $V(k_j/2^{\alpha-1})$ appears as a summand of $V \downarrow K[u^{2^{\alpha}}]$. Thus by Lemma \ref{lemma:GADoddsumofVsandWs}, we have $\Ker(\widetilde{u} - 1)^{2^{\alpha}} = \Ker(\widetilde{u}^{2^{\alpha}} - 1) \not\subseteq [\g_{ad}, \g_{ad}]$ if and only if all the summands of the form $W(m)$ in $V \downarrow K[u^{2^{\alpha}}]$ have $m$ even.\\

\noindent \emph{Claim 1: Assume that $\nu_2(m_i) \leq \alpha$ for some $i$. Then $\Ker(\widetilde{u} - 1)^{2^{\alpha}} \subseteq [\g_{ad}, \g_{ad}]$.} \\
\noindent It suffices to show that $W(m_i) \downarrow K[u^{2^{\alpha}}]$ has a summand $W(m)$ with $m$ odd. If $0 < m_i'' < 2^{\alpha}$, then $W(m_i) \downarrow K[u^{2^{\alpha}}]$ has $W(m_i')$ and $W(m_i'+1)$ as a summand. If $m_i'' = 0$, then $W(m_i) \downarrow K[u^{2^{\alpha}}] = W(m_i')^{2^{\alpha}}$ with $m_i'$ odd, since $\nu_2(m_i) \leq \alpha$.\\

\noindent \emph{Claim 2: Assume that $\nu_2(k_j) < \alpha$ for some $j$. Then $\Ker(\widetilde{u} - 1)^{2^{\alpha}} \subseteq [\g_{ad}, \g_{ad}]$.} \\
It suffices to show that $V(2k_j) \downarrow K[u^{2^{\alpha}}]$ has a summand $W(m)$ with $m$ odd. If $0 < k_j'' < 2^{\alpha-1}$, then $V(2k_j) \downarrow K[u^{2^{\alpha}}]$ has $W(k_j')$ and $W(k_j'+1)$ as a summand. Suppose then that $k_j'' = 0$. Then $V(2k_j) \downarrow K[u^{2^{\alpha}}] = W(k_j')^{2^{\alpha-1}}$, with $k_j'$ is odd since $\nu_2(k_j) < \alpha$.\\

The ``only if'' part of (ii) follows from Claim 1 and Claim 2. Conversely, if $\alpha = \nu_2(k_j)$ for all $1 \leq j \leq s$ and $\nu_2(m_i) > \alpha$ for all $1 \leq i \leq t$, we have $$V \downarrow K[u^{2^{\alpha}}] = \sum_{1 \leq i \leq t} W(m_i/2^{\alpha})^{2^{\alpha}} \perp \sum_{1 \leq j \leq s} V(k_j/2^{\alpha-1}).$$ Thus $\Ker(\widetilde{u} - 1)^{2^{\alpha}} = \Ker(\widetilde{u}^{2^{\alpha}} - 1) \not\subseteq [\g_{ad}, \g_{ad}]$ by Lemma \ref{lemma:GADoddsumofVsandWs}.

For (iii), let $u_{\Z} = u_{\Z,1} \cdots u_{\Z,t+s} \in \mathscr{U}_{\Z}$ be as in Section \ref{subsection:unipotentroots}, so that $u$ is the reduction modulo $p$ of the action of $u_{\Z}$ on $V_{\Z}$. Denote $\delta_1$, $\ldots$, $\delta_{t+s}$ as in Section \ref{subsection:unipotentroots}. It follows from Lemma \ref{lemma:GADreduce} (i), Lemma \ref{lemma:deltaWLunip}, and Lemma \ref{lemma:GADindecompV2l} that there exist $w_{i} \in L_{sc}^{(i)}$ such that \begin{align*}(u_{\Z,i}-1)^{2^{\alpha}} \cdot (\delta_i + w_i) &\equiv 0 \mod{2 L_{sc}^{(i)}} & \text{ if } 1 \leq i \leq t, \\ (u_{\Z,i}-1)^{2^{\alpha}} \cdot (\delta_i + w_i) &\equiv 2 \delta_{i} \mod{2 L_{sc}^{(i)}} & \text{ if } t+1 \leq i \leq t+s.\end{align*} Then $$(u_{\Z}-1)^{2^{\alpha}} \cdot (\delta + w_1 + \cdots + w_{t+s}) \equiv 2\delta_{t+1} + \cdots + 2\delta_{t+s} \mod{2L_{sc}}.$$ On the other hand, we have $u_{\Z,i} \cdot \delta_i = \delta_i + z_i$ for some $z_i \in L_{sc}^{(i)}$, as seen in the beginning of the proof of Lemma \ref{lemma:deltaV2Lunip}. Thus $(u_{\Z}-1) \cdot 2\delta_i \equiv 0 \mod{2L_{sc}^{(i)}}$ for all $t+1 \leq i \leq t+s$, and consequently $$(u_{\Z}-1)^{2^{\alpha}+1} \cdot (\delta + w_1 + \cdots + w_{t+s}) \equiv 0 \mod{2L_{sc}}.$$ It follows then from Lemma \ref{lemma:GADreduce} that $\Ker(\widetilde{u} - 1)^{2^{\alpha}+1} \not\subseteq [\g_{ad}, \g_{ad}]$, as claimed by (iii).\end{proof}


\begin{prop}\label{prop:unipGAD}
Let $u \in \Sp(V)$ be unipotent, with orthogonal decomposition $V \downarrow K[u] = \sum_{1 \leq i \leq t} W(m_i) \perp \sum_{1 \leq j \leq s} V(2k_j)$. Then the following statements hold:
	\begin{enumerate}[\normalfont (i)]
		\item Suppose that $s = 0$. Then $$\g_{ad} \cong V_1 \oplus [\g_{ad}, \g_{ad}]$$ as $K[u]$-modules.
		
		\item Suppose that $s > 0$, and let $\alpha = \max_{1 \leq j \leq s} \nu_2(k_j)$. Then:
			\begin{enumerate}[\normalfont (a)]
				\item If $\alpha = \nu_2(k_j)$ for all $1 \leq j \leq s$ and $\nu_2(m_i) > \alpha$ for all $1 \leq i \leq t$, then \begin{align*}
		\g_{ad} &\cong V_{2^{\alpha}} \oplus V' \\
		[\g_{ad},\g_{ad}] &\cong V_{2^{\alpha}-1} \oplus V' \end{align*} for some $K[u]$-module $V'$.
				
				\item If $\alpha > \nu_2(k_j)$ for some $1 \leq j \leq s$, or $\nu_2(m_i) \leq \alpha$ for some $1 \leq i \leq t$, then \begin{align*}
		\g_{ad} &\cong V_{2^{\alpha}+1} \oplus V' \\
		[\g_{ad},\g_{ad}] &\cong V_{2^{\alpha}} \oplus V' \end{align*} for some $K[u]$-module $V'$.
			\end{enumerate}
		
	\end{enumerate}


\end{prop}

\begin{proof}
Claim (i) follows from Lemma \ref{lemma:GADoddsumofWs} and Lemma \ref{jordanrestrictionNIL}. Similarly (ii) follows from Proposition \ref{prop:unipgadaction} and Lemma \ref{jordanrestrictionNIL}.
\end{proof}

