
We can now prove the main results stated in the introduction; all of them are straightforward consequences of the results from previous sections.

\begin{proof}[Proof of Theorem \ref{thm:unipGSCtoGAD}]
By Proposition \ref{prop:unipKeraction}, we have  \begin{equation}\label{eq:mainthmfinaleq}\begin{aligned}
		\g_{sc} &\cong V_{2^{\alpha}} \oplus V' \\
		\g_{sc}/Z(\g_{sc}) &\cong V_{2^{\alpha}-1} \oplus V' \end{aligned}\end{equation} for some $K[u]$-module $V'$.

If $s = 0$, then by Proposition \ref{prop:unipGAD} and Lemma \ref{lemma:gmodZisgadgad} we have $\g_{ad} \cong V_1 \oplus \g_{sc}/Z(\g_{sc}) \cong V_1 \oplus V_{2^{\alpha}-1} \oplus V'$ as $K[u]$-modules. Thus (i) holds.

For (ii), suppose that $s > 0$ and let $\beta = \max_{1 \leq j \leq s} \nu_2(k_j)$. Consider first the case where (ii)(a) holds, so $\nu_2(k_j) = \beta$ for all $1 \leq j \leq s$ and $\nu_2(m_i) > \beta$ for all $1 \leq i \leq t$. Then $\alpha = \beta$, so by Proposition \ref{prop:unipGAD} and Lemma \ref{lemma:gmodZisgadgad} we have \begin{align*}
		\g_{ad} &\cong V_{2^{\alpha}} \oplus V'' \\
		\g_{sc}/Z(\g_{sc}) &\cong V_{2^{\alpha}-1} \oplus V'' \end{align*} for some $K[u]$-module $V''$. We have $V' \cong V''$ by~\eqref{eq:mainthmfinaleq}, so $\g_{ad} \cong \g_{sc}$ as $K[u]$-modules.

We consider then the case where (ii)(b) holds, so either $\nu_2(k_j) < \beta$ for some $1 \leq j \leq s$, or $\nu_2(m_i) \leq \beta$ for some $1 \leq i \leq t$. Then by Proposition \ref{prop:unipGAD} and Lemma \ref{lemma:gmodZisgadgad}, we have \begin{align*}
		\g_{ad} &\cong V_{2^{\beta}+1} \oplus V'' \\
		\g_{sc}/Z(\g_{sc}) &\cong V_{2^{\beta}} \oplus V'' \end{align*} for some $K[u]$-module $V''$. By~\eqref{eq:mainthmfinaleq} we have $V'' \cong V_{2^{\alpha}-1} \oplus V'''$ and $V' \cong V_{2^{\beta}} \oplus V'''$ for some $K[u]$-module $V'''$. Thus \begin{align*}
		\g_{sc} &\cong V_{2^{\alpha}} \oplus V_{2^{\beta}} \oplus V''', \\
		\g_{ad} &\cong V_{2^{\alpha}-1} \oplus V_{2^{\beta}+1} \oplus V''' \end{align*} so claim (ii)(b) holds.\end{proof}

\begin{proof}[Proof of Theorem \ref{thm:nilGSCtoGAD}]
Similarly to Theorem \ref{thm:unipGSCtoGAD}, the result follows from Proposition \ref{prop:nilKeraction}, Lemma \ref{lemma:gmodZisgadgad}, and Proposition \ref{prop:nilgadaction}.
\end{proof}

\begin{proof}[Proof of Corollary \ref{cor:centralizerdimUNIP} and Corollary \ref{cor:centralizerdimNIL}]
Immediate from Theorem \ref{thm:unipGSCtoGAD} and Theorem \ref{thm:nilGSCtoGAD}.
\end{proof}

\begin{proof}[Proof of Corollary \ref{cor:regularcentralizerdim}]
For a regular unipotent $u \in \Sp(V)$ we have $V \downarrow K[u] = V(2\ell)$ \cite[p. 61]{LiebeckSeitzClass}. Then $\dim \g_{sc}^u = \ell+1$ by Lemma \ref{lemma:LieSpS2} and Lemma \ref{lemma:fixpdimsymwedge}. It follows then from Corollary \ref{cor:centralizerdimUNIP} that $\dim \g_{ad}^u = \dim \g_{sc}^u = \ell+1$.

For regular nilpotent $e \in \mathfrak{sp}(V)$ we have similarly $V \downarrow K[e] = V(2\ell)$ \cite[p. 60]{LiebeckSeitzClass}. It follows from Lemma \ref{lemma:LieSpS2} and \cite[Corollary 4.2]{KorhonenSymExt2021} that $\dim \g_{sc}^e = 2\ell$. Then $\dim \g_{ad}^e = \dim \g_{sc}^e = 2\ell$ by Corollary \ref{cor:centralizerdimNIL}, as claimed.
\end{proof}


