\newpage
\newpage
\begin{gather}
    X \sim  N\left(0,\begin{bmatrix}1 & 0 \\0 & 1\end{bmatrix}\right)\quad  X \sim  N\left(0,\begin{bmatrix}1 & c \\c & 1\end{bmatrix}\right)\\
    Y = X_1\cdot X_2 + \epsilon\\
    f_\theta(X) \rightarrow Y  \quad \Ss(f_\theta,X)
\end{gather}

\begin{gather}
    X = (X_1,X_2,X_3)\\
    Y = X_1 \cdot X_2 +  \epsilon\\
    X_3^{ood} = X_3^{te} + 1 
\end{gather}

\begin{gather}
    Y = X_1^2 \cdot X_2\\
    Y^{ood} = X_1 \cdot X_2^2\\
    f_\theta(X,Y)\\
    h_\Upsilon(X,Y^{ood})
\end{gather}