\subsection{Proof of Lemma \ref{lemma:balancedbase}: Controlling $\norm{\tilZt^T \Zt} $}\label{sec:balancedbase}


\begin{proof}[Proof of Lemma \ref{lemma:balancedbase}]
First, we recall that
\begin{align*}
    \Zplus   &= \left( \I -\mu M_t) \right) \Zt, \\
    \tilZplus&=\left( \I +\mu M_t \right) \tilZt,
\end{align*}
where
\begin{equation*}
    M_t= \Zt\ZtT - \tilZt\tilZtT - \symA +\Deltat.
\end{equation*}
We calculate that 
\begin{align*}
    \tilZplusT \Zplus
    =  \tilZplusT \left( \I +\mu M_t \right)\left( \I -\mu M_t \right) \Zt 
    =  \tilZtT \Zt - \mu^2  \tilZtT M_t^2 \Zt. 
\end{align*}
It follows that 
\begin{align}
  \norm{\tilZplusT \Zplus }
  \le & \norm{ \tilZtT \Zt} + \mu^2 \norm{M_t}^2 \norm{\tilZt} \norm{\Zt} \nonumber \\ 
  \le &  \norm{ \tilZtT \Zt} + 4 \mu^2 \norm{M_t}^2 \norm{X}, \label{ineq:balancebase1}
\end{align}
where in the last line we used that by symmetry $ \norm{\tilZt} = \norm{\Zt}$ and that by assumption $ \norm{\Zt} \le 2 \sqrt{\norm{X}} $.
In order to proceed we note that 
\begin{align*}
 \norm{M_t} \le \norm{\Zt}^2 + \norm{\tilZt}^2 + \norm{X} + \norm{\Deltat} \le 10 \norm{X},   
\end{align*}
where in the last line we used the assumptions $ \norm{\Zt} \le 2 \sqrt{\norm{X}}$ and $\norm{\Deltat} \le \norm{X}$ and that by symmetry $ \norm{\Zt} = \norm{\tilZt} $.
Inserting this inequality into \eqref{ineq:balancebase1} proves the claim.
\end{proof}