\subsection{Proof of Lemma \ref{lemma:noisetermgrowth}: Controlling $\norm{\Zt\Qtp}$}\label{sec:noisetermgrowth}

\begin{proof}[Proof of Lemma \ref{lemma:noisetermgrowth}]
We first derive a formula for $\QtT\Qplusp$.
By the definition of $\Qplusp$ we have $\LAT\Zplus\Qplusp = 0$.
Combined with $\Qt\QtT + \Qtp\QtpT = \I$, we obtain that
\begin{equation*}
    \LAT\Zplus\Qt\QtT\Qplusp = -\LAT\Zplus\Qtp\QtpT\Qplusp,
\end{equation*}
which implies
\begin{equation}\label{QtTQpluspeq}
\QtT\Qplusp = - \left(\LAT\Zplus\Qt \right)^{-1}\LAT\Zplus\Qtp\QtpT\Qplusp.
\end{equation}
Due to $\LAT\Zplus\Qplusp = 0$ we have
\begin{equation*}
\Zplus\Qplusp = \LA\LAT\Zplus\Qplusp + \LAP\LAPT\Zplus\Qplusp = \LAP\LAPT\Zplus\Qplusp,
\end{equation*}
which implies $\norm{\Zplus\Qplusp} = \norm{\LAPT\Zplus\Qplusp}$.
Using equation \eqref{QtTQpluspeq} we obtain that
\begin{align*}
    \LAPT\Zplus\Qplusp = & \LAPT\Zplus\Qt\QtT\Qplusp + \LAPT\Zplus\Qtp\QtpT\Qplusp \\
    = & -\LAPT\Zplus\Qt(\LAT\Zplus\Qt)^{-1}\LAT\Zplus\Qtp\QtpT\Qplusp + \LAPT\Zplus\Qtp\QtpT\Qplusp.
\end{align*}
Note that
\begin{align*}
    \LAPT\Zplus\Qt(\LAT\Zplus\Qt)^{-1}= & \LAPT\P{\Zplus\Qt}\P{\Zplus\Qt}^T\Zplus\Qt\left(\LAT\P{\Zplus\Qt}\P{\Zplus\Qt}^T\Zplus\Qt\right)^{-1} \\
    = & \LAPT\P{\Zplus\Qt}\P{\Zplus\Qt}^T\Zplus\Qt\left(\P{\Zplus\Qt}^T\Zplus\Qt\right)^{-1}\left(\LAT\P{\Zplus\Qt}\right)^{-1} \\
    = & \LAPT\P{\Zplus\Qt}\left(\LAT\P{\Zplus\Qt}\right)^{-1}.
\end{align*}
Thus, we obtain that 
\begin{equation*}
\LAPT\Zplus\Qplusp = -\LAPT\P{\Zplus\Qt}(\LAT\P{\Zplus\Qt})^{-1}\LAT\Zplus\Qtp\QtpT\Qplusp + \LAPT\Zplus\Qtp\QtpT\Qplusp.
\end{equation*}
By using the triangle inequality and the submultiplicativity of the spectral norm we obtain that
\begin{align}\label{LAPTZplusQplusple}
    \norm{\Zplus\Qplusp} = & \norm{\LAPT\Zplus\Qplusp} \nonumber\\
    \le & \norm{\LAPT\P{\Zplus\Qt}(\LAT\P{\Zplus\Qt})^{-1}\LAT\Zplus\Qtp\QtpT\Qplusp} + \norm{\LAPT\Zplus\Qtp\QtpT\Qplusp} \nonumber\\
    \le & \norm{\LAPT\P{\Zplus\Qt}} \norm{\left(\LAT\P{\Zplus\Qt}\right)^{-1}} \norm{\LAT\Zplus\Qtp} + \norm{\LAPT\Zplus\Qtp} \nonumber\\
    = & \frac{\norm{\LAPT\P{\Zplus\Qt}}}{\sqrt{1 - \norm{\LAPT\P{\Zplus\Qt}}^2}} \norm{\LAT\Zplus\Qtp} + \norm{\LAPT\Zplus\Qtp}.
\end{align}
In order to proceed bounding $\norm{\Zplus\Qplusp}$ from above, we first derive an upper bound for $\norm{\LAPT\P{\Zplus\Qt}}$. Note that
\begin{equation*}
\Zplus\Qt = \left(\I - \mu\left(\Zt\ZtT - \tilZt\tilZtT - \symA + \Deltat\right) \right)\Zt\Qt
\end{equation*}
For simplicity of notation, define 
\begin{equation*}
M_t := \Zt\ZtT - \tilZt\tilZtT - \symA +\Deltat,
\end{equation*}
\begin{equation*}
\hat{H}_t := \left(\I - \mu M_t \right)\P{\Zt\Qt}.
\end{equation*}
First, we note that 
    \begin{align}
     \norm{M_t}
    \le & \norm{X}+ \norm{\Zt \ZtT} + \norm{\tilZt \tilZtT} + \norm{\Deltat} \nonumber \\
    = & \norm{X}+2 \norm{\Zt}^2 + \norm{\Deltat}\nonumber  \\
    \le & 10 \norm{X}, \label{ineq:boundforM}
\end{align}
where in the last line we used the assumptions $ \norm{\Zt} \le 2 \sqrt{\norm{X}} $, $\norm{\Deltat} \le c \sglmin \left( X\right) $, and that $\norm{\Zt}=\norm{\tilZt}$ by symmetry.
Since $\Sigma_{\Zt\Qt}\Q{\Zt\Qt}^T$ has full rank by assumption, the matrix $H$ has the same column space as $\Zplus\Qt$. 
In particular, we have that
\begin{align*}
    \norm{\LAPT\P{\Zplus\Qt}} = &\norm{\LAPT\P{ \hat{H}_t }} \\
    \le &\norm{\LAPT \hat{H}_t }\norm{(\Sigma_{ \hat{H}_t } \Q{\hat{H}_t }^T)^{-1}} \\
    = &\frac{\norm{\LAPT \hat{H}_t }}{\sglmin \left(\hat{H}_t \right)}.
\end{align*}
Next, we observe that 
\begin{align*}
    \sglmin \left(\hat{H}_t \right) \ge & \sglmin \left( \Id - \mu M_t \right)\sglmin(\P{\Zt\Qt}) \\
    \ge & \left(1 - \mu \norm{M_t}\right)\sglmin(\P{\Zt\Qt}) \ge \frac{1}{2}.
\end{align*}
In the last inequality we used the assumption $\mu \le \frac{c}{\norm{X}\kappa}$ and inequality \eqref{ineq:boundforM}. 
Combining the above two inequalities we obtain that
\begin{align}
    \norm{\LAPT\P{\Zplus\Qt}} \le &2\norm{\LAPT \hat{H}_t } \nonumber\\
    = &2\norm{\LAPT(\I - \mu M_t )\P{\Zt\Qt}} \nonumber\\
    \le &2\norm{\LAPT\P{\Zt\Qt}} + 2\mu\norm{ M_t } \nonumber\\
    \le &2\norm{\LAPT\P{\Zt\Qt}} + 20\mu\norm{X} \label{ineq:aux1212}  \\
    \le &\frac{24c \varepsilon}{\kappa}.\label{LAPTPZplusQtle}
\end{align}
In the last two inequalities we used the assumptions $\mu \le \frac{c \varepsilon }{\norm{X}\kappa}$, $\norm{\LAPT\P{\Zt\Qt}} \le \frac{c \varepsilon }{\kappa}$ and inequality \eqref{ineq:boundforM}. In order to bound the term $\norm{\LAT\Zplus\Qtp}$, which appears in inequality \eqref{LAPTZplusQplusple}, we note that due to $\LAT\Zt\Qtp = 0$ we have that 
\begin{align}\label{LATZplusQtple}
    \norm{\LAT\Zplus\Qtp} = & \norm{\LAT \left( \I - \mu M_t \right)\Zt\Qtp} \nonumber\\
    = & \mu\norm{\LAT M_t\Zt\Qtp} \nonumber\\
    \le & \mu\norm{M_t}\norm{\Zt\Qtp} \nonumber\\
    \le & 10\mu\norm{X}\norm{\Zt\Qtp}.
\end{align}
In the last line we used inequality \eqref{ineq:boundforM}.
\iffalse
\begin{align}\label{LATZplusQtpeq}
    \LAT\Zplus\Qtp = &\LAT\left(\I - \mu\left(\Zt\ZtT - \tilZt\tilZtT - \symA\right) - \mu \Deltat\right)\Zt\Qtp \nonumber\\
    = &-\mu\LAT \left(\Zt\ZtT - \tilZt\tilZtT - \symA -\mu \Deltat \right)\Zt\Qtp \nonumber\\
    = &-\mu\LAT\left(\Zt\ZtT - \tilZt\tilZtT\right)\Zt\Qtp + \mu\LAT \left(\LA\Sigma_X\LAT - \tilLA \Sigma_X\tilLAT \right)\Zt\Qtp -\mu \LAT \Deltat \Zt \Qtp \nonumber\\
    = &-\mu\LAT \left(\Zt\ZtT - \tilZt\tilZtT \right) \Zt\Qtp  -  \mu \LAT \Deltat \Zt \Qtp  .
\end{align}
\fi
It remains to bound $\norm{\LAPT\Zplus\Qtp}$ in inequality \eqref{LAPTZplusQplusple}.
For simplicity of notation we denote $\hatK := \LAPT\Zt\Qtp$. First, we compute that
\begin{align}\label{LAPTZplusQtpeq}
    &\LAPT\Zplus\Qtp \nonumber\\
    = & \LAPT(\Zt - \mu(\Zt\ZtT - \tilZt\tilZtT - \symA + \Deltat)\Zt)\Qtp \nonumber\\
    = & \hatK - \mu\LAPT\Zt\ZtT\LAP \hatK + \mu\LAPT\tilZt\tilZtT\Zt\Qtp - \mu\LAPT\tilLA\Sigma_X\tilLAT\LAP \hatK - \mu \LAPT \Deltat \Zt \Qtp  \nonumber\\
    = & \hatK - \mu\LAPT\Zt(\Qt\QtT + \Qtp\QtpT)\ZtT\LAP \hatK + \mu\LAPT\tilZt\tilZtT\Zt\Qtp - \mu\LAPT\tilLA\Sigma_X\tilLAT\LAP \hatK \nonumber \\
     &- \mu \LAPT \Deltat \Zt \Qtp \nonumber\\
     = & \hatK - \mu\LAPT\Zt \Qt\QtT\ZtT\LAP \hatK - \mu \hatK \hatK^T \hatK + \mu\LAPT\tilZt\tilZtT\Zt\Qtp - \mu\LAPT\tilLA\Sigma_X\tilLAT\LAP \hatK \nonumber \\
     &- \mu \LAPT \Deltat \LAP \hatK  \nonumber\\
    = & \left(\I - \mu\LAPT\tilLA\Sigma_X\tilLAT\LAP - \mu\LAPT\Zt\Qt\QtT\ZtT\LAP - \mu \LAPT \Deltat \LAP \right) \hatK \left(\I - \mu \hatK^T \hatK \right) \nonumber\\
    & - \mu^2 \left( \LAPT\tilLA\Sigma_X\tilLAT\LAP + \LAPT\Zt\Qt\QtT\ZtT\LAP +  \LAPT \Deltat \LAP \right)  \hatK \hatK^T \hatK    \\
    &+ \mu\LAPT\tilZt\tilZtT\Zt\Qtp. \nonumber  
\end{align}
To proceed, we note that 
\begin{align*}
    & \norm{ \left( \I - \mu\LAPT\tilLA\Sigma_X\tilLAT\LAP - \mu\LAPT\Zt\Qt\QtT\ZtT\LAP - \mu \LAPT \Deltat \LAP  \right) \hatK \left(\I - \mu \hatK^T \hatK \right)} \\
    \le & \norm{\I - \mu\LAPT\tilLA\Sigma_X\tilLAT\LAP - \mu\LAPT\Zt\Qt\QtT\ZtT\LAP-  \mu \LAPT \Deltat \LAP }\norm{ \hatK \left(\I - \mu \hatK^T \hatK \right)} \\
    \le & \left(  \norm{ \I - \mu\LAPT\tilLA\Sigma_X\tilLAT\LAP - \mu\LAPT\Zt\Qt\QtT\ZtT\LAP } + \mu \norm{  \LAPT \Deltat \LAP }  \right) \norm{\hatK \left(\I - \mu \hatK^T\hatK \right)} \\
    \stackrel{(a)}{\le} & \left( 1+ \mu c \varepsilon \sglmin (X)  \right)  \norm{\hatK \left(\I - \mu \hatK^T\hatK \right)}  \\
    \stackrel{(b)}{=} &  \left( 1+ \mu c \varepsilon \sglmin (X)  \right) \left(  1 - \mu\norm{\hatK}^2 \right)\norm{\hatK} \\
    \le &  \left( 1+ \mu c \varepsilon \sglmin (X) - \mu\norm{\hatK}^2 \right)\norm{\hatK},
\end{align*}
where in inequality (a) we used the assumptions $ \norm{\Deltat} \le c \varepsilon \sglmin \left( X \right)  $, $ \mu \le \frac{c \varepsilon}{\kappa} $, and $ \norm{\Zt} \le 2 \sqrt[]{\norm{X}} $.
Equation (b) can be derived by the singular value decomposition of $\hat{K}$, the fact $\mu \le \frac{c \varepsilon }{\norm{X}\kappa} \le \frac{1}{\norm{\Zt}^2} \le \frac{1}{3\norm{\hatK}^2}$, and that the function $x \left(1- \mu x^2 \right)$ is monotonically increasing for $x\in [0, \frac{1}{\sqrt{3\mu}}]$. 
Furthermore, we note that
\begin{align*}
    & \mu^2\norm{(\LAPT\tilLA\Sigma_X\tilLAT\LAP + \LAPT\Zt\Qt\QtT\ZtT\LAP + \LAPT \Deltat \LAP  )\hatK \hatK^T \hatK} \\
    \le & \mu^2\norm{\LAPT\tilLA\Sigma_X\tilLAT\LAP + \LAPT\Zt\Qt\QtT\ZtT\LAP+\LAPT \Deltat \LAP}\norm{\hatK \hatK^T \hatK} \\
    \le & \mu^2 \left( \norm{ \LAPT\tilLA\Sigma_X\tilLAT\LAP } + \norm{ \LAPT\Zt\Qt\QtT\ZtT\LAP } + \norm{ \LAPT \Deltat \LAP }  \right)  \norm{\hatK}^3 \\ 
    \le & \mu^2 \left( \norm{X}+ \norm{\Zt}^2 + \norm{\Deltat}\right) \norm{\hatK}^3 \\
    \stackrel{(c)}{\le} & 6\mu^2\norm{X}\norm{\hatK}^3 \\
     \stackrel{(d)}{\le} & \frac{\mu}{2}\norm{\hatK}^3.
\end{align*}
In inequality (c) we use the assumptions $\norm{\Zt} \le 2\sqrt{\norm{X}}$ and $ \norm{\Deltat} \le c \varepsilon \sglmin (X) $. 
Inequality (d) follows from the assumption $\mu \le \frac{c \varepsilon}{\norm{X}\kappa}$.
Moreover, we observe that
\begin{align*}
    \norm{\LAPT\tilZt\tilZtT\Zt\Qtp} \le \norm{\LAPT\tilZt}\norm{\tilZtT\Zt \Qtp}  \le 2\sqrt{\norm{X}}\norm{\tilZtT\Zt \Qtp},
\end{align*}
where in the last inequality we used the assumption $ \norm{\Zt} \le 2 \sqrt{\norm{X} } $ as well as the fact that by symmetry $ \norm{\Zt} = \norm{\tilZt}  $.
Putting the above three inequalities into \eqref{LAPTZplusQtpeq} we obtain that
\begin{align}\label{LAPTZplusQtple}
    \norm{\LAPT\Zplus\Qtp} \le &  \left( 1+ \mu c \varepsilon \sglmin (X) - \mu\norm{\hatK}^2 \right)\norm{\hatK} + \frac{\mu}{2} \norm{\hatK}^3 +  2 \mu \sqrt{\norm{X}}\norm{\tilZtT\Zt \Qtp} \nonumber  \\
    = & \left( 1 - \frac{\mu}{2}\norm{\Zt\Qtp}^2 + \mu c \varepsilon \sglmin (X) \right) \norm{\Zt\Qtp} + 2\mu\sqrt{\norm{X}}\norm{ \tilZtT\Zt \Qtp }.
\end{align}
Putting inequalities \eqref{LAPTPZplusQtle}, \eqref{LATZplusQtple} and \eqref{LAPTZplusQtple} into \eqref{LAPTZplusQplusple} we obtain that
\begin{align*}
    \norm{\Zplus\Qplusp} \le & \frac{\norm{\LAPT\P{\Zplus\Qt}}}{\sqrt{1 - \norm{\LAPT\P{\Zplus\Qt}}^2}}\norm{\LAT\Zplus\Qtp} + \norm{\LAPT\Zplus\Qtp} \\
    \le & \frac{48c\varepsilon}{\kappa}\cdot 10\mu\norm{X}\norm{\Zt\Qtp}+ \left( 1 - \frac{\mu}{2}\norm{\Zt\Qtp}^2 + \mu c \varepsilon \sglmin (X) \right) \norm{\Zt\Qtp} + 2\mu\sqrt{\norm{X}}\norm{ \tilZtT\Zt \Qtp  } \\
    \le & \left(1 - \frac{\mu}{2}\norm{\Zt\Qtp}^2 +\mu \varepsilon\sglmin(X) \right)\norm{\Zt\Qtp} + 2\mu\sqrt{\norm{X}}\norm{ \tilZtT\Zt \Qtp },
\end{align*}
where the last line follows by choosing the absolute constant $c>0$ small enough.
This finishes the proof.
\end{proof}