C(v_1)_{ij}=
\begin{tikzpicture}[baseline=-1cm]
\draw[wall,fill=gray!20] (0,0) -- (-60:2) -- (-120:2) -- cycle;
\draw[edge,-o-={0.7}{>}] (-120:1.2) node[left]{$i$}
	arc[radius=1.2,start angle=-120,end angle=-60] node[right]{$j$};
\draw[fill=white] (0,0)circle(0.1) (-60:2)circle(0.1) (-120:2)circle(0.1);
\end{tikzpicture}
=\sum_{k=1}^n\returnc_k^{-1}
\begin{tikzpicture}[baseline=-1cm]
\draw[wall,fill=gray!20] (0,0) -- (-60:2) -- (-120:2) -- cycle;
\draw[wall,-o-={0.9}{>}] (-60:2) -- (-120:2);
\draw[edge,-o-={0.5}{>}] (-120:1.2) node[left]{$i$}
	arc[radius=0.8,start angle=60,end angle=0] node[below]{$k$\vphantom{$\bar{k}$}};
\draw[edge,-o-={0.5}{<}] (-60:1.2) node[right]{$j$}
	arc[radius=0.8,start angle=120,end angle=180] node[below]{$\bar{k}$};
\draw[fill=white] (0,0)circle(0.1) (-60:2)circle(0.1) (-120:2)circle(0.1);
\end{tikzpicture}
=\sum_{k=1}^n\returnc_k^{-1}\ceC(v_3)_{ki}\ceC(v_2)_{j\bar{k}}.