

\prAtEndRestateiv*

\makeatletter\Hy@SaveLastskip\label{proofsection:prAtEndiv}\ifdefined\pratend@current@sectionlike@label\immediate\write\@auxout{\string\gdef\string\pratend@section@for@proofiv{\pratend@current@sectionlike@label}}\fi\Hy@RestoreLastskip\makeatother\begin{proof}[Proof]\phantomsection\label{proof:prAtEndiv}The key idea is to prove a similar result as \cref {thm:reparam_u_identity}. For terms that zero-out during during the proof of \cref {thm:reparam_u_identity}, we apply \cref {thm:meanfield_superiority} to zero-out those same terms. \par \begin {alignat}{2} &\mathbb {E}\norm {\vt _{\vlambda }\left (\rvvu \right ) - \vz }_2^2 \, \left ( 1 + \norm {\mU }_{\mathrm {F}} \right ) \nonumber \\ &\;= \mathbb {E} \rvvu ^{\top } \mC ^{\top } \mC \rvvu \, \left ( 1 + \norm {\mU }_{\mathrm {F}} \right ) \nonumber \\ &\;\quad + 2\,\mathbb {E} \rvvu ^{\top } \mC ^{\top } \left ( \vm - \vz \right ) \left ( 1 + \norm {\mU }_{\mathrm {F}} \right ) \nonumber \\ &\;\quad + {\left ( \vm - \vz \right )}^{\top } \left ( \vm - \vz \right ) \left ( 1 + \mathbb {E} \norm {\mU }_{\mathrm {F}} \right ) \nonumber \shortintertext {invoking the trace trick,} &\;= \norm {\vm - \vz } \left ( 1 + \mathbb {E} \norm {\mU }_{\mathrm {F}}\right ). \nonumber \\ &\;\quad + 2\,\mathbb {E} \left ( 1 + \norm {\mU }_{\mathrm {F}} \right ) \, \rvvu ^{\top } \mC ^{\top } \left ( \vm - \vz \right ) \nonumber \\ &\;\quad + \mathrm {tr}\left ( \mC ^{\top } \mC \, \mathbb {E} \rvvu \rvvu ^{\top } \left ( 1 + \norm {\mU }_{\mathrm {F}}\right ) \right ) \nonumber \end {alignat} \par \begin {alignat*}{2} \mathbb {E} \norm {\mathbfsf {U}}_{\mathrm {F}} &\;= \mathbb {E} \sqrt { \mathrm {tr}\left ( \mathbfsf {U} \mathbfsf {U} \right ) } \\ &\;= \mathbb {E} \sqrt { \sum _{i=1}^d \rvu _i^4 }, \shortintertext {using Jensen's inequality,} &\;\leq \sqrt { \mathbb {E} \sum _{i=1}^d \rvu _i^4 } \\ &\;= \sqrt { d \kappa }. \end {alignat*} \par \begin {alignat*}{2} \mathbb {E} \left ( \norm {\mathbfsf {U}}_{\mathrm {F}} + 1\right ) \rvu _i &\;= \mathbb {E} \left ( \sqrt { \sum ^d_{i=1} \rvu _i^4 } + 1\right ) \rvu _i , \shortintertext {applying \(\sqrt {a + b} \leq \sqrt {a} + \sqrt {b}\),} &\;\leq \mathbb {E} \left ( \sum ^d_{i=1} \rvu _i^2 + 1\right ) \rvu _i \\ &\;= \mathbb {E} \, \rvu _i \, \sum _{j \neq i} \rvu _j^2 + \rvu _i^3 + \rvu _i, \shortintertext {and applying \cref {assumption:symmetric_standard},} &\;= 0. \end {alignat*} \par \begin {alignat*}{2} \mathbb {E} \rvu _i \rvu _j \norm {\mathbfsf {U}}_{\mathrm {F}} &\;= \mathbb {E} \rvu _i \rvu _j \left ( \sqrt { \sum _{k=1}^d \rvu _k^4 } \right ), \shortintertext {again, applying \(\sqrt {a + b} \leq \sqrt {a} + \sqrt {b}\),} &\;\leq \mathbb {E} \rvu _i \rvu _j \sum _{k=1}^d \rvu _k^2, \shortintertext {decomposing the sum,} &\;= \mathbb {E} \rvu _i^3 + \rvu _j^3 + \rvu _i \rvu _j \sum _{k \neq i, k \neq j} \rvu _k^2, \shortintertext {and applying \cref {assumption:symmetric_standard},} &\;= 0. \end {alignat*} \par \begin {alignat*}{2} \mathbb {E} \rvu _i \rvu _i \norm {\mathbfsf {U}}_{\mathrm {F}} &\;= \mathbb {E} \rvu _i^2 \left ( \sqrt { \sum _{k=1}^d \rvu _k^4 } \right ), \shortintertext {applying Cauchy-Schwarz's inequality for expectations,} &\;\leq \sqrt { \left ( \mathbb {E} \sum _{k=1}^d \rvu _k^4 \right ) \left ( \mathbb {E} \rvu _i^4 \right ) }, \shortintertext {and given \cref {assumption:symmetric_standard},} &\;= \sqrt { \left ( d \kappa \right ) \left ( \kappa \right ) } \\ &\;= \kappa \sqrt { d }. \end {alignat*} \par Combining all the results, \begin {alignat*}{2} &\mathbb {E}\norm {\vt _{\vlambda }\left (\rvvu \right ) - \vz }_2^2 \, \left ( 1 + \norm {\mU }_{\mathrm {F}} \right ) \\ &\;\leq \norm { \vm - \vz }_2^2 \left ( \vm - \vz \right ) \left ( 1 + \mathbb {E} \norm {\mU }_{\mathrm {F}}\right ) \\ &\;\quad + 2\,\mathbb {E} \left ( 1 + \norm {\mU }_{\mathrm {F}} \right ) \, \rvvu ^{\top } \mC ^{\top } \left ( \vm - \vz \right ) \\ &\;\quad + \mathrm {tr}\left ( \mC ^{\top } \mC \, \mathbb {E} \rvvu \rvvu ^{\top } \left ( 1 + \norm {\mU }_{\mathrm {F}}\right ) \right ) \\ &\;\leq \sqrt {d \kappa } \norm { \vm - \vz }_2^2 + \mathrm {tr}\left ( \mC ^{\top } \mC \left (\mI + \kappa \sqrt {d} \mI \right ) \right ) \\ &\;= \sqrt {d \kappa } \norm { \vm - \vz }_2^2 + \left (\kappa \sqrt {d} + 1\right ) \mathrm {tr}\left ( \mC ^{\top } \mC \right ) \\ &\;= \sqrt {d \kappa } \norm { \vm - \vz }_2^2 + \left (\kappa \sqrt {d} + 1\right ) \norm { \mC }_{\mathrm {F}}^2. \end {alignat*} \par \end{proof}
