% \begin{gmchange}
\section{Proofs}
\subsection{Proof for~\cref{th:nnfdaglinear}  in~\cref{sec:background:propositional-logic}}%
\label{sec:proofnnfdaglinear}
%
\begin{figure}[th]
    \centering
    \begin{subfigure}[t]{0.48\textwidth}
        \input{nnf_dag_and.tex}
        \caption{Case $\vi\defas\vi_1\wedge\vi_2$}%
        \label{fig:2root:and}
    \end{subfigure}
    \begin{subfigure}[t]{0.48\textwidth}
        \input{nnf_dag_iff.tex}
        \caption{Case $\vi\defas\vi_1\iff\vi_2$}%
        \label{fig:2root:iff}
    \end{subfigure}
    %    \vspace{-.3cm}
    \caption{2-root DAGs for the pair $\langle{\NNF{\vi}},\NNF{\neg\vi}\rangle$ for $\vi\defas\vi_1\wedge\vi_2$ and $\vi\defas\vi_1\iff\vi_2$ (those for $\vi_1\vee\vi_2$ and $\vi_1\imp\vi_2$ are similar to that of $\vi_1\wedge\vi_2$).}%
    \label{fig:2root}
\end{figure}
%We present the proof for~\cref{th:nnfdaglinear} in~\cref{sec:background:propositional-logic}.
\begin{proof}
    The NNF DAG that represents \NNF{\vi} is a sub-graph of the 2-root DAG for the
    pair $\langle{\NNF{\vi}},\NNF{\neg\vi}\rangle$ %\GMCHANGE{
    %}. 
    We prove
    that the latter grows linearly in size w.r.t.\ $\vi$ by reasoning
    inductively on the structure of \vi. (The size of a DAG ``$\dots$'' is denoted with ``$|\dots|$''.)
    %i.e.\ ``|\dots|'' is \#nodes(\dots)+\#arcs(\dots).
    %    We prove it by induction on the structure of \vi.
    \begin{description}
        \item[if $\vi$ is an atom:] $\NNF{\vi}=\vi$ and
            $\NNF{\neg\vi}=\neg\vi$, so that $|\langle\NNF{\vi},\NNF{\neg\vi}\rangle|=2$.
        \item[if $\vi\defas\neg\vi_1$:] we assume by induction that
            we have computed
            \tuple{\NNF{\vi_1},\NNF{\neg\vi_1}}. Then
            $\tuple{\NNF{\vi},\NNF{\neg\vi}}=\tuple{\NNF{\neg\vi_1},\NNF{\vi_1}}$
            (i.e., we just invert the
            order of the pair), so that
            $|\tuple{\NNF{\vi},\NNF{\neg\vi}}|=|\tuple{\NNF{\neg\vi_1},\NNF{\vi_1}}|=|\tuple{\NNF{\vi_1},\NNF{\neg\vi_1}}|$.
            % $|\langle\NNF{\neg\vi_1},\NNF{\vi_1}\rangle|=|\langle\NNF{\vi_1},\NNF{\neg\vi_1}\rangle|$.
            %        \item[if $\vi\defas(\vi_1\bowtie\vi_2)$ s.t.\ $\bowtie\ \in\set{\wedge,\vee,\imp,\iff}$:]
        \item[if $\vi\defas(\vi_1\bowtie\vi_2)$ s.t.\ $\bowtie\ \in\set{\wedge,\iff}$:]
            {we assume by induction that
            we have computed
            \tuple{\NNF{\vi_1},\NNF{\neg\vi_1}} and
            \tuple{\NNF{\vi_2},\NNF{\neg\vi_2}}.
            (See \Cref{fig:2root}). Then we show that}
            \begin{equation}\label{eq:recursize}
                |\langle \NNF{\vi},\NNF{\neg\vi}\rangle| \leq
                18+|\langle \NNF{\vi_1},\NNF{\neg\vi_1}\rangle|+|\langle
                \NNF{\vi_2},\NNF{\neg\vi_2}\rangle|:
            \end{equation}
            % Specifically:
            \begin{description}
                \item[if $\bowtie$ is $\wedge$:]
                    the DAGs for $\NNF{\vi}$ and $\NNF{\neg\vi}$ add 2 ``$\wedge/\vee$'' nodes and $2+2$ arcs:\\
                    $
                        \begin{aligned}
                            \quad\NNF{\pos\phantom{(}\vi_1\wedge\vi_2\phantom{)}}\defas\NNF{\pos\vi_1}\wedge\NNF{\pos\vi_2}; \\
                            \quad\NNF{\neg(\vi_1\wedge\vi_2)}\defas\NNF{\neg\vi_1}\vee\NNF{\neg\vi_2}.
                        \end{aligned}
                    $
                    \\{Thus, $|\langle \NNF{\vi},\NNF{\neg\vi}\rangle| =
                        6+|\langle \NNF{\vi_1},\NNF{\neg\vi_1}\rangle|+|\langle
                        \NNF{\vi_2},\NNF{\neg\vi_2}\rangle|$.}
                    % \item[if $\bowtie$ is $\vee$:]
                    %     the DAGs for $\NNF{\vi}$ and $\NNF{\neg\vi}$ add 2 ``$\wedge/\vee$'' nodes and $2+2$ arcs:\\
                    %     $
                    %         \begin{aligned}
                    %             \quad\NNF{\pos\phantom{(}\vi_1\vee\vi_2\phantom{)}}\defas\NNF{\pos\vi_1}\vee\NNF{\pos\vi_2}; \\
                    %             \quad\NNF{\neg(\vi_1\vee\vi_2)}\defas\NNF{\neg\vi_1}\wedge\NNF{\neg\vi_2}.
                    %         \end{aligned}
                    %     $
                    %     \\{Thus, $|\langle \NNF{\vi},\NNF{\neg\vi}\rangle| =
                    %         6+|\langle \NNF{\vi_1},\NNF{\neg\vi_1}\rangle|+|\langle
                    %         \NNF{\vi_2},\NNF{\neg\vi_2}\rangle|$.}
                    % \item[if $\bowtie$ is $\imp$:]
                    %     the DAGs for $\NNF{\vi}$ and $\NNF{\neg\vi}$ add 2 ``$\wedge/\vee$'' nodes and $2+2$ arcs:\\
                    %     $
                    %         \begin{aligned}
                    %             \quad\NNF{\pos\phantom{(}\vi_1\imp\vi_2\phantom{)}}\defas\NNF{\neg\vi_1}\vee\NNF{\pos\vi_2}; \\
                    %             \quad\NNF{\neg(\vi_1\imp\vi_2)}\defas\NNF{\pos\vi_1}\wedge\NNF{\neg\vi_2}.
                    %         \end{aligned}
                    %     $
                    %     \\{Thus, $|\langle \NNF{\vi},\NNF{\neg\vi}\rangle| =
                    %         6+|\langle \NNF{\vi_1},\NNF{\neg\vi_1}\rangle|+|\langle
                    %         \NNF{\vi_2},\NNF{\neg\vi_2}\rangle|$.}
                \item[if $\bowtie$ is $\iff$:]
                    the DAGs for $\NNF{\vi}$ and $\NNF{\neg\vi}$ share the sub-DAGs for
                    $\NNF{\vi_1}$, $\NNF{\neg\vi_1}$, $\NNF{\vi_2}$, $\NNF{\neg\vi_2}$, adding
                    3+3 ``$\wedge$''/``$\vee$'' nodes and $6+6$ arcs:\\
                    $
                        \begin{aligned}
                            \quad\NNF{\pos\phantom{(}\vi_1\iff\vi_2\phantom{)}}\defas(\NNF{\neg\vi_1}\vee\NNF{\pos\vi_2})\wedge(\NNF{\pos\vi_1}\vee \NNF{\neg\vi_2}); \\
                            \quad\NNF{\neg(\vi_1\iff\vi_2)}\defas(\NNF{\pos\vi_1}\vee\NNF{\pos\vi_2})\wedge(\NNF{\neg\vi_1}\vee\NNF{\neg\vi_2}).
                        \end{aligned}
                    $
                    \\{Thus, $|\langle \NNF{\vi},\NNF{\neg\vi}\rangle| =
                        18+|\langle \NNF{\vi_1},\NNF{\neg\vi_1}\rangle|+|\langle
                        \NNF{\vi_2},\NNF{\neg\vi_2}\rangle|$.}
            \end{description}
        \item[if $\vi\defas(\vi_1\bowtie\vi_2)$ s.t.\ $\bowtie\ \in\set{\vee,\imp}$:]
            %          \item[if $\bowtie\ \in \set{\vee, \imp}$:]
            these cases can be reduced to the previous cases, since $\NNF{\vi_1\vee\vi_2}= \NNF{\neg(\neg\vi_1\wedge\neg\vi_2)}$ and $\NNF{\vi_1\imp\vi_2}= \NNF{\neg(\vi_1\wedge\neg\vi_2)}$.
    \end{description}
    {Therefore, overall, from~\eqref{eq:recursize} we have
    that $|\langle \NNF{\vi},\NNF{\neg\vi}\rangle|$ is $O(|\vi|)$.}
    %18\cdot|\vi|$.}
    %
    % RS; gia' detto nel main part del paper
    % Intuitively, we only need at most 2 nodes for each sub-formula $\vi_i$ of $\vi$,
    % representing $\NNF{\vi_i}$ and $\NNF{\neg\vi_i}$ for positive and negative
    % occurrences of $\vi_i$ respectively. These nodes are shared among up
    % to exponentially-many branches generated by expanding the nested iffs.
\end{proof}
%\end{gmchange}

%%%%%%%%%%%%%%%%%%%%%%%%%%%%%%%%%%%%%%%%%%%%%%%%%%%%%%%%%%%%%
%%%
%%%%%%%%%%%%%%%%%%%%%%%%%%%%%%%%%%%%%%%%%%%%%%%%%%%%%%%%%%%%%
\newpage
%\begin{gmchange}
\newcommand{\muof}[1]{\residual{#1}{\mu}}
\subsection{Proof for~\cref{th:munnf} in~\cref{sec:background:propositional-logic}}%
\label{sec:proofmunnf}

\input{fig_threevalues}
In the following the symbol ``\any'' denotes any formula which is not
in $\set{\top,\bot}$. Following~\citeA{sebastiani_are_2020}, we adopt a 3-value
semantics for residuals $\residual{\vi}{\mu}\in\set{\top,\bot,\any}$,
so that ``$\residual{\vi}{\mu}=\any$'' means
``$\residual{\vi}{\mu}\not\in\set{\top,\bot}$'' and
``$\residual{\vi_1}{\mu}=\residual{\vi_2}{\mu}$'' means that the two
residuals $\residual{\vi_1}{\mu}$ and $\residual{\vi_2}{\mu}$ are either both $\top$, or both $\bot$, or neither is in
\set{\top,\bot}. (Notice that, in the latter case,
$\residual{\vi_1}{\mu}=\residual{\vi_2}{\mu}$ even when
$\residual{\vi_1}{\mu}$ and $\residual{\vi_2}{\mu}$ are different
formulas.)
We extend this definition to tuples in an obvious way:
$\tuple{\residual{\vi_1}{\mu},\dots,\residual{\vi_n}{\mu}}=
    \tuple{\residual{\psi_1}{\mu},\dots,\residual{\psi_n}{\mu}}$ iff
$\residual{\vi_i}{\mu}=\residual{\psi_i}{\mu}$ for each $i\in[1\dots n]$.

The 3-value semantics of the Boolean operators is
reported for convenience in
Figure~\ref{fig:threeval}.
As a straightforward consequence of the above semantics, we have that:
\begin{eqnarray*}
    \residual{(\neg\vi)}{\mu}&=&\neg(\residual{\vi}{\mu})\ \  \mbox{(hereafter
        simply ``$\residual{\neg\vi}{\mu}$'')}\\
    \residual{(\vi_1\bowtie\vi_2)}{\mu}&=&
    \residual{\vi_1}{\mu}\bowtie\residual{\vi_2}{\mu}\ \  \mbox{for $\bowtie\ \in \set{\wedge,\vee,\imp,\iff}$}.
\end{eqnarray*}
Also, the usual transformations apply:
$\muof{\neg(\vi_1\wedge\vi_2)}=\muof{\neg\vi_1}\vee\muof{\neg\vi_2}$,
$\muof{\neg(\vi_1\vee\vi_2)}=\muof{\neg\vi_1}\wedge\muof{\neg\vi_2}$,
$\muof{(\vi_1\iff\vi_2)}=
    (\neg\muof{\vi_1}\vee\muof{\vi_2})\wedge(\muof{\vi_1}\vee\neg\muof{\vi_2})$
and
$\muof{\neg(\vi_1\iff\vi_2)}=
    (\muof{\vi_1}\vee\muof{\vi_2})\wedge(\neg\muof{\vi_1}\vee\neg\muof{\vi_2})$.
%
For convenience, sometimes we denote as $\bar{v}$ the
complement of $v\in\set{\top,\bot,\any}$, i.e. $\bar{v}\defas\neg v$,
so that
$\bar{\top}=\bot, \bar{\bot}=\top,
    \bar{\any}=\any$.

We prove the following property, from which
\cref{th:munnf}
in~\cref{sec:background:propositional-logic} follows directly.

% \ignore{\begin{property}%
%     \label{th:munnf2}
%     Consider a Boolean formula $\vi(\allA)$, and let $\NNF{\vi}$ be its NNF DAG. 
%     Consider a partial assignment $\muA$ on $\allA$. Then
%     $\residual{\vi}{\muA}=v$ iff $\residual{\NNF{\vi}}{\muA}=v$ for $v\in\set{\top,\bot,\any}$.
% \end{property}}

\begin{property}
    Consider a %\ignoreinlong{Boolean }
    formula $\vi$, and let $\NNF{\vi}$ be its
    NNF DAG.\@ Consider a partial assignment $\mu$. % on $\allA$.
    % Let $\langle\NNF{\vi},\NNF{\neg\vi}\rangle$ be the 2-root DAG as
    % in~\cref{sec:proofnnfdaglinear}.
    Then:
    \begin{equation}
        \label{eq:nnfeq}
        \pair{\residual{\vi}{\mu}}{\residual{\neg\vi}{\mu}}=\pair{\residual{\NNF{\vi}}{\mu}}{\residual{\NNF{\neg\vi}}{\mu}}.
    \end{equation}

\end{property}

\begin{proof}%
    % RS: spostato sopra
    % We first notice that $\residual{\vi}{\mu}=v$ iff
    % $\residual{\neg\vi}{\mu}=\bar{v}$, where $\bar{v}$ is the
    % complement of $v$, i.e.\ $\bar{\top}=\bot, \bar{\bot}=\top,
    % \bar{\any}=\any$.
    As in~\cref{sec:proofnnfdaglinear}, we prove this fact by reasoning on the 2-root DAG for the
    pair $\langle\NNF{\vi},\NNF{\neg\vi}\rangle$. Specifically, we
    prove~\eqref{eq:nnfeq}
    by induction on the structure of $\vi$.


    %% RS: spostato a sopra
    % (With a little abuse of notation, we say that $\residual{\vi}{\mu}=\residual{\psi}{\mu}$ even in the case when $\residual{\vi}{\mu}$ and $\residual{\psi}{\mu}$ are different formulas s.t.\ $\residual{\vi}{\mu},\residual{\psi}{\mu}\notin\set{\top,\bot}$, meaning that they both fall in the case $\any$.)
    \begin{description}
        \item[if $\vi$ is an atom:] then $\NNF{\vi}=\vi$ and $\NNF{\neg\vi}=\neg\vi$, so that $\residual{\vi}{\mu}=\residual{\NNF{\vi}}{\mu}$ and $\residual{\neg\vi}{\mu}=\residual{\NNF{\neg\vi}}{\mu}$.
            %------------------- NOT -------------------
        \item[if $\vi\defas\neg\vi_1$:] we assume by induction
            that
            $\pair{\residual{\vi_1}{\mu}}{\residual{\neg\vi_1}{\mu}}=\pair{\residual{\NNF{\vi_1}}{\mu}}{\residual{\NNF{\neg\vi_1}}{\mu}}$.
                {Let $v$ be
                    s.t. $\pair{\residual{\vi}{\mu}}{\residual{\neg\vi}{\mu}}=\pair{v}{\bar{v}}$. Then:}
            \[
                \begin{aligned}
                    \pair{\residual{\neg\vi_1}{\mu}}{\residual{\vi_1}{\mu}}=\pair{v}{\bar{v}}             & \Iff    \\
                    \pair{\residual{\vi_1}{\mu}}{\residual{\neg\vi_1}{\mu}}=\pair{\bar{v}}{v}             & \Iffind \\
                    \pair{\residual{\NNF{\vi_1}}{\mu}}{\residual{\NNF{\neg\vi_1}}{\mu}}=\pair{\bar{v}}{v} & \Iff    \\
                    \pair{\residual{\NNF{\neg\vi_1}}{\mu}}{\residual{\NNF{\vi_1}}{\mu}}=\pair{v}{\bar{v}} &
                \end{aligned}
            \]

            % then $\langle\residual{\neg\vi_1}{\mu},\residual{\vi_1}{\mu}\rangle=\langle v,\bar{v}\rangle$ iff $\langle\residual{\vi_1}{\mu},\residual{\neg\vi_1}{\mu}\rangle=\langle\bar{v},v\rangle$. By induction hypothesis, this holds iff $\langle\residual{\NNF{\vi_1}}{\mu},\residual{\NNF{\neg\vi_1}}{\mu}\rangle=\langle\bar{v},v\rangle$, and so iff $\langle\residual{\NNF{\vi}}{\mu},\residual{\NNF{\neg\vi}}{\mu}\rangle=\langle v,\bar{v}\rangle$;%, hence $\residual{\NNF{\vi}}{\mu}=v$ and $\residual{\NNF{\neg\vi}}{\mu}=\bar{v}$. 
            %        \item[if $\vi\defas(\vi_1\bowtie\vi_2)$:] s.t.\ $\bowtie~\in\set{\wedge,\vee,\imp,\iff}$. We assume by induction that
        \item[if $\vi\defas(\vi_1\bowtie\vi_2)$:] s.t.\ $\bowtie~\in\set{\wedge,\iff}$. We assume by induction that
            \[
                \begin{aligned}
                    \pair{\residual{\vi_1}{\mu}}{\residual{\neg\vi_1}{\mu}}=\pair{\residual{\NNF{\vi_1}}{\mu}}{\residual{\NNF{\neg\vi_1}}{\mu}}, \\
                    \pair{\residual{\vi_2}{\mu}}{\residual{\neg\vi_2}{\mu}}=\pair{\residual{\NNF{\vi_2}}{\mu}}{\residual{\NNF{\neg\vi_2}}{\mu}}.
                \end{aligned}
            \]
            Then,
            \begin{description}
                %--------------- AND ------------------------
                \item[if $\bowtie$ is $\wedge$:]
                    \[
                        \begin{aligned}[t]
                            \langle\residual{(\vi_1\wedge\vi_2)}{\mu},\residual{\neg(\vi_1\wedge\vi_2)}{\mu}\rangle=
                            %\langle\residual{\vi_1}{\mu}\wedge\residual{\vi_2}{\mu},\neg(\residual{\vi_1}{\mu}\wedge\residual{\vi_2}{\mu})\rangle=
                            \langle\residual{\vi_1}{\mu}\wedge\residual{\vi_2}{\mu},\residual{\neg\vi_1}{\mu}\vee\residual{\neg\vi_2}{\mu}\rangle                         & \eqind \\
                            \langle\residual{\NNF{\vi_1}}{\mu}\wedge\residual{\NNF{\vi_2}}{\mu},\residual{\NNF{\neg\vi_1}}{\mu}\vee\residual{\NNF{\neg\vi_2}}{\mu}\rangle & =      \\
                            \langle\residual{(\NNF{\vi_1}\wedge\NNF{\vi_2})}{\mu},\residual{(\NNF{\neg\vi_1}\vee\NNF{\neg\vi_2})}{\mu}\rangle                             & =      \\
                            \langle\residual{\NNF{\vi_1\wedge\vi_2}}{\mu},\residual{\NNF{\neg(\vi_1\wedge\vi_2)}}{\mu}\rangle                                             &
                        \end{aligned}
                    \]
                    %     %--------------- OR ------------------------
                    % \item[if $\bowtie$ is $\vee$:]
                    %     \[
                    %         \begin{aligned}[t]
                    %             \langle\residual{(\vi_1\vee\vi_2)}{\mu},\residual{\neg(\vi_1\vee\vi_2)}{\mu}\rangle=
                    %             %\langle\residual{\vi_1}{\mu}\vee\residual{\vi_2}{\mu},\neg(\residual{\vi_1}{\mu}\vee\residual{\vi_2}{\mu})\rangle=
                    %             \langle\residual{\vi_1}{\mu}\vee\residual{\vi_2}{\mu},\residual{\neg\vi_1}{\mu}\wedge\residual{\neg\vi_2}{\mu}\rangle                         & \eqind \\
                    %             \langle\residual{\NNF{\vi_1}}{\mu}\vee\residual{\NNF{\vi_2}}{\mu},\residual{\NNF{\neg\vi_1}}{\mu}\wedge\residual{\NNF{\neg\vi_2}}{\mu}\rangle & =      \\
                    %             \langle\residual{(\NNF{\vi_1}\vee\NNF{\vi_2})}{\mu},\residual{(\NNF{\neg\vi_1}\wedge\NNF{\neg\vi_2})}{\mu}\rangle                             & =      \\
                    %             \langle\residual{\NNF{\vi_1\vee\vi_2}}{\mu},\residual{\NNF{\neg(\vi_1\vee\vi_2)}}{\mu}\rangle                                                 &
                    %         \end{aligned}
                    %     \]
                    %     %--------------- IMPLIES ------------------------
                    % \item[if $\bowtie$ is $\imp$:]
                    %     \[
                    %         \begin{aligned}[t]
                    %             \langle\residual{(\vi_1\imp\vi_2)}{\mu},\residual{\neg(\vi_1\imp\vi_2)}{\mu}\rangle=
                    %             %\langle\residual{\neg\vi_1}{\mu}\vee\residual{\vi_2}{\mu},\neg(\residual{\neg\vi_1}{\mu}\vee\residual{\vi_2}{\mu})\rangle=
                    %             \langle\residual{\neg\vi_1}{\mu}\vee\residual{\vi_2}{\mu},\residual{\vi_1}{\mu}\wedge\residual{\neg\vi_2}{\mu}\rangle                         & \eqind \\
                    %             \langle\residual{\NNF{\neg\vi_1}}{\mu}\vee\residual{\NNF{\vi_2}}{\mu},\residual{\NNF{\vi_1}}{\mu}\wedge\residual{\NNF{\neg\vi_2}}{\mu}\rangle & =      \\
                    %             \langle\residual{(\NNF{\neg\vi_1}\vee\NNF{\vi_2})}{\mu},\residual{(\NNF{\vi_1}\wedge\NNF{\neg\vi_2})}{\mu}\rangle                             & =      \\
                    %             \langle\residual{\NNF{\vi_1\imp\vi_2}}{\mu},\residual{\NNF{\neg(\vi_1\imp\vi_2)}}{\mu}\rangle                                                 &
                    %         \end{aligned}
                    %     \]

                    %--------------- OR and IMPLIES ------------------------
                    % \item[if $\bowtie\ \in \set{\vee, \imp}$:] \GMCHANGE{these cases can be reduced to the previous cases, since $\NNF{\vi_1\vee\vi_2}=\NNF{\neg(\neg\vi_1\wedge\neg\vi_2)}$ and $\NNF{\vi_1\imp\vi_2}= \NNF{\neg(\vi_1\wedge\neg\vi_2)}$.}
                    %--------------- IFF ------------------------
                \item[if $\bowtie$ is $\iff$:]
                    \[
                        \begin{aligned}
                            \langle\residual{(\vi_1\iff\vi_2)}{\mu},\residual{\neg(\vi_1\iff\vi_2)}{\mu}\rangle                                                                                                                                                 & =      \\
                            \langle\residual{((\neg\vi_1\vee\vi_2)\wedge(\vi_1\vee\neg\vi_2))}{\mu},\residual{((\vi_1\vee\vi_2)\wedge(\vi_1\vee\vi_2))}{\mu}\rangle                                                                                             & =      \\
                            % push the residual inside the conjunctions and disjunctions
                            \langle(\residual{\neg\vi_1}{\mu}\vee\residual{\vi_2}{\mu})\wedge(\residual{\vi_1}{\mu}\vee\residual{\neg\vi_2}{\mu}),(\residual{\vi_1}{\mu}\vee\residual{\vi_2}{\mu})\wedge(\residual{\vi_1}{\mu}\vee\residual{\vi_2}{\mu})\rangle & \eqind \\
                            % apply induction hypothesis by changing each psi into NNF(psi)
                            \langle(\residual{\NNF{\neg\vi_1}}{\mu}\vee\residual{\NNF{\vi_2}}{\mu})\wedge(\residual{\NNF{\vi_1}}{\mu}\vee\residual{\NNF{\neg\vi_2}}{\mu}),                                                                                               \\
                            (\residual{\NNF{\vi_1}}{\mu}\vee\residual{\NNF{\vi_2}}{\mu})\wedge(\residual{\NNF{\vi_1}}{\mu}\vee\residual{\NNF{\vi_2}}{\mu})\rangle                                                                                               & =      \\
                            % extract only the residual (and not NNF) from the conjunctions and disjunctions
                            \langle\residual{((\NNF{\neg\vi_1}\vee\NNF{\vi_2})\wedge(\NNF{\vi_1}\vee\NNF{\neg\vi_2}))}{\mu},                                                                                                                                    &        \\\residual{((\NNF{\vi_1}\vee\NNF{\vi_2})\wedge(\NNF{\vi_1}\vee\NNF{\vi_2}))}{\mu}\rangle&=\\
                            % say that NNF(...) is NNF(\vi_1 \iff \vi_2)
                            \langle\residual{\NNF{\vi_1\iff\vi_2}}{\mu},\residual{\NNF{\neg(\vi_1\iff\vi_2)}}{\mu}\rangle                                                                                                                                       & .
                        \end{aligned}
                    \]


                    % %--------------- OR ------------------------
                    % \item[if $\bowtie$ is $\vee$:] then $\residual{\NNF{\vi}}{\mu}=\residual{\NNF{\vi_1}}{\mu}\vee\residual{\NNF{\vi_2}}{\mu}$ and 
                    % $\residual{\NNF{\neg\vi}}{\mu}=\residual{\NNF{\neg\vi_1}}{\mu}\wedge\residual{\NNF{\neg\vi_2}}{\mu}$, so that:
                    % \begin{alphaenumerate}
                    %     \item $\langle\residual{\vi}{\mu},\residual{\neg\vi}{\mu}\rangle=\langle\top,\bot\rangle$ iff $\residual{\vi_1}{\mu}=\top,\residual{\neg\vi_1}{\mu}=\bot$ or $\residual{\vi_2}{\mu}=\top,\residual{\neg\vi_2}{\mu}=\bot$. By induction hypothesis, this holds iff $\residual{\NNF{\vi_1}}{\mu}=\top,\residual{\NNF{\neg\vi_1}}{\mu}=\bot$ or $\residual{\NNF{\vi_2}}{\mu}=\top,\residual{\NNF{\neg\vi_2}}{\mu}=\bot$, hence iff $\langle\residual{\NNF{\vi}}{\mu},\residual{\NNF{\neg\vi}}{\mu}\rangle=\langle\top,\bot\rangle$;

                    %     \item $\langle\residual{\vi}{\mu},\residual{\neg\vi}{\mu}\rangle=\langle\bot,\top\rangle$ iff $\residual{\vi_1}{\mu}=\residual{\vi_2}{\mu}=\bot,\residual{\neg\vi_1}{\mu}=\residual{\neg\vi_2}{\mu}=\top$. By induction hypothesis, this holds iff $\residual{\NNF{\vi_1}}{\mu}=\residual{\NNF{\vi_2}}{\mu}=\bot,\residual{\NNF{\neg\vi_1}}{\mu}=\residual{\NNF{\neg\vi_2}}{\mu}=\top$, hence iff $\langle\residual{\NNF{\vi}}{\mu},\residual{\NNF{\neg\vi}}{\mu}\rangle=\langle\bot,\top \rangle$;
                    % \end{alphaenumerate}
                    % %------------------- IMPL ----------------------
                    % \item[if $\bowtie$ is $\imp$:] then $\residual{\NNF{\vi}}{\mu}=\residual{\NNF{\neg\vi_1}}{\mu}\vee\residual{\NNF{\vi_2}}{\mu}$ and 
                    % $\residual{\NNF{\neg\vi}}{\mu}=\residual{\NNF{\vi_1}}{\mu}\wedge\residual{\NNF{\neg\vi_2}}{\mu}$, so that:
                    % \begin{alphaenumerate}
                    %     \item $\langle\residual{\vi}{\mu},\residual{\neg\vi}{\mu}\rangle=\langle\top,\bot\rangle$ iff $\residual{\vi_1}{\mu}=\bot,\residual{\neg\vi_1}{\mu}=\top$ or $\residual{\vi_2}{\mu}=\top,\residual{\neg\vi_2}{\mu}=\bot$. By induction hypothesis, this holds iff $\residual{\NNF{\vi_1}}{\mu}=\bot,\residual{\NNF{\neg\vi_1}}{\mu}=\top$ or $\residual{\NNF{\vi_2}}{\mu}=\top,\residual{\NNF{\neg\vi_2}}{\mu}=\bot$, hence iff $\langle\residual{\NNF{\vi}}{\mu},\residual{\NNF{\neg\vi}}{\mu}\rangle=\langle\top,\bot\rangle$;

                    %     \item $\langle\residual{\vi}{\mu},\residual{\neg\vi}{\mu}\rangle=\langle\bot,\top\rangle$ iff $\residual{\neg\vi_1}{\mu}=\residual{\vi_2}{\mu}=\bot,\residual{\vi_1}{\mu}=\residual{\neg\vi_2}{\mu}=\top$. By induction hypothesis, this holds iff $\residual{\NNF{\neg\vi_1}}{\mu}=\residual{\NNF{\vi_2}}{\mu}=\bot,\residual{\NNF{\vi_1}}{\mu}=\residual{\NNF{\neg\vi_2}}{\mu}=\top$, hence iff $\langle\residual{\NNF{\vi}}{\mu},\residual{\NNF{\neg\vi}}{\mu}\rangle=\langle\bot,\top \rangle$;
                    % \end{alphaenumerate}

                    % %------------------- IFF ----------------------
                    % \item[if $\bowtie$ is $\iff$:] then $\residual{\NNF{\vi}}{\mu}=(\residual{\NNF{\vi_1}}{\mu}\vee\residual{\NNF{\neg\vi_2}}{\mu})\wedge(\residual{\NNF{\neg\vi_1}}{\mu}\vee\residual{\NNF{\vi_2}}{\mu})$ and $\residual{\NNF{\neg\vi}}{\mu}=(\residual{\NNF{\vi_1}}{\mu}\vee\residual{\NNF{\vi_2}}{\mu})\wedge(\residual{\NNF{\neg\vi_1}}{\mu}\vee\residual{\NNF{\neg\vi_2}}{\mu})$, so that:    
                    % \begin{alphaenumerate}
                    %     \item $\langle\residual{\vi}{\mu},\residual{\neg\vi}{\mu}\rangle=\langle\top,\bot\rangle$ iff $\residual{\vi_1}{\mu}=\residual{\vi_2}{\mu}=v,\residual{\neg\vi_1}{\mu}=\residual{\neg\vi_2}{\mu}=\bar{v}$. By induction hypothesis, this holds iff $\residual{\NNF{\vi_1}}{\mu}=\residual{\NNF{\vi_2}}{\mu}=v,\residual{\NNF{\neg\vi_1}}{\mu}=\residual{\NNF{\neg\vi_2}}{\mu}=\bar{v}$, hence iff $\langle\residual{\NNF{\vi}}{\mu},\residual{\NNF{\neg\vi}}{\mu}\rangle=\langle\top,\bot\rangle$;

                    %     \item $\langle\residual{\vi}{\mu},\residual{\neg\vi}{\mu}\rangle=\langle\bot,\top\rangle$ iff $\residual{\vi_1}{\mu}=\residual{\neg\vi_2}{\mu}=v,\residual{\neg\vi_1}{\mu}=\residual{\vi_2}{\mu}=\bar{v}$. By induction hypothesis, this holds iff $\residual{\NNF{\vi_1}}{\mu}=\residual{\NNF{\neg\vi_2}}{\mu}=v,\residual{\NNF{\neg\vi_1}}{\mu}=\residual{\NNF{\vi_2}}{\mu}=\bar{v}$, hence iff $\langle\residual{\NNF{\vi}}{\mu},\residual{\NNF{\neg\vi}}{\mu}\rangle=\langle\bot,\top\rangle$;
                    % \end{alphaenumerate}

                    % \item[if $\bowtie$ is $\vee$:] then $\residual{\NNF{\vi}}{\mu}=\residual{\NNF{\vi_1}}{\mu}\vee\residual{\NNF{\vi_2}}{\mu}$, so that:
                    % \begin{alphaenumerate}
                    %     \item if $\residual{\vi}{\mu}=\top$ then $\residual{\vi_1}{\mu}=\top$ or $\residual{\vi_2}{\mu}=\top$. By induction hypothesis, $\residual{\NNF{\vi_1}}{\mu}=\top$ or $\residual{\NNF{\vi_2}}{\mu}=\top$, hence $\residual{\NNF{\vi}}{\mu}=\top$;

                    %     \item if $\residual{\vi}{\mu}=\bot$ then $\residual{\vi_1}{\mu}=\residual{\vi_2}{\mu}=\bot$. By induction hypothesis, $\residual{\NNF{\vi_1}}{\mu}=\residual{\NNF{\vi_2}}{\mu}=\bot$, hence $\residual{\NNF{\vi}}{\mu}=\bot$;

                    %     \item if $\residual{\vi}{\mu}=\star$ then
                    %     $\langle\residual{\vi_1}{\mu},\residual{\vi_2}{\mu}\rangle\in\set{\langle\bot,\star\rangle,\langle\star,\bot\rangle,\langle\star,\star\rangle}$. By induction hypothesis, $\langle\residual{\NNF{\vi_1}}{\mu},\residual{\NNF{\vi_2}}{\mu}\rangle\in\set{\langle\bot,\star\rangle,\langle\star,\bot\rangle,\langle\star,\star\rangle}$, hence $\residual{\NNF{\vi}}{\mu}=\star$;
                    % \end{alphaenumerate}

                    % \item[if $\bowtie$ is $\imp$:] then $\residual{\NNF{\vi}}{\mu}=\residual{\NNF{\neg\vi_1}}{\mu}\vee\residual{\NNF{\vi_2}}{\mu}$, so that:
                    % \begin{alphaenumerate}
                    %     \item if $\residual{\vi}{\mu}=\top$ then $\residual{\vi_1}{\mu}=\bot$ or $\residual{\vi_2}{\mu}=\top$. By induction hypothesis, $\residual{\NNF{\vi_1}}{\mu}=\bot$ or $\residual{\NNF{\vi_2}}{\mu}=\top$, hence $\residual{\NNF{\vi}}{\mu}=\top$;

                    %     \item if $\residual{\vi}{\mu}=\bot$ then $\residual{\vi_1}{\mu}=\top$ and $\residual{\vi_2}{\mu}=\bot$. By induction hypothesis, $\residual{\NNF{\vi_1}}{\mu}=\top$ and $\residual{\NNF{\vi_2}}{\mu}=\bot$, hence $\residual{\NNF{\vi}}{\mu}=\bot$;

                    %     \item if $\residual{\vi}{\mu}=\star$ then
                    %     $\langle\residual{\neg\vi_1}{\mu},\residual{\vi_2}{\mu}\rangle\in\set{\langle\top,\star\rangle,\langle\star,\bot\rangle,\langle\star,\star\rangle}$. By induction hypothesis, $\langle\residual{\NNF{\neg\vi_1}}{\mu},\residual{\NNF{\vi_2}}{\mu}\rangle\in\set{\langle\top,\star\rangle,\langle\star,\bot\rangle,\langle\star,\star\rangle}$, hence $\residual{\NNF{\vi}}{\mu}=\star$;
                    % \end{alphaenumerate}
                    % \item[if $\bowtie$ is $\iff$:] then $\residual{\NNF{\vi}}{\mu}=(\residual{\NNF{\neg\vi_1}}{\mu}\vee\residual{\NNF{\vi_2}}{\mu})\wedge(\residual{\NNF{\vi_1}}{\mu}\vee\residual{\NNF{\neg\vi_2}}{\mu})$, so that:
                    % \begin{alphaenumerate}
                    %     % \item if $\residual{\vi}{\mu}=\top$ then either $\residual{\vi_1}{\mu}=\residual{\vi_2}{\mu}=\top$, $\residual{\neg\vi_1}{\mu}=\residual{\neg\vi_2}{\mu}=\bot$ or $\residual{\vi_1}{\mu}=\residual{\vi_2}{\mu}=\bot$,$\residual{\neg\vi_1}{\mu}=\residual{\neg\vi_2}{\mu}=\top$. By induction hypothesis, either $\residual{\NNF{\vi_1}}{\mu}=\residual{\NNF{\vi_2}}{\mu}=\top$,$\residual{\NNF{\neg\vi_1}}{\mu}=\residual{\NNF{\neg\vi_2}}{\mu}=\bot$ or $\residual{\NNF{\vi_1}}{\mu}=\residual{\NNF{\vi_2}}{\mu}=\bot$,$\residual{\NNF{\neg\vi_1}}{\mu}=\residual{\NNF{\neg\vi_2}}{\mu}=\top$, hence $\residual{\NNF{\vi}}{\mu}=\top$;
                    %     \item if $\residual{\vi}{\mu}=\top$ then $\langle\residual{\vi_1}{\mu},\residual{\vi_2}{\mu},\residual{\neg\vi_1}{\mu},\residual{\neg\vi_2}{\mu}\rangle\in\set{\langle\top,\top,\bot,\bot\rangle,\langle\bot,\bot,\top,\top\rangle}$. By induction hypothesis, $\langle\residual{\NNF{\vi_1}}{\mu},\residual{\NNF{\vi_2}}{\mu},\residual{\NNF{\neg\vi_1}}{\mu},\residual{\NNF{\neg\vi_2}}{\mu}\rangle\in\set{\langle\top,\top,\bot,\bot\rangle,\langle\bot,\bot,\top,\top\rangle}$, hence $\residual{\NNF{\vi}}{\mu}=\top$;

                    %     \item if $\residual{\vi}{\mu}=\bot$ then $\langle\residual{\vi_1}{\mu},\residual{\vi_2}{\mu},\residual{\neg\vi_1}{\mu},\residual{\neg\vi_2}{\mu}\rangle\in\set{\langle\top,\bot,\bot,\top\rangle,\langle\bot,\top,\top,\bot\rangle}$. By induction hypothesis, $\langle\residual{\NNF{\vi_1}}{\mu},\residual{\NNF{\vi_2}}{\mu},\residual{\NNF{\neg\vi_1}}{\mu},\residual{\NNF{\neg\vi_2}}{\mu}\rangle\in\set{\langle\top,\bot,\bot,\top\rangle,\langle\bot,\top,\top,\bot\rangle}$, hence $\residual{\NNF{\vi}}{\mu}=\bot$;

                    %     \item if $\residual{\vi}{\mu}=\star$ then $\langle\residual{\vi_1}{\mu},\residual{\vi_2}{\mu},\residual{\neg\vi_1}{\mu},\residual{\neg\vi_2}{\mu}\rangle\in\{\langle\top,\star,\bot,\star\rangle$, $\langle\bot,\star,\top,\star\rangle$, $\langle\star,\top,\star,\bot\rangle$, $\langle\star,\bot,\star,\top\rangle$, $\langle\star,\star,\star,\star\rangle\}$. By induction hypothesis, \\$\langle\residual{\NNF{\vi_1}}{\mu},\residual{\NNF{\vi_2}}{\mu},\residual{\NNF{\neg\vi_1}}{\mu},\residual{\NNF{\neg\vi_2}}{\mu}\rangle\in\{\langle\top,\star,\bot,\star\rangle$, $\langle\bot,\star,\top,\star\rangle$, $\langle\star,\top,\star,\bot\rangle$, $\langle\star,\bot,\star,\top\rangle$, $\langle\star,\star,\star,\star\rangle\}$, hence $\residual{\NNF{\vi}}{\mu}=\star$;
                    % \end{alphaenumerate}
            \end{description}
            %--------------- OR and IMPLIES ------------------------
        \item[if $\vi\defas(\vi_1\bowtie\vi_2)$:] s.t.\ $\bowtie~\in\set{\vee,\imp}$. These cases can be reduced to the previous cases, since $\NNF{\vi_1\vee\vi_2}=\NNF{\neg(\neg\vi_1\wedge\neg\vi_2)}$ and $\NNF{\vi_1\imp\vi_2}= \NNF{\neg(\vi_1\wedge\neg\vi_2)}$.
    \end{description}
\end{proof}
{Thus,
$\pair{\residual{\vi}{\mu}}{\residual{\neg\vi}{\mu}}=\pair{\residual{\NNF{\vi}}{\mu}}{\residual{\NNF{\neg\vi}}{\mu}}$
so that $\residual{\vi}{\mu}=v$ iff
$\residual{\NNF{\vi}}{\mu}=v$ for every
$v\in\set{\top,\bot}$, so that \cref{th:munnf}
in~\cref{sec:background:propositional-logic} holds.}

%\end{gmchange}

%%%%%%%%%%%%%%%%%%%%%%%%%%%%%%%%%%%%%%%%%%%%%%%%%%%%%%%%%%%%%
%%%
%%%%%%%%%%%%%%%%%%%%%%%%%%%%%%%%%%%%%%%%%%%%%%%%%%%%%%%%%%%%%

\newpage

% \begin{gmchange}
\subsection{Proof for~\cref{th:existsetaB} in~\cref{sec:solution}}%
\label{sec:proofexistsetaB}
%We present the proof for~\cref{th:existsetaB} in~\cref{sec:solution}.
\begin{proof}%
    We first show how such a $\etaB$ can be built, then we prove that it satisfies \vinnfcnfpg.
    %In order to simplify the proof, we assume that all sub-formulas occur with double polarity in $\vi$.
    For every sub-formula $\vi_i$ of $\vi$, whose positive and negative occurrences in $\vinnfcnfpg$ are associated with the variables $\poslab{B_i}$ and $\neglab{B_i}$ respectively, do:
    \begin{enumerate}[(a)]
        \item if $\residual{\vi_i}{\mualpha} = \top$, and hence $\residual{\NNF{\vi_i}}{\mualpha}=\top$ and $\residual{\NNF{\neg\vi_i}}{\mualpha}=\bot$ by \cref{th:munnf}, then set $\etaB(\poslab{B_i})=\top$ and $\etaB(\neglab{B_i})=\bot$;
        \item if $\residual{\vi_i}{\mualpha} = \bot$, and hence $\residual{\NNF{\vi_i}}{\mualpha}=\bot$ and $\residual{\NNF{\neg\vi_i}}{\mualpha}=\top$ by \cref{th:munnf}, then set $\etaB(\poslab{B_i})=\bot$ and $\etaB(\neglab{B_i})=\top$;
        \item otherwise if $\residual{\vi_i}{\mualpha} \notin \set{\top,\bot}$, then let $\etaB(\poslab{B_i})=\etaB(\neglab{B_i})=\bot$;
    \end{enumerate}
    (If $\vi_i$ occurs only positively or negatively, then we only assign $\poslab{B_i}$ or $\neglab{B_i}$ respectively.)\\
    We prove that $\mualpha\cup\etaB\pmodels\vinnfcnfpg$ by induction on the structure of $\vinnfcnfpg$.
    Consider a sub-formula $\vi_i$ of $\vi$. Then
    \begin{enumerate}[(i)]
        \item $\vinnfcnfpg\defas\PlaistedCNF(
                  \overbrace{\NNF{\vi}[\NNF{\vi_i}|\poslab{B_i}]}^{(1)} \wedge
                  \overbrace{\left(\neg \poslab{B_i}\vee\NNF{\vi_i}\right)}^{(2)})$ if $\vi_i$ occurs positively in $\vi$;
        \item $\vinnfcnfpg\defas\PlaistedCNF(
                  \overbrace{\NNF{\vi}[\NNF{\neg\vi_i}|\neglab{B_i}]}^{(3)} \wedge
                  \overbrace{\left(\neg \neglab{B_i}\vee\NNF{\neg\vi_i}\right)}^{(4)})$ if $\vi_i$ occurs negatively in $\vi$;
    \end{enumerate}
    % \begin{subequations}
    % \begin{align}
    %     \vinnfcnfpg\defas\PlaistedCNF\Big(
    %         \label{eq:proof:a}&\NNF{\vi}[\NNF{\vi_i},\NNF{\neg\vi_i}/\poslab{B_i},\neglab{B_i}]
    %      \wedge\\
    %      \label{eq:proof:b}& \left(\neg \poslab{B_i}\vee\NNF{\vi_i}\right) \wedge \\
    %      \label{eq:proof:c}& \left(\neg \neglab{B_i}\vee\NNF{\neg\vi_i}\right)\Big).
    % \end{align}
    % \end{subequations}
    For each pair of cases we have:
    \begin{enumerate}[(a)]
        \item\begin{enumerate}[(i)]
            \item $\mualpha\cup\etaB\pmodels
                      (1)$ since we substitute $\top$ for $\top$; $\mualpha\cup\etaB\pmodels
                      (2)$ since $\mualpha\pmodels\NNF{\vi_i}$;
            \item $\mualpha\cup\etaB\pmodels
                      (3)$ since we substitute $\bot$ for $\bot$; $\mualpha\cup\etaB\pmodels
                      (4)$ since $\mualpha\pmodels\neg\neglab{B_i}$;
        \end{enumerate}
        \item \begin{enumerate}[(i)]
                  \item $\mualpha\cup\etaB\pmodels
                            (1)$ since we substitute $\bot$ for $\bot$; $\mualpha\cup\etaB\pmodels
                            (2)$ since $\mualpha\pmodels\neg\poslab{B_i}$;
                  \item $\mualpha\cup\etaB\pmodels
                            (3)$ since we substitute $\top$ for $\top$; $\mualpha\cup\etaB\pmodels
                            (4)$ since $\mualpha\pmodels\NNF{\neg\vi_i}$;
              \end{enumerate}
        \item \begin{enumerate}[(i)]
                  \item $\mualpha\cup\etaB\pmodels
                            (1)$ since we substitute $\bot$ for $*$; $\mualpha\cup\etaB\pmodels
                            (2)$ since $\mualpha\pmodels\neg\poslab{B_i}$;
                  \item $\mualpha\cup\etaB\pmodels
                            (3)$ since we substitute $\bot$ for $*$; $\mualpha\cup\etaB\pmodels
                            (4)$ since $\mualpha\pmodels\neg\neglab{B_i}$;
              \end{enumerate}
              %----------------------------------------
              % \item $\muA\cup\etaB\pmodels%\eqref{eq:proof:a}
              % (1)$ because we substitute $\top$ for $\top$ and $\bot$ for $\bot$; $\muA\cup\etaB\pmodels%\eqref{eq:proof:b}
              % (2)$ because $\muA\pmodels\NNF{\vi_i}$; $\muA\cup\etaB\pmodels%\eqref{eq:proof:c}
              % TODO$ because $\etaB\pmodels\neg\neglab{B_i}$;
              % \item $\muA\cup\etaB\pmodels%\eqref{eq:proof:a}
              % TODO$ because we substitute $\bot$ for $\bot$ and $\top$ for $\top$; $\muA\cup\etaB\pmodels%\eqref{eq:proof:b}
              % TODO$ because $\etaB\pmodels\neg\poslab{B_i}$; $\muA\cup\etaB\pmodels%\eqref{eq:proof:c}
              % TODO$ because $\muA\pmodels\NNF{\neg\vi_i}$;
              % \item $\muA\cup\etaB\pmodels%\eqref{eq:proof:a}
              % TODO$ because $\muA$ satisfies $\vi$ even without assigning a truth value to $\vi_i$, so that we can safely substitute both $\NNF{\vi_i}$ and $\NNF{\neg\vi_i}$ with $\bot$; $\muA\cup\etaB\pmodels%\eqref{eq:proof:b}
              % TODO$ because $\etaB\pmodels\neg\poslab{B_i}$;
              % $\muA\cup\etaB\pmodels%\eqref{eq:proof:c}
              % TODO$ because $\etaB\pmodels\neg\neglab{B_i}$.
    \end{enumerate}
    Therefore, $\mualpha\cup\etaB\pmodels\vinnfcnfpg$.
\end{proof}

% \end{gmchange}
\newpage
\section{An analysis of candidate solvers}%
\label{appendix:tooltable}

In Table~\ref{tab:allsat-solvers} we report an analysis of the features of every candidate
AllSAT and AllSMT solver, as discussed in \sref{sec:survey-allsat-solvers}.

\input{tools-table}
\newpage

\section{Details on experimental results}%

\label{appendix:experiments}
    In this section, we report the scatter plots on individual
    benchmarks for the experiments presented
    in~\cref{sec:experiments:results}, \cref{fig:plt:all:bool:scatter,fig:plt:all:lra:scatter}.
    In particular, \cref{fig:plt:syn:bool:scatter,,fig:plt:circ:scatter,,fig:plt:aig:scatter} show the results on the Boolean synthetic, ISCAS'85 and WMI benchmarks, respectively. \cref{fig:plt:syn:lra:scatter,,fig:plt:wmi:scatter} show the results of the AllSMT experiments on the synthetic and WMI benchmarks, respectively.
\begin{figure}
    \centering
    % \begin{subfigure}[t]{\textwidth}
    \begin{subfigure}[t]{\textwidth}
        \begin{subfigure}[t]{0.29\textwidth}
            \includegraphics[width=\textwidth]{plots/bool/no-rep/syn-bool/models_compare_LAB_vs_LABELNEG_POL.pdf}%
            \label{fig:plt:syn:bool:norep:models:lab_vs_pol}
        \end{subfigure}\hfill
        \begin{subfigure}[t]{0.29\textwidth}
            \includegraphics[width=\textwidth]{plots/bool/no-rep/syn-bool/models_compare_LABELNEG_POL_vs_NNF_MUTEX_POL.pdf}%
            \label{fig:plt:syn:bool:norep:models:pol_vs_nnfpol}
        \end{subfigure}\hfill
        \begin{subfigure}[t]{0.29\textwidth}
            \includegraphics[width=\textwidth]{plots/bool/no-rep/syn-bool/models_compare_LAB_vs_NNF_MUTEX_POL.pdf}%
            \label{fig:plt:syn:bool:norep:models:lab_vs_nnfpol}
        \end{subfigure}\hfill
        \begin{subfigure}[t]{0.29\textwidth}
            \includegraphics[width=\textwidth]{plots/bool/no-rep/syn-bool/time_compare_LAB_vs_LABELNEG_POL.pdf}%
            \label{fig:plt:syn:bool:norep:time:lab_vs_pol}
        \end{subfigure}\hfill
        \begin{subfigure}[t]{0.29\textwidth}
            \includegraphics[width=\textwidth]{plots/bool/no-rep/syn-bool/time_compare_LABELNEG_POL_vs_NNF_MUTEX_POL.pdf}%
            \label{fig:plt:syn:bool:norep:time:pol_vs_nnfpol}
        \end{subfigure}\hfill
        \begin{subfigure}[t]{0.29\textwidth}
            \includegraphics[width=\textwidth]{plots/bool/no-rep/syn-bool/time_compare_LAB_vs_NNF_MUTEX_POL.pdf}%
            \label{fig:plt:syn:bool:norep:time:lab_vs_nnfpol}
            % \end{subfigure}
        \end{subfigure}
        \caption{Results for disjoint enumeration. %\TseitinCNF{}, \PlaistedCNF{} and $\NNFna{}+\PlaistedCNF$ reported 163, 94 and 20 timeouts, respectively (points on the dashed lines).
        }%
        \label{fig:plt:syn:bool:norep:scatter}
    \end{subfigure}
    %%%%%%%%%%%% REP %%%%%%%%%%%%%
    \begin{subfigure}[t]{\textwidth}
        \begin{subfigure}[t]{0.29\textwidth}
            \includegraphics[width=\textwidth]{plots/bool/rep/syn-bool/models_compare_LAB_vs_LABELNEG_POL.pdf}%
            \label{fig:plt:syn:bool:rep:models:lab_vs_pol}
        \end{subfigure}\hfill
        \begin{subfigure}[t]{0.29\textwidth}
            \includegraphics[width=\textwidth]{plots/bool/rep/syn-bool/models_compare_LABELNEG_POL_vs_NNF_MUTEX_POL.pdf}%
            \label{fig:plt:syn:bool:rep:models:pol_vs_nnfpol}
        \end{subfigure}\hfill
        \begin{subfigure}[t]{0.29\textwidth}
            \includegraphics[width=\textwidth]{plots/bool/rep/syn-bool/models_compare_LAB_vs_NNF_MUTEX_POL.pdf}%
            \label{fig:plt:syn:bool:rep:models:lab_vs_nnfpol}
        \end{subfigure}\hfill
        \begin{subfigure}[t]{0.29\textwidth}
            \includegraphics[width=\textwidth]{plots/bool/rep/syn-bool/time_compare_LAB_vs_LABELNEG_POL.pdf}%
            \label{fig:plt:syn:bool:rep:time:lab_vs_pol}
        \end{subfigure}\hfill
        \begin{subfigure}[t]{0.29\textwidth}
            \includegraphics[width=\textwidth]{plots/bool/rep/syn-bool/time_compare_LABELNEG_POL_vs_NNF_MUTEX_POL.pdf}%
            \label{fig:plt:syn:bool:rep:time:pol_vs_nnfpol}
        \end{subfigure}\hfill
        \begin{subfigure}[t]{0.29\textwidth}
            \includegraphics[width=\textwidth]{plots/bool/rep/syn-bool/time_compare_LAB_vs_NNF_MUTEX_POL.pdf}%
            \label{fig:plt:syn:bool:rep:time:lab_vs_nnfpol}
            % \end{subfigure}
        \end{subfigure}
        \caption{Results for non-disjoint enumeration. %\TseitinCNF{}, \PlaistedCNF{} and $\NNFna{}+\PlaistedCNF$ reported 122, 69 and 0 timeouts, respectively (points on the dashed lines).
        }%
        \label{fig:plt:syn:bool:rep:scatter}
    \end{subfigure}
    \caption{Set of scatter plots comparing the different CNF-izations on the Boolean synthetic benchmarks. The first and second rows compare them in terms of size of \TAna{} and execution time, respectively. All the axes are on a logarithmic scale.}%
    \label{fig:plt:syn:bool:scatter}
\end{figure}
\begin{figure}
    \centering
    % \begin{subfigure}[t]{\textwidth}
    \begin{subfigure}[t]{\textwidth}
        \begin{subfigure}[t]{0.29\textwidth}
            \includegraphics[width=\textwidth]{plots/bool/no-rep/iscas85/models_compare_LAB_vs_LABELNEG_POL.pdf}%
            \label{fig:plt:circ:norep:models:lab_vs_pol}
        \end{subfigure}\hfill
        \begin{subfigure}[t]{0.29\textwidth}
            \includegraphics[width=\textwidth]{plots/bool/no-rep/iscas85/models_compare_LABELNEG_POL_vs_NNF_MUTEX_POL.pdf}%
            \label{fig:plt:circ:norep:models:pol_vs_nnfpol}
        \end{subfigure}\hfill
        \begin{subfigure}[t]{0.29\textwidth}
            \includegraphics[width=\textwidth]{plots/bool/no-rep/iscas85/models_compare_LAB_vs_NNF_MUTEX_POL.pdf}%
            \label{fig:plt:circ:norep:models:lab_vs_nnfpol}
        \end{subfigure}\hfill
        \begin{subfigure}[t]{0.29\textwidth}
            \includegraphics[width=\textwidth]{plots/bool/no-rep/iscas85/time_compare_LAB_vs_LABELNEG_POL.pdf}%
            \label{fig:plt:circ:norep:time:lab_vs_pol}
        \end{subfigure}\hfill
        \begin{subfigure}[t]{0.29\textwidth}
            \includegraphics[width=\textwidth]{plots/bool/no-rep/iscas85/time_compare_LABELNEG_POL_vs_NNF_MUTEX_POL.pdf}%
            \label{fig:plt:circ:norep:time:pol_vs_nnfpol}
        \end{subfigure}\hfill
        \begin{subfigure}[t]{0.29\textwidth}
            \includegraphics[width=\textwidth]{plots/bool/no-rep/iscas85/time_compare_LAB_vs_NNF_MUTEX_POL.pdf}%
            \label{fig:plt:circ:norep:time:lab_vs_nnfpol}
            % \end{subfigure}
        \end{subfigure}
        \caption{Results for disjoint enumeration. %\TseitinCNF{}, \PlaistedCNF{} and $\NNFna{}+\PlaistedCNF$ reported 49, 44 and 27 timeouts, respectively (points on the dashed lines).
        }%
        \label{fig:plt:circ:norep:scatter}
    \end{subfigure}
    %%%%%%%%%%%% REP %%%%%%%%%%%%%
    \begin{subfigure}[t]{\textwidth}
        \begin{subfigure}[t]{0.29\textwidth}
            \includegraphics[width=\textwidth]{plots/bool/rep/iscas85/models_compare_LAB_vs_LABELNEG_POL.pdf}%
            \label{fig:plt:circ:rep:models:lab_vs_pol}
        \end{subfigure}\hfill
        \begin{subfigure}[t]{0.29\textwidth}
            \includegraphics[width=\textwidth]{plots/bool/rep/iscas85/models_compare_LABELNEG_POL_vs_NNF_MUTEX_POL.pdf}%
            \label{fig:plt:circ:rep:models:pol_vs_nnfpol}
        \end{subfigure}\hfill
        \begin{subfigure}[t]{0.29\textwidth}
            \includegraphics[width=\textwidth]{plots/bool/rep/iscas85/models_compare_LAB_vs_NNF_MUTEX_POL.pdf}%
            \label{fig:plt:circ:rep:models:lab_vs_nnfpol}
        \end{subfigure}\hfill
        \begin{subfigure}[t]{0.29\textwidth}
            \includegraphics[width=\textwidth]{plots/bool/rep/iscas85/time_compare_LAB_vs_LABELNEG_POL.pdf}%
            \label{fig:plt:circ:rep:time:lab_vs_pol}
        \end{subfigure}\hfill
        \begin{subfigure}[t]{0.29\textwidth}
            \includegraphics[width=\textwidth]{plots/bool/rep/iscas85/time_compare_LABELNEG_POL_vs_NNF_MUTEX_POL.pdf}%
            \label{fig:plt:circ:rep:time:pol_vs_nnfpol}
        \end{subfigure}\hfill
        \begin{subfigure}[t]{0.29\textwidth}
            \includegraphics[width=\textwidth]{plots/bool/rep/iscas85/time_compare_LAB_vs_NNF_MUTEX_POL.pdf}%
            \label{fig:plt:circ:rep:time:lab_vs_nnfpol}
            % \end{subfigure}
        \end{subfigure}
        \caption{Results for non-disjoint enumeration. %\TseitinCNF{}, \PlaistedCNF{} and $\NNFna{}+\PlaistedCNF$ reported 41, 38 and 3 timeouts, respectively (points on the dashed lines).
        }%
        \label{fig:plt:circ:rep:scatter}
    \end{subfigure}
    \caption{Set of scatter plots comparing the different CNF-izations on the %\ignoreinlong{circuits}\ignoreinshort{\GMCHANGEp{
        ISCAS'85 %}} 
        benchmarks. The first and second rows compare them in terms of size of \TAna{} and execution time, respectively. All the axes are on a logarithmic scale.}%
    \label{fig:plt:circ:scatter}
\end{figure}
\begin{figure}
    \centering
    % \begin{subfigure}[t]{\textwidth}
    \begin{subfigure}[t]{\textwidth}
        \begin{subfigure}[t]{0.29\textwidth}
            \includegraphics[width=\textwidth]{plots/bool/no-rep/aig/models_compare_LAB_vs_LABELNEG_POL.pdf}%
            \label{fig:plt:aig:norep:models:lab_vs_pol}
        \end{subfigure}\hfill
        \begin{subfigure}[t]{0.29\textwidth}
            \includegraphics[width=\textwidth]{plots/bool/no-rep/aig/models_compare_LABELNEG_POL_vs_NNF_MUTEX_POL.pdf}%
            \label{fig:plt:aig:norep:models:pol_vs_nnfpol}
        \end{subfigure}\hfill
        \begin{subfigure}[t]{0.29\textwidth}
            \includegraphics[width=\textwidth]{plots/bool/no-rep/aig/models_compare_LAB_vs_NNF_MUTEX_POL.pdf}%
            \label{fig:plt:aig:norep:models:lab_vs_nnfpol}
        \end{subfigure}\hfill
        \begin{subfigure}[t]{0.29\textwidth}
            \includegraphics[width=\textwidth]{plots/bool/no-rep/aig/time_compare_LAB_vs_LABELNEG_POL.pdf}%
            \label{fig:plt:aig:norep:time:lab_vs_pol}
        \end{subfigure}\hfill
        \begin{subfigure}[t]{0.29\textwidth}
            \includegraphics[width=\textwidth]{plots/bool/no-rep/aig/time_compare_LABELNEG_POL_vs_NNF_MUTEX_POL.pdf}%
            \label{fig:plt:aig:norep:time:pol_vs_nnfpol}
        \end{subfigure}\hfill
        \begin{subfigure}[t]{0.29\textwidth}
            \includegraphics[width=\textwidth]{plots/bool/no-rep/aig/time_compare_LAB_vs_NNF_MUTEX_POL.pdf}%
            \label{fig:plt:aig:norep:time:lab_vs_nnfpol}
            % \end{subfigure}
        \end{subfigure}
        \caption{Results for disjoint enumeration.
            %\TseitinCNF{},\ \PlaistedCNF{} and $\NNFna{}+\PlaistedCNF{}$ reported 79, 73 and 72 timeouts, respectively.
        }%
        \label{fig:plt:aig:norep:scatter}
    \end{subfigure}
    %%%%%%%%%%%% REP %%%%%%%%%%%%%
    \begin{subfigure}[t]{\textwidth}
        \begin{subfigure}[t]{0.29\textwidth}
            \includegraphics[width=\textwidth]{plots/bool/rep/aig/models_compare_LAB_vs_LABELNEG_POL.pdf}%
            \label{fig:plt:aig:rep:models:lab_vs_pol}
        \end{subfigure}\hfill
        \begin{subfigure}[t]{0.29\textwidth}
            \includegraphics[width=\textwidth]{plots/bool/rep/aig/models_compare_LABELNEG_POL_vs_NNF_MUTEX_POL.pdf}%
            \label{fig:plt:aig:rep:models:pol_vs_nnfpol}
        \end{subfigure}\hfill
        \begin{subfigure}[t]{0.29\textwidth}
            \includegraphics[width=\textwidth]{plots/bool/rep/aig/models_compare_LAB_vs_NNF_MUTEX_POL.pdf}%
            \label{fig:plt:aig:rep:models:lab_vs_nnfpol}
        \end{subfigure}\hfill
        \begin{subfigure}[t]{0.29\textwidth}
            \includegraphics[width=\textwidth]{plots/bool/rep/aig/time_compare_LAB_vs_LABELNEG_POL.pdf}%
            \label{fig:plt:aig:rep:time:lab_vs_pol}
        \end{subfigure}\hfill
        \begin{subfigure}[t]{0.29\textwidth}
            \includegraphics[width=\textwidth]{plots/bool/rep/aig/time_compare_LABELNEG_POL_vs_NNF_MUTEX_POL.pdf}%
            \label{fig:plt:aig:rep:time:pol_vs_nnfpol}
        \end{subfigure}\hfill
        \begin{subfigure}[t]{0.29\textwidth}
            \includegraphics[width=\textwidth]{plots/bool/rep/aig/time_compare_LAB_vs_NNF_MUTEX_POL.pdf}%
            \label{fig:plt:aig:rep:time:lab_vs_nnfpol}
            % \end{subfigure}
        \end{subfigure}
        \caption{Results for non-disjoint enumeration.
            %\TseitinCNF{},\ \PlaistedCNF{} and $\NNFna{}+\PlaistedCNF{}$ reported 78, 60 and 51 timeouts, respectively.
        }%
        \label{fig:plt:aig:rep:scatter}
    \end{subfigure}
    \caption{Set of scatter plots comparing the different CNF-izations on the AIG benchmarks. The first and second rows compare them in terms of size of \TA{\vi} and execution time, respectively. All the axes are on a logarithmic scale.}%
    \label{fig:plt:aig:scatter}
\end{figure}
%
\begin{figure}
    \centering
    % \begin{subfigure}[t]{\textwidth}
    \begin{subfigure}[t]{\textwidth}
        \begin{subfigure}[t]{0.29\textwidth}
            \includegraphics[width=\textwidth]{plots/lra/no-rep/syn-lra/models_compare_LAB_vs_LABELNEG_POL.pdf}%
            \label{fig:plt:syn:lra:norep:models:lab_vs_pol}
        \end{subfigure}\hfill
        \begin{subfigure}[t]{0.29\textwidth}
            \includegraphics[width=\textwidth]{plots/lra/no-rep/syn-lra/models_compare_LABELNEG_POL_vs_NNF_MUTEX_POL.pdf}%
            \label{fig:plt:syn:lra:norep:models:pol_vs_nnfpol}
        \end{subfigure}\hfill
        \begin{subfigure}[t]{0.29\textwidth}
            \includegraphics[width=\textwidth]{plots/lra/no-rep/syn-lra/models_compare_LAB_vs_NNF_MUTEX_POL.pdf}%
            \label{fig:plt:syn:lra:norep:models:lab_vs_nnfpol}
        \end{subfigure}\hfill
        \begin{subfigure}[t]{0.29\textwidth}
            \includegraphics[width=\textwidth]{plots/lra/no-rep/syn-lra/time_compare_LAB_vs_LABELNEG_POL.pdf}%
            \label{fig:plt:syn:lra:norep:time:lab_vs_pol}
        \end{subfigure}\hfill
        \begin{subfigure}[t]{0.29\textwidth}
            \includegraphics[width=\textwidth]{plots/lra/no-rep/syn-lra/time_compare_LABELNEG_POL_vs_NNF_MUTEX_POL.pdf}%
            \label{fig:plt:syn:lra:norep:time:pol_vs_nnfpol}
        \end{subfigure}\hfill
        \begin{subfigure}[t]{0.29\textwidth}
            \includegraphics[width=\textwidth]{plots/lra/no-rep/syn-lra/time_compare_LAB_vs_NNF_MUTEX_POL.pdf}%
            \label{fig:plt:syn:lra:norep:time:lab_vs_nnfpol}
            % \end{subfigure}
        \end{subfigure}
        \caption{Results for disjoint enumeration. %\TseitinCNF{}, \PlaistedCNF{} and $\NNFna{}+\PlaistedCNF$ reported 171, 98 and 58 timeouts, respectively (points on the dashed lines).
        }%
        \label{fig:plt:syn:lra:norep:scatter}
    \end{subfigure}
    %%%%%%%%%%%% REP %%%%%%%%%%%%%
    \begin{subfigure}[t]{\textwidth}
        \begin{subfigure}[t]{0.29\textwidth}
            \includegraphics[width=\textwidth]{plots/lra/rep/syn-lra/models_compare_LAB_vs_LABELNEG_POL.pdf}%
            \label{fig:plt:syn:lra:rep:models:lab_vs_pol}
        \end{subfigure}\hfill
        \begin{subfigure}[t]{0.29\textwidth}
            \includegraphics[width=\textwidth]{plots/lra/rep/syn-lra/models_compare_LABELNEG_POL_vs_NNF_MUTEX_POL.pdf}%
            \label{fig:plt:syn:lra:rep:models:pol_vs_nnfpol}
        \end{subfigure}\hfill
        \begin{subfigure}[t]{0.29\textwidth}
            \includegraphics[width=\textwidth]{plots/lra/rep/syn-lra/models_compare_LAB_vs_NNF_MUTEX_POL.pdf}%
            \label{fig:plt:syn:lra:rep:models:lab_vs_nnfpol}
        \end{subfigure}\hfill
        \begin{subfigure}[t]{0.29\textwidth}
            \includegraphics[width=\textwidth]{plots/lra/rep/syn-lra/time_compare_LAB_vs_LABELNEG_POL.pdf}%
            \label{fig:plt:syn:lra:rep:time:lab_vs_pol}
        \end{subfigure}\hfill
        \begin{subfigure}[t]{0.29\textwidth}
            \includegraphics[width=\textwidth]{plots/lra/rep/syn-lra/time_compare_LABELNEG_POL_vs_NNF_MUTEX_POL.pdf}%
            \label{fig:plt:syn:lra:rep:time:pol_vs_nnfpol}
        \end{subfigure}\hfill
        \begin{subfigure}[t]{0.29\textwidth}
            \includegraphics[width=\textwidth]{plots/lra/rep/syn-lra/time_compare_LAB_vs_NNF_MUTEX_POL.pdf}%
            \label{fig:plt:syn:lra:rep:time:lab_vs_nnfpol}
            % \end{subfigure}
        \end{subfigure}
        \caption{Results for non-disjoint enumeration. %\TseitinCNF{}, \PlaistedCNF{} and $\NNFna{}+\PlaistedCNF$ reported 168, 95 and 26 timeouts, respectively (points on the dashed lines).
        }%
        \label{fig:plt:syn:lra:rep:scatter}
    \end{subfigure}
    \caption{Set of scatter plots comparing the different CNF-izations on the \smtlarat{} synthetic benchmarks. The first and second rows compare them in terms of size of \TAna{} and execution time, respectively. All the axes are on a logarithmic scale.}%
    \label{fig:plt:syn:lra:scatter}
\end{figure}
%
\begin{figure}
    \centering
    % \begin{subfigure}[t]{\textwidth}
    \begin{subfigure}[t]{\textwidth}
        \begin{subfigure}[t]{0.29\textwidth}
            \includegraphics[width=\textwidth]{plots/lra/no-rep/wmi/models_compare_LAB_vs_LABELNEG_POL.pdf}%
            \label{fig:plt:wmi:norep:models:lab_vs_pol}
        \end{subfigure}\hfill
        \begin{subfigure}[t]{0.29\textwidth}
            \includegraphics[width=\textwidth]{plots/lra/no-rep/wmi/models_compare_LABELNEG_POL_vs_NNF_MUTEX_POL.pdf}%
            \label{fig:plt:wmi:norep:models:pol_vs_nnfpol}
        \end{subfigure}\hfill
        \begin{subfigure}[t]{0.29\textwidth}
            \includegraphics[width=\textwidth]{plots/lra/no-rep/wmi/models_compare_LAB_vs_NNF_MUTEX_POL.pdf}%
            \label{fig:plt:wmi:norep:models:lab_vs_nnfpol}
        \end{subfigure}\hfill
        \begin{subfigure}[t]{0.29\textwidth}
            \includegraphics[width=\textwidth]{plots/lra/no-rep/wmi/time_compare_LAB_vs_LABELNEG_POL.pdf}%
            \label{fig:plt:wmi:norep:time:lab_vs_pol}
        \end{subfigure}\hfill
        \begin{subfigure}[t]{0.29\textwidth}
            \includegraphics[width=\textwidth]{plots/lra/no-rep/wmi/time_compare_LABELNEG_POL_vs_NNF_MUTEX_POL.pdf}%
            \label{fig:plt:wmi:norep:time:pol_vs_nnfpol}
        \end{subfigure}\hfill
        \begin{subfigure}[t]{0.29\textwidth}
            \includegraphics[width=\textwidth]{plots/lra/no-rep/wmi/time_compare_LAB_vs_NNF_MUTEX_POL.pdf}%
            \label{fig:plt:wmi:norep:time:lab_vs_nnfpol}
            % \end{subfigure}
        \end{subfigure}
        \caption{Results for disjoint enumeration. %\TseitinCNF{}, \PlaistedCNF{} and $\NNFna{}+\PlaistedCNF$ reported 24, 23 and 10 timeouts, respectively (points on the dashed lines).
        }%
        \label{fig:plt:wmi:norep:scatter}
    \end{subfigure}
    %%%%%%%%%%%% REP %%%%%%%%%%%%%
    \begin{subfigure}[t]{\textwidth}
        \begin{subfigure}[t]{0.29\textwidth}
            \includegraphics[width=\textwidth]{plots/lra/rep/wmi/models_compare_LAB_vs_LABELNEG_POL.pdf}%
            \label{fig:plt:wmi:rep:models:lab_vs_pol}
        \end{subfigure}\hfill
        \begin{subfigure}[t]{0.29\textwidth}
            \includegraphics[width=\textwidth]{plots/lra/rep/wmi/models_compare_LABELNEG_POL_vs_NNF_MUTEX_POL.pdf}%
            \label{fig:plt:wmi:rep:models:pol_vs_nnfpol}
        \end{subfigure}\hfill
        \begin{subfigure}[t]{0.29\textwidth}
            \includegraphics[width=\textwidth]{plots/lra/rep/wmi/models_compare_LAB_vs_NNF_MUTEX_POL.pdf}%
            \label{fig:plt:wmi:rep:models:lab_vs_nnfpol}
        \end{subfigure}\hfill
        \begin{subfigure}[t]{0.29\textwidth}
            \includegraphics[width=\textwidth]{plots/lra/rep/wmi/time_compare_LAB_vs_LABELNEG_POL.pdf}%
            \label{fig:plt:wmi:rep:time:lab_vs_pol}
        \end{subfigure}\hfill
        \begin{subfigure}[t]{0.29\textwidth}
            \includegraphics[width=\textwidth]{plots/lra/rep/wmi/time_compare_LABELNEG_POL_vs_NNF_MUTEX_POL.pdf}%
            \label{fig:plt:wmi:rep:time:pol_vs_nnfpol}
        \end{subfigure}\hfill
        \begin{subfigure}[t]{0.29\textwidth}
            \includegraphics[width=\textwidth]{plots/lra/rep/wmi/time_compare_LAB_vs_NNF_MUTEX_POL.pdf}%
            \label{fig:plt:wmi:rep:time:lab_vs_nnfpol}
            % \end{subfigure}
        \end{subfigure}
        \caption{Results for non-disjoint enumeration. %\TseitinCNF{}, \PlaistedCNF{} and $\NNFna{}+\PlaistedCNF$ reported 24, 24 and 10 timeouts, respectively (points on the dashed lines).
        }%
        \label{fig:plt:wmi:rep:scatter}
    \end{subfigure}
    \caption{Set of scatter plots comparing the different CNF-izations on the WMI benchmarks. The first and second rows compare them in terms of size of \TAna{} and execution time, respectively. All the axes are on a logarithmic scale.}%
    \label{fig:plt:wmi:scatter}
\end{figure}
