\subsection{Equivariant Segre number at rank \texorpdfstring{$r=-2$}{Lg}} \label{sec:chern-rank-2}
We shall compute the explicit expression for the equivariant (non-virtual) Chern series at rank $r=2$ for the Hilbert schemes. First recall the Chern limit from Proposition \ref{prop:chern-ver-limit},
\equanum{\label{eqn:chern-ver-limit}I^{\mathcal{C}}(V;q)&=\lim_{\e\->0}\Omega\left(-q\e^{2-r}(1+\e)^r;\frac{e^{-\e w_1}}{1+\e},\dots ,\frac{e^{-\e w_r}}{1+\e};e^{\e \lambda_1},e^{\e \lambda_2}\right).
}
By definition, the Chern number $[q^n]I^{\mathcal{C}}(V;q)$ of any rank 2 equivariant bundle $V$ has total degree $-2n$ to $0$ in $\lambda_1,\lambda_2$. Thus by comparing coefficients, we see the positive degree terms in (\ref{eqn:log-total}) must vanish after taking this limit. The following lemma, based on a similar statement mentioned in \cite[ยง4.6]{GM}, allows us to compute the remaining negative degree coefficients 
\[H_{(0),-1,-1}(q,z), H_{(1),-1,-1}(q,z), H_{(0),-1,0}(q,z)\]
from the degree 0 coefficients given by (\ref{eqn:deg0}).

\begin{lemma}\label{lem:differential}
Let $r\geq 0$ and suppose $H(z_1,\dots,z_r)$ is a power series in $z_1,\dots z_r$ whose coefficients are series in some other variables $q_1,q_2,\dots$. If $H$ is symmetric in $z_1,\dots,z_r$ with expansion
\[H(ze^{x_1},\dots,ze^{x_r})=\sum_{\substack{\mu\text{ partition}}}H_{\mu}(z)\prod_{i=1}^{\ell (\mu)}e_{\mu_i}(x_1,\dots,x_r),\]
then for any $k\geq 0$, we have
\[D_z^kH_{(0)}(z)=k!\sum_{|\mu|=k}\binom{r}{\mu}H_{\mu}(z)\]
where $\binom{r}{\mu}$ denotes $\prod_{i=1}^{\ell(\mu)}\binom{r}{\mu_i}$, and $D_z=z\frac{\partial}{\partial z}$.
\end{lemma}
\begin{proof}
We begin by claiming that the statement is closed under polynomial expressions; that is, if the equality holds for both $F(z_1,\dots,z_r)$ and $G(z_1,\dots,z_r)$, then it holds for $F\cdot G$ and  $aF+G$ for any $a\in\QQ[\![q_1,q_2,\dots]\!]$. The additive part is straightforward, and we shall prove the multiplicative part of this claim. Expand 
\equa{F(ze^{x_1},\dots ,ze^{x_r})=\sum_{\mu\text{ partition}}F_\mu(z) e_\mu(x_1,\dots,x_r),\\
G(ze^{x_1},\dots ,ze^{x_r})=\sum_{\mu\text{ partition}}G_\mu(z) e_\mu(x_1,\dots,x_r),
}
then $H=F \cdot G$ can be expanded as
\[H(ze^{x_1},\dots ,ze^{x_r})=\sum_{\mu\text{ partition}}H_\mu(z) e_\mu(x_1,\dots,x_r)=\sum_{\nu+\xi=\mu}F_\nu(z) G_\xi(z) e_\mu(x_1,\dots,x_r)\]
where by $\nu+\xi$ we mean combining them as sequences to get a partition of size $|\nu|+|\xi|$ with length $\ell(\nu)+\ell(\xi)$. Suppose the statement holds for both $F$ and $G$, then we have
\equa{D_z^kH_{(0)}(z)&=D_z^k\left(F_{(0)}(z)G_{(0)}(z)\right)\\
&=\sum_{i=1}^k\binom{k}{i}D_z^iF_{(0)}D_z^{k-i}G_{(0)}\\
&=\sum_{i=1}^k\binom{k}{i}i!(k-i)!\sum_{|\nu|=i,|\xi|=k-i}\binom{r}{\nu}F_{\nu}\binom{r}{\xi}G_{\xi}\\
%&=k!\sum_{\nu,\xi,|\nu|+|\xi|=k}\binom{r}{\nu+\xi}F_{\nu}G_{\xi}\\
&=k!\sum_{|\mu|=k}\binom{r}{\mu}H_{\mu}.
}

Since $H(z_1,\dots ,z_r)$ is symmetric, by the above observation, it suffices to prove the statement when $H$ is the power sum symmetric polynomial $p_n(z_1,\dots ,z_r)=z_1^n+\dots +z_r^n$. For each $n\geq 0$, we expand
\equa{H(ze^{x_1},\dots ,ze^{x_r})=p_n(ze^{x_1},\dots ,ze^{x_r})&=\sum_{j=1}^rz^ne^{nx_j}=z^n\left(r+\sum_{i>0}\frac{n^i}{i!}p_i(x_1,\dots ,x_r)\right).}
This means $H_{(0)}(z)=rz^n$ and 
\[D_z^kH_{(0)}(z)=rn^kz^n.\]

Fix $r\geq 1$, we write
\[p_n(x_1,\dots ,x_r)=\sum_{|\mu|=n}C_\mu e_\mu(x_1,\dots ,x_r)\]
for some constant terms $C_\mu$. Evaluate at $x_1=\dots=x_r=1$ and get
\[r=\sum_{|\mu|=n}\binom{r}{\mu}C_\mu.\]
\begin{comment}

Substitute this into (\ref{pow-sum-expansion}) and obtain for any $k\geq 1$, $|\mu|=k$,
\[H_{\mu}(z)=z^n\frac{n^k}{k!}C_\mu.\] 
We shall use the following Newton's identities of symmetric polynomials. For $r, n\geq 1$,
\equanum{\label{newton1}p_n(x_1,\dots ,r_r)&=(-1)^{n-1}ne_n(x_1,\dots ,x_r)+\sum_{i=1}^{n-1}(-1)^{i-1}e_{i}(x_1,\dots ,x_r)p_{n-i}(x_1,\dots ,x_r).}
Suppose for an induction that for any $1\leq k\leq n$,
\[\sum_{|\nu|=k}\binom{r}{\nu}C_\nu=r.\]
\AC{I can prove this directly from the definition without all of the computations above. Use that $e_{\mu}(1,\ldots,1) = {r\choose \mu}$ and plug it into the defining equation. Using $p_n(1,\ldots,1)=r$ you obtain the result.}

The base case of this induction is the trivial case $n=1$. Identity (\ref{newton1}) gives us
\equa{p_n=(-1)^{n-1}ne_n+\sum_{i=1}^{n-1}(-1)^{i-1}e_{i}\sum_{|\mu|=n-i}C_\mu e_\mu.}
By comparing coefficients, we get
\AC{You are not comparing coefficients your are evaluating at $x_i = 1$ for all $i$ right?}
\equa{\sum_{|\mu|=n}\binom{r}{\mu}C_\mu&=(-1)^{n-1}n\binom{r}{n}+\sum_{i=1}^{n-1}(-1)^{i-1}\binom{r}{i}\sum_{|\nu|=n-i}\binom{r}{\nu}C_\nu\\
&=(-1)^{n-1}r\binom{r-1}{n-1}+\sum_{i=1}^{n-1}(-1)^{i-1}\binom{r}{i}r\\
&=r\cdot\left((-1)^{n-1}\binom{r-1}{n-1}+\sum_{i=1}^{n-1}(-1)^{i-1}\binom{r}{i}\right)\\
&=r
}
where the last equality is a standard property of binomial coefficients. This finishes the induction. 
\end{comment}
Hence
\[k!\sum_{|\mu|=k}\binom{r}{\mu}H_\mu(z)=z^nn^k\sum_{|\mu|=k}\binom{r}{\mu}C_\mu=rn^kz^n=D_z^kH_{(0)}(z).\]
A quick calculation for the $k=0$ or $r=0$ cases finishes the proof.

\end{proof}

\begin{comment}
\begin{lemma}\label{lem:differential}
Suppose $r\geq 0$ and $H(q;z_1,\dots ,z_r)$ is a power series symmetric in $z_1,\dots ,z_r$ with the following expansion:
\[H(q;ze^{x_1},\dots ,ze^{x_r})=\sum_{\substack{\mu\text{ partition}}}H_{\mu}(q,z)\prod_{i=1}^{\text{length }{\mu}}e_{\mu_i}(x_1,\dots ,x_r).\]
Then we have
\[D_zH_{(0)}(q,z)=rH_{(1)}(q,z),\]
\[D_z^2H_{(0)}(q,z)=2r^2H_{(1,1)}(q,z)+2\binom{r}{2}H_{(2)}(q,z).\]
where $D_z=z\frac{\partial}{\partial z}$.
\end{lemma}
\begin{proof}
Write 
\[H(q;z_1,\dots ,z_r)=\sum_{\mu}h_\mu(q)\prod_{i=1}^{\text{length }{\mu}}e_{\mu_i}(z_1,\dots ,z_r).\]
Then 
\[H(q;ze^{x_1},\dots ,ze^{x_r})=\sum_{\mu}h_\mu(q)z^{|\mu|}\prod_{i=1}^{\text{length }{\mu}}e_{\mu_i}(e^{x_1},\dots ,e^{x_r}).\]
Expand $e_{i}(e^{x_1},\dots ,e^{x_r})$ and get
\equa{e_{i}(e^{x_1},\dots ,e^{x_r})=&\sum_{j_1,\dots ,j_i}\sum_{n=0}^\infty \frac{(x_{j_1}+\dots +x_{j_i})^n}{n!}\\
=&\binom ri+\binom{r-1}{i-1}e_1(x_1,\dots ,x_r)+\frac12\binom{r-1}{i-1}e_1(x_1,\dots .,x_r)^2\\
&+\left(\binom{r-2}{i-2}-\binom{r-1}{i-1}\right)e_2(x_1,\dots ,x_r)+\dots 
}
where the terms whose total degree in $x_1,\dots ,x_r$ is greater than 2 are omitted. Substituting and comparing coefficients we get
\[H_{(0)}(q,z)=\sum_{\mu}h_\mu(q)z^{|\mu|}\prod_{i=1}^{\text{length }{\mu}}\binom r {\mu_i},\]
\equa{H_{(1)}(q,z)&=\sum_{\mu\neq (0)}h_\mu(q)z^{|\mu|}\sum_{i}\binom{r-1}{\mu_i-1}\prod_{j\neq i}\binom r{ \mu_j}\\
&=\frac{1}r\sum_{\mu}|\mu|h_\mu(q)z^{|\mu|}\prod_{i}\binom{r}{\mu_i}=\frac1rD_zH_{(0)}.
}
This proves the first identity. We also have
\equa{H_{(2)}(q,z)&=\sum_{\mu\neq (0)}h_\mu(q)z^{|\mu|}\sum_{i}\left(\binom{r-2}{\mu_i-2}-\binom{r-1} {\mu_i-1}\right)\prod_{j\neq i}\binom{r}{\mu_j}\\
&=\sum_{\mu\neq (0)}h_\mu(q)z^{|\mu|}\sum_{i}\left(\frac{\mu_i(\mu_i-1)}{r(r-1)}-\frac{\mu_i}{r}\right)\prod_{i}\binom{r}{\mu_i},
}
\equa{H_{(1,1)}(q,z)&=\sum_{\mu\neq (0)}h_\mu(q)z^{|\mu|}\left(\sum_{i}\frac12\binom{r-1}{\mu_i-1}\prod_{j\neq i}\binom{r}{\mu_j}+\frac12\sum_{i\neq j}\binom{r-1}{\mu_i-1}\binom{r-1}{\mu_j-1}\prod_{\ell\neq i,j}\binom{r}{\mu_\ell}\right)\\
&=\sum_{\mu\neq (0)}h_\mu(q)z^{|\mu|}\left(\left(\sum_i\frac{\mu_i}{2r}+\sum_{i\neq j}\frac{\mu_i\mu_j}{2r^2}\right)\prod_{i}\binom{r}{\mu_i}\right),
}
and therefore,
\equa{2r^2H_{(1,1)}+2\binom r2H_{(2)}&=\sum_{\mu\neq (0)}h_\mu(q)z^{|\mu|}\left(\sum_{i\neq j}\left(
\mu_ir-\mu_i(r-1)+\mu_i\mu_j+\mu_i^2-\mu_i
\right)\prod_{i}\binom{r}{\mu_i}\right)\\
&=\sum_{\mu\neq (0)}|\mu|^2h_\mu(q)z^{|\mu|}\prod_{i}\binom r{\mu_i}=D_z^2H_{(0)}.
}


\end{proof}
\end{comment}


We would like to apply the above lemma to the series from (\ref{eqn:deg0}). First, using the admissibility of $\Omega$ combined with an expansion as used in (\ref{eqn:log-partition-E}), we obtain 
\[\log\Omega(q;z_1,\dots,z_r;e^{-\lam_1},e^{-\lam_2})=\sum_{\substack{k_1,k_2\geq -1}}G_{k_1,k_2}(q;z_1,\dots,z_r)\int_SE_{k_1,k_2}(c_1(S),c_2(S))\]
for some series $G_{k_1,k_2}(q;z_1,\dots,z_r)$. Comparing to (\ref{eqn:log-total}), we see
\[G_{k_1,k_2}(q;ze^{w_1},\dots,ze^{w_r})=\sum_{\mu\text{ partition} }(-1)^{k_1+k_2}H_{\mu,k_1,k_2}(q,z)c_\mu(V)\]
Apply Lemma \ref{lem:differential}, where we set $H(z_1,\dots,z_r)$ in the lemma to be $G_{k_1,k_2}(q;z_1,\dots,z_r)$ and the variables $x_1,\dots,x_r$ to be $w_1,\dots w_r$, we conclude 
\[D_z^kH_{(0),k_1,k_2}(q,z)=k!\sum_{|\mu|=k}\binom{r}{\mu}H_{\mu,k_1,k_2}(q,z).\]
When $r=2$, the series $H_{(2),-1,-1}, H_{(1,1),-1,-1}$ and $H_{(1),-1,0}$ are known explicitly by (\ref{eqn:deg0}). This allows us to calculate $H_{(1),-1,-1},H_{(0),-1,-1}$ and $H_{(0),-1,0}$ by taking anti-derivatives using the identities
\[\li_1 =  -\log(1-q),\indent D_z\li_n(qz^k) = k\li_{n-1}(qz^k)\]
for $k,n>0$. They are obtained as follows
\equanum{\label{eqn:H-omega-fomula}H_{(1),-1,-1}(q,z)&=-\li_2(qz^2)+\li_2(qz),\\
H_{(0),-1,-1}(q,z)&=h_{(0),-1,-1}(q)-\li_3(qz^2)+2\li_3(qz),\\
H_{(0),-1,0}(q,z)&=h_{(0),-1,0}(q)+\frac12\li_2(qz^2)-\li_2(qz),\\
}
for some terms $h_{(0),-1,-1}(q),h_{(0),-1,0}(q)$ independent of $z$. By (\ref{eqn:log-total}) and the following lemma, we have 
\equa{h_{(0),-1,-1}(q)&=[\lam^{-2}]\log\Omega(q;0,\dots ,0;e^{\lambda},e^{\lambda})=-\li_3(q),\\
h_{(0),-1,0}(q)&=[\lam^{-1}]\frac12\log\Omega(q;0,\dots ,0;e^{\lambda},e^{\lambda})=\frac12\li_2(q)}
where the factor $\frac12$ in the second line is due to $H_{(0),-1,0}=H_{(0),0,-1}$.
\begin{lemma}
The following identity is satisfied:
\[\log\Omega(Q;0,\dots ,0;e^{\lambda},e^{\lambda})=-\sum_{n=1}^\infty\frac1n\frac{Q^n}{(1-e^{n\lambda})^2}.\]
\end{lemma}
\begin{proof}
By \cite[Theorem~2.3]{GM},
\equa{&\Omega(Q;z_1,\dots ,z_r;q_1,q_2)\\
=&\Exp\left(-\frac{Q+\sum z_i}{(1-q_1)(1-q_2)}\right)\cdot \sum_{\mu}(-1)^{|\mu|}\frac{\tilde{H}_\mu[Q+1;q_1,q_2]\tilde{H}_\mu[z_1+\dots+z_r;q_1,q_2]T_\mu(q_1,q_2)}{N_\mu(q_1,q_2)}.}
Here $T_\mu(q_1,q_2)=\prod_{\square\in\mu}q_1^{c(\square)}q_2^{r(\square)}$, $N_\mu(q_1,q_2)=\prod_{\square\in\mu}(q_1^{a(\square)+1}-q_2^{l(\square)})(q_1^{a(\square)}-q_2^{l(\square)+1})$, and $\tilde{H}_\mu$ is the \emph{modified Macdonald polynomial} defined by \cite[Theorem 1]{Mac-poly}. Evaluating at $z_1=\dots=z_n=0$, the term $\tilde{H}_\mu[z_1+\dots+z_r;q_1,q_2]$ vanishes unless $\mu=(0)$, and when $\mu=(0)$, we have $\tilde{H}_{\mu}=1$. This can be seen from its Schur function expansion \cite[Definition 1]{Mac-poly}
\[\tilde{H}_{\mu}[X;q_1,q_2]=\sum_{|\nu|=|\mu|} s_\nu[X]\tilde{K}_{\mu\nu}(q_1,q_2)\]
where $\tilde{K}_{\mu\nu}$ are the modified Macdonald-Kostka polynomials.
Therefore when $z_1=\dots=z_r=0$, the summation in the above equation evaluates to $1$, and
\[\Omega(Q;0,\dots ,0;q_1,q_2)=\Exp\left(-\frac{Q}{(1-q_1)(1-q_2)}\right)\]
By definition of plethystic exponential, 
\[\log\Omega(Q;0,\dots ,0;q_1,q_2)=-\sum_{n=1}^\infty\frac1n\frac{Q^n}{(1-q_1^n)(1-q_2^n)}.\]
Substituting $q_1=q_2=e^\lambda$ gives the desired form.
\end{proof}

Now we can compute the Chern series. In order to take the limit (\ref{eqn:chern-ver-limit}) of $H_{\mu,k_1,k_2}(q,z)$, we need to substitute $q\leadsto-q\e^{2-r}(1+\e)^r$ and $z\leadsto(1+\e)^{-1}$. In (\ref{eqn:log-total}), the series $H_{\mu,k_1,k_2}$ is multiplied by a homogeneous function of degree $k_1+k_2$ in $\lam_1,\lam_2$, as well as a homogeneous function of degree $|\mu|$ in $w_1,\dots,w_r$. The limit requires us to substitute $\vec\lam\leadsto-\e\vec\lam$ and $\vec w\leadsto-\e \vec w$. Therefore before taking the limit $\e\->0$, we need to multiply by $(-\e)^{|\mu|+k_1+k_2}$. Applying this procedure to (\ref{eqn:deg0}) and (\ref{eqn:H-omega-fomula}), the limit of $H_{(0),-1,-1},H_{(1),-1,-1},H_{(2),-1,-1}$ in the $r=2$ case all return $\log(1+q)$, while the other terms all vanish. Hence (\ref{eqn:chern-ver-limit}) yields
\equanum{\label{eqn:chern-rank-2}I^{\mathcal{C}}(V;q)=&\exp\left(\log(1+q)\int_Sc_0(V)+\log(1+q)\int_Sc_1(V)+\log(1+q)\int_Sc_2(V)\right)\\
=&(1+q)^{\int_Sc(V)}}
for any $\T$-equivariant bundle $V$ of rank 2.



\subsection{Virtual Segre number in rank \texorpdfstring{$r=-1$}{Lg}} \label{sec:vir-chern-rank-1}
Recall that on Hilbert schemes, the obstruction theory at a fixed point $[Z_\mu]$ is given by $(K^{[n]}_S)^\vee|_{Z_\mu}$, so
\[\frac{1}{e(T^\vir_{Z_\mu})}=\frac{e((K_S^{[n]})^\vee|_{Z_\mu})}{e(T_{Z_\mu})} =(-1)^{|\mu|}\frac{e((K_S^{[n]})|_{Z_\mu})}{e(T_{Z_\mu})}.\] 
\begin{comment}
Similar to Proposition \ref{prop:chern-ver-limit}, the virtual Chern series on Hilbert schemes can be extracted from the master partition function as follows
\equanum{\label{eqn:chern-limit}{\mathcal{C}}_S(\O_S,V;q)=\lim_{\e\->0}\Omega\left(q\e^{1-r}(1+\e)^r;\frac{e^{-\e v_1}}{1+\e},\dots,\frac{e^{-\e v_r}}{1+\e},e^{\e c_1(K_S)};e^{\e\lambda_1},e^{\e\lambda_2}\right).
}
Considering $z$ as the weight of a trivial $\CC^*$-action on $S$ and $\hilb^n(S)$, we write $z=e^l$ where $l=c_1(z)$. We shall focus on the case where $V=L=\O_S\<v_1\>$ is a line bundle. Applying the $r=2$ version of (\ref{eqn:log-total}) setting $w_{2}=c_1(K_S)-l$, we obtain the following expansion:
\equa{&\log \Omega\left(q;ze^{c_1(L)},ze^{-c_1(K_S)-l};e^{-\lambda_1},e^{-\lambda_2}\right)\\
=&\lam_1^{-1}\lam_2^{-1}\cdot (H_{(0),-1,-1}+e_1(w_1,-c_1(K_S)-l)H_{(1),-1,-1}\\
&\indent +e_2(w_1,-c_1(K_S)-l)H_{(2),-1,-1}+e_1(w_1,-c_1(K_S)-l)^2H_{(1,1),-1,-1})\\
&+(\lam_1^{-1}+\lam_2^{-1})\cdot\left(H_{(0),-1,0}+e_1(w_1,-c_1(K_S)-l)H_{(1),-1,0}\right)\\
&+(\lam_1^{-1}\lam_2+\lam_1\lam_2^{-1})\cdot H_{(0),-1,1}+H_{(0),0,0}.
}
Similar to the previous section, the series $H_{\mu,k_1,k_2}$ in the right-hand side are already found in (\ref{eqn:deg0}) and (\ref{eqn:H-omega-fomula}), and we would like to take the limit (\ref{eqn:chern-limit}). Make substitutions $q\leadsto q(1+\e), z\leadsto(1+\e)^{-1}, w_1\leadsto-\e w_1, \vec\lam\leadsto-\e \vec \lam$, then take $\e\->0$. Most of the above summands will then vanish or cancel out, and we are left with
\[\log {\mathcal{C}}_S(\O_S,L;q)=\log(1-q)\int_Sc_1(K_S)+\log(1-q)\int_Sc_1(L)c_1(K_S)\]
Therefore
\equa{{\mathcal{C}}_S(\O_S,L;w)=(1-q)^{\int_Sc(L)c_1(K_S)}=\left(\frac1{1-q}\right)^{\int_Sc(L)c_1(S)}.}
\end{comment}
Let $L=\O_S\<v_1\>$ be an equivariant line bundle, and $V=L\oplus\O_S\<v_2\>$. Apply (\ref{eqn:chern-rank-2}) to $V$ and we have
\[I^{\mathcal{C}}(V;q)=(1+q)^{\int_Sc(V)}=(1+q)^{\int_S(1+w_1+w_2+w_1w_2)}.\]
Set $w_2=c_1(K_S)-1$ and replace $q$ by $-q$, then this becomes
\[I^{\mathcal{C}}(V;-q)|_{w_2=c_1(K_S)-1}=(1-q)^{\int_Sc(L)c_1(K_S)}.\]
On the other hand, we have by definition
\equa{&I^{\mathcal{C}}(V;-q)|_{w_2=c_1(K_S)-1}\\
=&\sum_{\mu} (-1)^{|\mu|}q^{|\mu|}\prod_{\square\in\mu}\frac{(1+w_1-c(\square)\lam_1-r(\square)\lam_2)(c_1(K_S)-c(\square)\lam_1-r(\square)\lam_2)}{((a(\square)+1)\lambda_1-l(\square)\lambda_2)((l(\square)+1)\lambda_2-a(\square)\lambda_1)}\\
=&\sum_{\mu}(-1)^{|\mu|}q^{|\mu|}\frac{c(L^{[n]}|_{Z_\mu})e((K_S^{[n]})|_{Z_\mu})}{e(T|_{Z_\mu})}\\
=&\sum_{\mu}q^{|\mu|}\frac{c(L^{[n]}|_{Z_\mu})}{e(T^\vir|_{Z_\mu})}=\mathcal{C}_S(\O_S,L;q)
}
Therefore we conclude
\equa{{\mathcal{C}}_S(\O_S,L;w)=(1-q)^{\int_Sc(L)c_1(K_S)}=\left(\frac1{1-q}\right)^{\int_Sc(L)c_1(S)}.}
\begin{comment}
\AC{Here is a shorter proof of the above:
Start by noting that $c(e^uK_S^{[n]}) = (1+u)^nc_{(1+u)^{-1}}(K_S^{[n]})$ so we have that 
$$
\sum_{n\geq 0}q^n\int_{\hilb} c(L^{[n]}) c_{n}(K_S^{[n]}) = \sum_{n\geq 0}q^n\int_{\hilb} c(L^{[n]}) c(e^uK_S^{[n]})|_{c(e^u)=0}q,.
$$
Since the first left-hand side is equal to $(1+q)^{c(L)\cdot\big(c(e^u)+c_1(K_S)\big)}$, setting $c(e^u)$ equal to zero gives us the required result.
}
\end{comment}
In particular, restricting to the lowest degree part in the variables $\lam_1,\lam_2,w_1$, we obtain the following Corollary.
\begin{corollary}\label{cor:nek2d}For $S=\CC^2$, the following equality holds
\[\sum_{n=1}^\infty q^n\int_{[\hilb^n(S)]^\vir}1:=\sum_{Z\in\hilb^n(S)^\T}\frac{1}{e(T^\vir_Z)}=e^{\frac{(\lambda_1+\lambda_2)}{\lambda_1\lambda_2}q}.\]
\end{corollary}


\subsection{Segre-Verlinde correspondence in non-zero degrees}\label{sec:reduced-computation} \input{2.2new-computation}


\subsection{Strong Segre symmetry and weak Verlinde symmetry}\label{sec:sym}
Let $r>0$. According to Theorem \ref{thm:SV2d-deg-pos}, the following identity holds for the Segre series
\equa{&[q^n]\sum_{|\mu|=k}\binom{r}{\mu}\log A^{r,N}_{\mu,(0),(0)}((-1)^Nq)=[q^n]\sum_{|\xi|=k}\binom{N}{\xi}\log A^{r,N}_{(0),(0),\xi}((-1)^Nq)\\
=&(-1)^{nN-1}\frac{r}{n}(-n(r+N))_{(k-1)}\binom{-nr-1}{nN-1}\\
=&(-1)^{nN-1}\frac{r}{n}\cdot\frac{(-nr-1)\cdots (-n(r+N)-k+2)}{(nN-1)!}\\
=&(-1)^{k-1}rN\cdot(n(r+N)+k-2)_{(k-2)}\binom{n(r+N)}{nN}
}
The right-hand side does not change if we swap $r$ and $N$, that is
\equa{\sum_{|\mu|=k}\binom{r}{\mu}\log A^{r,N}_{\mu,(0),(0)}((-1)^Nq)=\sum_{|\mu|=k}\binom{r}{\mu}\log A^{N,r}_{(0),(0),\mu}((-1)^rq).}
This is consistent with the strong Segre symmetry of Conjecture \ref{con:strong-sym}.

As for the Verlinde series, the weak Segre symmetry of Corollary \ref{cor:sv-sym2d-intro} together with the weak Segre-Verlinde correspondence of Corollary \ref{cor:weak-SV2d-virtual-intro} would imply a weak Verlinde symmetry. However, calculations using a computer program show the ``strong'' Verlinde symmetry does not hold for $S=\CC^2$. This can also be observed from the fact that the equivariant Verlinde series only depends on $V$ through $c_1(V)$ but depends on $E$ through $c_1(E),c_2(E),\dots,c_N(E)$.