\section{Evaluation of matrices in Wanier gauge}
\secl{wannier-gauge}

%\stm{we may comment out the middle line of each subequation}

\beas{Oww-2}
\left(A\ww\right)^{a}_{ij}&\equiv&  i\ip{ u_i\ww}{\partial_a u_j\ww}  \nonumber\\ 
%   &=& \sum_\mathbf{R} e^{i\kk(\R+\bt_j-\bt_i)}\memnR{\hat{r}_a-\RR-\bt_j } = \nonumber \\
    &=&  e^{i\kk(\bt_j-\bt_i)}\sum_\mathbf{R} e^{i\kk\R}  \mathbb{A}^a_{ij}(\RR) \eql{Aww-2}  \\
%
\left(B\ww\right)^{a}_{ij}&\equiv&  i\me{ u_i\ww}{\Ham}{\partial_a u_j\ww} \nonumber\\
% &=& \sum_\mathbf{R} e^{i\kk(\R+\bt_j-\bt_i)}\memnR{\Ham\cdot(\hat{r}_a-\RR-\bt_j) } = \nonumber\\
 &=& e^{i\kk(\bt_j-\bt_i)}\sum_\mathbf{R} e^{i\kk\mathbf{R}}\mathbb{B}^a_{ij}(\RR)  \eql{Bww-2} \\
%
\Hwan^{ab}_{ij}&\equiv&  \me{\partial_a u_i\ww}{\Ham}{\partial_b u_j\ww} \nonumber\\ 
%   &=& \sum_\mathbf{R} e^{i\kk(\R+\bt_j-\bt_i)}\memnR{(\hat{r}_a-\bt_i)\cdot \Ham\cdot(\hat{r}_a-\RR-\bt_j) } = \nonumber\\
 &=& e^{i\kk(\bt_j-\bt_i)}\sum_\mathbf{R} e^{i\kk\mathbf{R}}\mathbb{C}^a_{ij}(\RR)  \eql{Hww-2} \\
%
\Fwan^{ab}_{ij}&\equiv&  \ip{\partial_a u_i\ww}{\partial_b u_j\ww}  \nonumber\\ 
 &=& e^{i\kk(\bt_j-\bt_i)}\sum_\mathbf{R} e^{i\kk\mathbf{R}}\mathbb{F}^{ab}_{ij}(\RR)  \eql{Fww-2} 
\eeas
\stm{is it ok to have $\Hwan$ expressed through $\mathbb{C}$ and not $\mathbb{H}$}
Where
%
\beas{O-R}
\mathbb{A}^a_{ij}(\RR)    & =& \memnR{\hat{r}_a-t_j^a } \\
\mathbb{B}^a_{ij}(\RR)    & =& \memnR{\Ham \cdot(\hat{r}_a-\hat{R}_a -t_j^a)}\\
\mathbb{C}^{ab}_{ij}(\RR) & =& \memnR{(\hat{r}_a-t_i^a)\cdot \Ham \cdot (\hat{r}_b-t_j^a-\hat{R}_b ) }\\
\mathbb{F}^{ab}_{ij}(\RR) & =& \memnR{(\hat{r}_a-t_i^a)\cdot (\hat{r}_b-t_j^b-\hat{R}_b ) }
\eeas
%
These matrix elements can be computed 
using finite-difference schemes based on the ab initio bandstructures computed on regular $\kk$-grids --- 
a procedure that is widely described in the literature \cite{marzari-prb97,wang-prb06,lopez-prb12, Ryoo-SHC}
\stm{should we expand a bit about that?}

And  the derivatives will be evaluated as 
\begin{multline}
\partial_d\left(\cal{O}\ww\right)_{ij} 
  = i e^{i\kk(\bt_j-\bt_i)}  \sum_\mathbf{R} e^{i\kk\mathbf{R}}  \mathbb{O}_{ij}(\RR) (R_d+t_j^d-t_i^d) \\
    =  i(t_j^d-t_i^d)\left(\cal{O}\ww\right)_{ij} + i e^{i\kk(\bt_j-\bt_i)}  \sum_\mathbf{R} e^{i\kk\mathbf{R}}  \mathbb{O}_{ij}(\RR) R_d
\eql{Awwad}  \\
\end{multline}

%\beas{Oww-der}
%\partial_d\left(A\ww\right)^{a}_{ij} & = &i\sum_\mathbf{R} e^{i\kk\mathbf{R}}  \mathbb{A}^a_{ij}(\RR) (R_d+t_j^d-t_i^d)\eql{Awwad}  \\
%\partial_d\left(B\ww\right)^{a}_{ij}  &= & i\sum_\mathbf{R} e^{i\kk\mathbf{R}}\mathbb{B}^a_{ij}(\RR) (R_d+t_j^d-t_i^d) \eql{Bwwad} \\
%\partial_d\Hwan^{ab}_{ij} &= &i\sum_\mathbf{R} e^{i\kk\mathbf{R}}\mathbb{C}^{ab}_{ij}(\RR) (R_d+t_j^d-t_i^d)\eql{Hwwabd} \\
%\partial_d\Hwan^{c}_{ij} &= & i\sum_\mathbf{R} e^{i\kk\mathbf{R}}\mathbb{C}^c_{ij}(\RR) (R_d+t_j^d-t_i^d)\eql{Hwwcd} \\
%\partial_d\Fwan^{ab}_{ij} & = & i\sum_\mathbf{R} e^{i\kk\mathbf{R}} \mathbb{F}^{ab}_{ij}(\RR) (R_d+t_j^d-t_i^d) \eql{Fwwabd}\\
%\partial_d\left(\Omega\ww  \right)^{c}_{ij}& = &\abc\sum_\mathbf{R} e^{i\kk\mathbf{R}}\mathbb{A}^a_{ij}(\RR) \hat{R}_b (R_d+t_j^d-t_i^d)\eql{Owwcd}
%\eeas


%%% Local Variables:
%%% mode: latex
%%% TeX-master: "pap"
%%% End:
