\section{The Known Examples}
Before proving that $3C(\al,1-\al)$ and $Q_2(\frac{1}{3})$ are the only two examples (up to isomorphism) of these $2$-generated primitive axial algebras of Monster type with skew axet $X'(1+2)$, it would be useful to indeed show that they satisfy the conditions we desire. 
\subsection{$3C(\al,1-\al)$}
First, let $A=3C(\al,1-\al)$ with $\al\notin \{\frac{1}{2},-1\}$. In \cite{mcinroy2022axial} and \cite{franchi20212}, this example has already been stated. Let $x,y,z$ be distinct axes of $\mcal{J}(\al)$-type.  Note that as $\al\neq-1$, there is an identity in $A$ of $\id=\frac{1}{\al+1}(x+y+z)$. Letting $w=\id-x$, one can see that $w$ is an axis of $\mcal{J}(1-\al)$-type. Notice 
\[ \id=\frac{1}{\al+1}(\id-w+y+z)\]
and so
\[\al\id=(-w+y+z).\]
Further,
\begin{eqnarray*}
wy &=& (\id-x)y = y-\frac{\al}{2}(x+y-z)\\
&=& y-\frac{\al}{2}\left(\frac{1}{\al}[-(\al+1)w+y+z] + y-z\right)\\
&=& y-\frac{1}{2}[-(\al+1)w+y+z] - \frac{\al}{2}(y-z) = \frac{\al+1}{2}w+\frac{1-\al}{2}y-\frac{1-\al}{2}z
\end{eqnarray*}
Hence $z\in \GenA{w,y}$ and $x$ is too. Therefore $A=\GenA{w,y}$. As $A$ is now of $\mcal{M}(\al,1-\al)$-type, let the Miyamoto involution of $w$ and $y$ be $\tau_w$ and $\tau_y$ respectively. As $y$ is of $\mcal{J}(\al)$-type, $\tau_y$ is the identity. On the other hand, one can check that $x\in A_0(w)$ and $y-z\in A_{1-\al}(w)$. Further,
\[ y = \frac{\al}{2}x + \frac{\al+1}{2}w +\frac{1}{2}(y-z)\]
and so
\[ y^{\tau_w}=\frac{\al+1}{2}w+\frac{\al}{2}x -\frac{1}{2}(y-z) =z.\]
Therefore $A$ is skew with axet $X'(1+2)$.

\subsection{$Q_2(\frac{1}{3})$}
Let $A=Q_2(\frac{1}{3})$ be defined as in \cite{galt2021double} with $\eta=\frac{1}{3}$. The algebra can be spanned by two single axes, $s_1$ and $s_2$, and two double axes, $d_1$ and $d_2$ with the multiplication defined in Table \ref{mult Q}.
\begin{table}[b]
\begin{center}
    \begin{tabular}{c|c|c|c|c}
         & $s_1$ & $s_2$ & $d_1$ &$d_2$   \\
         \hline
        $s_1$ & $s_1$ &$0$& $\frac{1}{3}s_1+\frac{1}{6}d_1-\frac{1}{6}d_2$& $\frac{1}{3}s_1-\frac{1}{6}d_1+\frac{1}{6}d_2$\\
        \hline
        $s_2$ & & $s_2$ & $\frac{1}{3}s_2+\frac{1}{6}d_1-\frac{1}{6}d_2$& $\frac{1}{3}s_2-\frac{1}{6}d_1+\frac{1}{6}d_2$\\
        \hline
        $d_1$ &  &  & $d_1$&$-\frac{1}{3}s_1-\frac{1}{3}s_2+\frac{1}{3}d_1+\frac{1}{3}d_2$ \\
        \hline
        $d_2$ &  &  &  & $d_2$
    \end{tabular}
       \caption{The multiplication table of $Q_2(\frac{1}{3})$}
       \label{mult Q}
       \end{center}
\end{table}
Notice that the identity for $A$ is $\id = \frac{3}{5}(s_1+s_2+d_1+d_2)$ and  $s_1$ is $\jor{\frac{1}{3}}$-axis while $d_1$ is $\mon{\frac{2}{3},\frac{1}{3}}$-axis. Let $t_1:=\id-d_1$ and $t_2:=\id -d_2$ which are axes with fusion law $\mcal{M}(\frac{1}{3},\frac{2}{3})$. We have that 
\[ s_1t_1 = s_1(\id -d_1)=s_1-\frac{1}{3}s_1-\frac{1}{6}d_1+\frac{1}{6}d_2 = \frac{2}{3}s_1-\frac{1}{6}d_1+\frac{1}{6}d_2= \frac{2}{3}s_1-\frac{1}{6}t_1+\frac{1}{6}t_2.\]
Therefore $t_2\in \GenA{s_1,t_1}$. Further,
\[ \frac{5}{3}\id = s_1+s_2+d_1+d_2= s_1+s_2-(\id - d_1)-(\id-d_2)+2\id= s_1+s_2-t_1-t_2+2\id\]
Hence $-\frac{1}{3}\id = s_1+s_2-t_1-t_2$. We have
\begin{eqnarray*}t_1t_2 = (\id-d_1)(\id-d_2) &=& \id -d_1-d_2+d_1d_2\\
&=& \id -\frac{1}{3}s_1-\frac{1}{3}s_2-\frac{2}{3}d_1-\frac{2}{3}d_2\\
&=& \id -\frac{1}{3}s_1-\frac{1}{3}s_2+\frac{2}{3}(\id-d_1)+\frac{2}{3}(\id-d_2)-\frac{4}{3}\id\\
&=&-\frac{1}{3}\id -\frac{1}{3}s_1-\frac{1}{3}s_2+\frac{2}{3}t_1+\frac{2}{3}t_2\\
&=& s_1+s_2-t_1-t_2 -\frac{1}{3}s_1-\frac{1}{3}s_2+\frac{2}{3}t_1+\frac{2}{3}t_2\\
&=& \frac{2}{3}s_1+\frac{2}{3}s_2-\frac{1}{3}t_1-\frac{1}{3}t_2.
\end{eqnarray*}
Hence $s_2$ and $\id$ are in $\GenA{s_1,t_1}$. Therefore $d_1,d_2\in \GenA{s_1,t_1}$ and so $A=\GenA{s_1,t_1}$. As $s_1$ is a $\jor{\frac{1}{3}}$-axis, $\tu{{s_1}}$ is the identity map.  The reader can check that:
\begin{itemize}
    \item $t_1 \in A_1(t_1)$,
    \item $d_1 \in A_0(t_1)$, 
    \item $s_1+s_2-d_2 \in A_\frac{1}{3}(t_1)$, and
    \item $s_1-s_2 \in  A_\frac{2}{3}(t_1)$.
\end{itemize}
Hence
\[s_1 = \frac{5}{12}t_1+\frac{1}{6}d_1+\frac{1}{4}(s_1+s_2-d_2)+\frac{1}{2}(s_1-s_2)=\frac{1}{2}(s_1+s_2)+\frac{1}{2}(s_1-s_2),\]
with $\frac{1}{2}(s_1+s_2)\in A_{\{0,1,\frac{1}{3}\}}(t_1)$. Therefore
\[ s_1^{\tu{t_1}} = \frac{1}{2}(s_1+s_2)-\frac{1}{2}(s_1-s_2)=s_2.\]
Therefore $A$ is skew with axet $X'(1+2)$.
