
\subsection{Virtual Segre number in rank \texorpdfstring{$r=-1$}{Lg}} \label{sec:chern-rank-2}
We shall compute the explicit expression for the Chern series at rank $r=1$ for Hilbert schemes. To begin, we consider the non-virtual Chern series for rank $r=2$, which is known to have universal series structure as a result of \cite[(2.6)]{GM}. By definition, the non-virtual Chern number $[q^n]I^{\mathcal{C}}(V;q)$ of any rank 2 equivariant bundle $V$ has total degree $-2n$ to $0$ in $\lambda_1,\lambda_2$. Comparing coefficients, we see the positive degree terms must vanish. By a non-virtual version of the argument of Section \ref{sec:proj-reduction}, the degree 0 terms are given by taking the Chern limit \cite[Proposition 3.4]{GM} of the expressions \cite[(3.16)]{GM}.

The following lemma, based on a similar statement mentioned in \cite[ยง4.6]{GM}, allows us to compute the remaining negative degree terms using these degree 0 terms. At last, we obtain
\equanum{\label{eqn:chern-rank-2}I^{\mathcal{C}}(V;q)=&\exp\left(\log(1+q)\int_Sc_0(V)+\log(1+q)\int_Sc_1(V)+\log(1+q)\int_Sc_2(V)\right)\\
=&(1+q)^{\int_Sc(V)}}
for any $\T$-equivariant bundle $V$ of rank 2.

\begin{lemma}\label{lem:differential}
Let $r\geq 0$ and suppose $H(z_1,\dots,z_r)$ is a power series in $z_1,\dots z_r$ whose coefficients are series in some other variables $q_1,q_2,\dots$. If $H$ is symmetric in $z_1,\dots,z_r$ with expansion
\[H(ze^{x_1},\dots,ze^{x_r})=\sum_{\substack{\mu\text{ partition}}}H_{\mu}(z)\prod_{i=1}^{\ell (\mu)}e_{\mu_i}(x_1,\dots,x_r),\]
then for any $k\geq 0$, we have
\[D_z^kH_{(0)}(z)=k!\sum_{|\mu|=k}\binom{r}{\mu}H_{\mu}(z)\]
where $\binom{r}{\mu}$ denotes $\prod_{i=1}^{\ell(\mu)}\binom{r}{\mu_i}$, and $D_z=z\frac{\partial}{\partial z}$.
\end{lemma}
\begin{proof}
We begin by claiming that the statement is closed under polynomial expressions; that is, if the equality holds for both $F(z_1,\dots,z_r)$ and $G(z_1,\dots,z_r)$, then it holds for $F\cdot G$ and  $aF+G$ for any $a\in\QQ[\![q_1,q_2,\dots]\!]$. The additive part is straightforward, and we shall prove the multiplicative part of this claim. Expand 
\equa{F(ze^{x_1},\dots ,ze^{x_r})=\sum_{\mu\text{ partition}}F_\mu(z) e_\mu(x_1,\dots,x_r),\\
G(ze^{x_1},\dots ,ze^{x_r})=\sum_{\mu\text{ partition}}G_\mu(z) e_\mu(x_1,\dots,x_r),
}
then $H=F \cdot G$ can be expanded as
\[H(ze^{x_1},\dots ,ze^{x_r})=\sum_{\mu\text{ partition}}H_\mu(z) e_\mu(x_1,\dots,x_r)=\sum_{\nu+\xi=\mu}F_\nu(z) G_\xi(z) e_\mu(x_1,\dots,x_r)\]
where by $\nu+\xi$ we mean combining them as sequences to get a partition of size $|\nu|+|\xi|$ with length $\ell(\nu)+\ell(\xi)$. Suppose the statement holds for both $F$ and $G$, then we have
\equa{D_z^kH_{(0)}(z)&=D_z^k\left(F_{(0)}(z)G_{(0)}(z)\right)\\
&=\sum_{i=1}^k\binom{k}{i}D_z^iF_{(0)}D_z^{k-i}G_{(0)}\\
&=\sum_{i=1}^k\binom{k}{i}i!(k-i)!\sum_{|\nu|=i,|\xi|=k-i}\binom{r}{\nu}F_{\nu}\binom{r}{\xi}G_{\xi}\\
%&=k!\sum_{\nu,\xi,|\nu|+|\xi|=k}\binom{r}{\nu+\xi}F_{\nu}G_{\xi}\\
&=k!\sum_{|\mu|=k}\binom{r}{\mu}H_{\mu}.
}

Since $H(z_1,\dots ,z_r)$ is symmetric, by the above observation, it suffices to prove the statement when $H$ is the power sum symmetric polynomial $p_n(z_1,\dots ,z_r)=z_1^n+\dots +z_r^n$. For each $n\geq 0$, we expand
\equa{H(ze^{x_1},\dots ,ze^{x_r})=p_n(ze^{x_1},\dots ,ze^{x_r})&=\sum_{j=1}^rz^ne^{nx_j}=z^n\left(r+\sum_{i>0}\frac{n^i}{i!}p_i(x_1,\dots ,x_r)\right).}
This means $H_{(0)}(z)=rz^n$ and 
\[D_z^kH_{(0)}(z)=rn^kz^n.\]

Fix $r\geq 1$, we write
\[p_n(x_1,\dots ,x_r)=\sum_{|\mu|=n}C_\mu e_\mu(x_1,\dots ,x_r)\]
for some constant terms $C_\mu$. Evaluate at $x_1=\dots=x_r=1$ and get
\[r=\sum_{|\mu|=n}\binom{r}{\mu}C_\mu.\]
\begin{comment}

Substitute this into (\ref{pow-sum-expansion}) and obtain for any $k\geq 1$, $|\mu|=k$,
\[H_{\mu}(z)=z^n\frac{n^k}{k!}C_\mu.\] 
We shall use the following Newton's identities of symmetric polynomials. For $r, n\geq 1$,
\equanum{\label{newton1}p_n(x_1,\dots ,r_r)&=(-1)^{n-1}ne_n(x_1,\dots ,x_r)+\sum_{i=1}^{n-1}(-1)^{i-1}e_{i}(x_1,\dots ,x_r)p_{n-i}(x_1,\dots ,x_r).}
Suppose for an induction that for any $1\leq k\leq n$,
\[\sum_{|\nu|=k}\binom{r}{\nu}C_\nu=r.\]
\AC{I can prove this directly from the definition without all of the computations above. Use that $e_{\mu}(1,\ldots,1) = {r\choose \mu}$ and plug it into the defining equation. Using $p_n(1,\ldots,1)=r$ you obtain the result.}

The base case of this induction is the trivial case $n=1$. Identity (\ref{newton1}) gives us
\equa{p_n=(-1)^{n-1}ne_n+\sum_{i=1}^{n-1}(-1)^{i-1}e_{i}\sum_{|\mu|=n-i}C_\mu e_\mu.}
By comparing coefficients, we get
\AC{You are not comparing coefficients your are evaluating at $x_i = 1$ for all $i$ right?}
\equa{\sum_{|\mu|=n}\binom{r}{\mu}C_\mu&=(-1)^{n-1}n\binom{r}{n}+\sum_{i=1}^{n-1}(-1)^{i-1}\binom{r}{i}\sum_{|\nu|=n-i}\binom{r}{\nu}C_\nu\\
&=(-1)^{n-1}r\binom{r-1}{n-1}+\sum_{i=1}^{n-1}(-1)^{i-1}\binom{r}{i}r\\
&=r\cdot\left((-1)^{n-1}\binom{r-1}{n-1}+\sum_{i=1}^{n-1}(-1)^{i-1}\binom{r}{i}\right)\\
&=r
}
where the last equality is a standard property of binomial coefficients. This finishes the induction. 
\end{comment}
Hence
\[k!\sum_{|\mu|=k}\binom{r}{\mu}H_\mu(z)=z^nn^k\sum_{|\mu|=k}\binom{r}{\mu}C_\mu=rn^kz^n=D_z^kH_{(0)}(z).\]
A quick calculation for the $k=0$ or $r=0$ cases finishes the proof.

\end{proof}


Now we proceed with the virtual case. Recall that on Hilbert schemes, the obstruction theory at a fixed point $[Z_\mu]$ is given by $(K^{[n]}_S)^\vee|_{Z_\mu}$, so
\[\frac{1}{e(T^\vir_{Z_\mu})}=\frac{e((K_S^{[n]})^\vee|_{Z_\mu})}{e(T_{Z_\mu})} =(-1)^{|\mu|}\frac{e((K_S^{[n]})|_{Z_\mu})}{e(T_{Z_\mu})}.\] 
\begin{comment}
Similar to Proposition \ref{prop:chern-ver-limit}, the virtual Chern series on Hilbert schemes can be extracted from the master partition function as follows
\equanum{\label{eqn:chern-limit}{\mathcal{C}}_S(\O_S,V;q)=\lim_{\e\->0}\Omega\left(q\e^{1-r}(1+\e)^r;\frac{e^{-\e v_1}}{1+\e},\dots,\frac{e^{-\e v_r}}{1+\e},e^{\e c_1(K_S)};e^{\e\lambda_1},e^{\e\lambda_2}\right).
}
Considering $z$ as the weight of a trivial $\CC^*$-action on $S$ and $\hilb^n(S)$, we write $z=e^l$ where $l=c_1(z)$. We shall focus on the case where $V=L=\O_S\<v_1\>$ is a line bundle. Applying the $r=2$ version of (\ref{eqn:log-total}) setting $w_{2}=c_1(K_S)-l$, we obtain the following expansion:
\equa{&\log \Omega\left(q;ze^{c_1(L)},ze^{-c_1(K_S)-l};e^{-\lambda_1},e^{-\lambda_2}\right)\\
=&\lam_1^{-1}\lam_2^{-1}\cdot (H_{(0),-1,-1}+e_1(w_1,-c_1(K_S)-l)H_{(1),-1,-1}\\
&\indent +e_2(w_1,-c_1(K_S)-l)H_{(2),-1,-1}+e_1(w_1,-c_1(K_S)-l)^2H_{(1,1),-1,-1})\\
&+(\lam_1^{-1}+\lam_2^{-1})\cdot\left(H_{(0),-1,0}+e_1(w_1,-c_1(K_S)-l)H_{(1),-1,0}\right)\\
&+(\lam_1^{-1}\lam_2+\lam_1\lam_2^{-1})\cdot H_{(0),-1,1}+H_{(0),0,0}.
}
Similar to the previous section, the series $H_{\mu,k_1,k_2}$ in the right-hand side are already found in (\ref{eqn:deg0}) and (\ref{eqn:H-omega-fomula}), and we would like to take the limit (\ref{eqn:chern-limit}). Make substitutions $q\leadsto q(1+\e), z\leadsto(1+\e)^{-1}, w_1\leadsto-\e w_1, \vec\lam\leadsto-\e \vec \lam$, then take $\e\->0$. Most of the above summands will then vanish or cancel out, and we are left with
\[\log {\mathcal{C}}_S(\O_S,L;q)=\log(1-q)\int_Sc_1(K_S)+\log(1-q)\int_Sc_1(L)c_1(K_S)\]
Therefore
\equa{{\mathcal{C}}_S(\O_S,L;w)=(1-q)^{\int_Sc(L)c_1(K_S)}=\left(\frac1{1-q}\right)^{\int_Sc(L)c_1(S)}.}
\end{comment}
Let $L=\O_S\<v_1\>$ be an equivariant line bundle, and $V=L\oplus\O_S\<v_2\>$. Apply (\ref{eqn:chern-rank-2}) to $V$ and we have
\[I^{\mathcal{C}}(V;q)=(1+q)^{\int_Sc(V)}=(1+q)^{\int_S(1+w_1+w_2+w_1w_2)}.\]
Set $w_2=c_1(K_S)-1$ and replace $q$ by $-q$, then this becomes
\[I^{\mathcal{C}}(V;-q)|_{w_2=c_1(K_S)-1}=(1-q)^{\int_Sc(L)c_1(K_S)}.\]
On the other hand, we have by definition
\equa{&I^{\mathcal{C}}(V;-q)|_{w_2=c_1(K_S)-1}\\
=&\sum_{\mu} (-1)^{|\mu|}q^{|\mu|}\prod_{\square\in\mu}\frac{(1+w_1-c(\square)\lam_1-r(\square)\lam_2)(c_1(K_S)-c(\square)\lam_1-r(\square)\lam_2)}{((a(\square)+1)\lambda_1-l(\square)\lambda_2)((l(\square)+1)\lambda_2-a(\square)\lambda_1)}\\
=&\sum_{\mu}(-1)^{|\mu|}q^{|\mu|}\frac{c(L^{[n]}|_{Z_\mu})e((K_S^{[n]})|_{Z_\mu})}{e(T|_{Z_\mu})}\\
=&\sum_{\mu}q^{|\mu|}\frac{c(L^{[n]}|_{Z_\mu})}{e(T^\vir|_{Z_\mu})}=\mathcal{C}_S(\O_S,L;q)
}
Therefore we conclude
\equa{{\mathcal{C}}_S(\O_S,L;w)=(1-q)^{\int_Sc(L)c_1(K_S)}=\left(\frac1{1-q}\right)^{\int_Sc(L)c_1(S)}.}
\begin{comment}
\AC{Here is a shorter proof of the above:
Start by noting that $c(e^uK_S^{[n]}) = (1+u)^nc_{(1+u)^{-1}}(K_S^{[n]})$ so we have that 
$$
\sum_{n\geq 0}q^n\int_{\hilb} c(L^{[n]}) c_{n}(K_S^{[n]}) = \sum_{n\geq 0}q^n\int_{\hilb} c(L^{[n]}) c(e^uK_S^{[n]})|_{c(e^u)=0}q,.
$$
Since the first left-hand side is equal to $(1+q)^{c(L)\cdot\big(c(e^u)+c_1(K_S)\big)}$, setting $c(e^u)$ equal to zero gives us the required result.
}
\end{comment}
In particular, restricting to the lowest degree part in the variables $\lam_1,\lam_2,w_1$, we obtain the following Corollary.
\begin{corollary}\label{cor:nek2d}For $S=\CC^2$, the following equality holds
\[\sum_{n=1}^\infty q^n\int_{[\hilb^n(S)]^\vir}1:=\sum_{Z\in\hilb^n(S)^\T}\frac{1}{e(T^\vir_Z)}=e^{\frac{(\lambda_1+\lambda_2)}{\lambda_1\lambda_2}q}.\]
\end{corollary}


\subsection{Segre-Verlinde correspondence in non-zero degrees}\label{sec:reduced-computation} \input{2.2new-computation}


\subsection{Strong Segre symmetry and weak Verlinde symmetry}\label{sec:sym}
Let $r>0$. According to Theorem \ref{thm:SV2d-deg-pos}, the following identity holds for the Segre series
\equa{&[q^n]\sum_{|\mu|=k}\binom{r}{\mu}\log A^{r,N}_{\mu,(0),(0)}((-1)^Nq)=[q^n]\sum_{|\xi|=k}\binom{N}{\xi}\log A^{r,N}_{(0),(0),\xi}((-1)^Nq)\\
=&(-1)^{nN-1}\frac{r}{n}(-n(r+N))_{(k-1)}\binom{-nr-1}{nN-1}\\
=&(-1)^{nN-1}\frac{r}{n}\cdot\frac{(-nr-1)\cdots (-n(r+N)-k+2)}{(nN-1)!}\\
=&(-1)^{k-1}rN\cdot(n(r+N)+k-2)_{(k-2)}\binom{n(r+N)}{nN}
}
The right-hand side does not change if we swap $r$ and $N$, that is
\equa{\sum_{|\mu|=k}\binom{r}{\mu}\log A^{r,N}_{\mu,(0),(0)}((-1)^Nq)=\sum_{|\mu|=k}\binom{r}{\mu}\log A^{N,r}_{(0),(0),\mu}((-1)^rq).}
This is consistent with the strong Segre symmetry of Conjecture \ref{con:strong-sym}. We have checked that this conjecture holds when
\begin{equation}
\label{eq:2dsegsym}
\begin{cases}
n=1,\text{for $N\leq 5$, $r\leq 3$,}\\
n=2,\text{for $N\leq 3$, $r\leq 3$,}\\
n=3,\text{for $N\leq 3$, $r\leq 2$,}\\
n=4,5,\text{for $N\leq 2$, $r=1$.}\\
\end{cases}
\end{equation}

As for the Verlinde series, the weak Segre symmetry of Corollary \ref{cor:sv-sym2d-intro} together with the weak Segre-Verlinde correspondence of Corollary \ref{cor:weak-SV2d-virtual-intro} would imply a weak Verlinde symmetry. However, calculations using a computer program show the ``strong'' Verlinde symmetry does not hold for $S=\CC^2$. This can also be observed from the fact that the equivariant Verlinde series only depends on $V$ through $c_1(V)$ but depends on $E$ through $c_1(E),c_2(E),\dots,c_N(E)$ thus breaking the symmetry.